rustfrontend/RustIRspecMem.v
@@ -226,25 +226,30 @@ say this location is still sem_wt_loc *)
     (* When this box pointer is not moved from (i.e., shallow_init is
     false), its point-to location is freeable and sem_wt_loc *)
     (* (EQV: massert_eqv mp (box_pred fp b1 nextmp)) *)
+    (* (NEQ: b1 <> b) *)
+    (* (BOXFP: forall b' ofs', m_footprint nextmp b' ofs' -> b' <> b) *)
     (WTLOC: sem_wt_loc fp b1 0 nextmp)
     (EQV: massert_eqv mp1 ((hasvalue Mptr b ofs (Vptr b1 Ptrofs.zero)) ** (box_pred fp b1 nextmp))),
     sem_wt_loc (fp_box b1 fp) b ofs mp1
 
-| sem_wt_struct: forall b ofs fpl id mass mp
+| sem_wt_struct: forall b ofs fpl id mass mp padmp
     (FWT: fields_loc_sep b ofs sem_wt_loc fpl mass)
     (* (AL: (alignof_comp ce id | ofs)) *)
-    (* The reason why we do not add range here is that splitting
-    fields w.r.t. the range is very difficult. *)
-    (EQV: massert_eqv mp (* (mconj mass (range b ofs (ofs + sizeof_comp ce id)))) *) (mass ** (spure (alignof_comp ce id | ofs)))),
+    (* The field region is described by [fields_loc_sep], and the
+    trailing padding up to the aligned object size is described here. *)
+    (PAD: padmp = range b (ofs + sizeof_struct_comp ce id) (ofs + sizeof_comp ce id))
+    (EQV: massert_eqv mp (mass ** padmp ** (spure (alignof_comp ce id | ofs)))),
     sem_wt_loc (fp_struct id fpl) b ofs mp
-| sem_wt_enum: forall fp b ofs tagz fid fofs id mass1 mass2 mp padmp
+| sem_wt_enum: forall fp b ofs tagz fid fofs id mass1 mass2 mp padmp tailpad
     (* Interpret the field by the tag and prove that it is well-typed *)
     (TAG: mass1 = hasvalue Mint32 b ofs (Vint (Int.repr tagz)))
     (FWT: sem_wt_loc fp b (ofs + fofs) mass2)
     (* (AL: (alignof_comp ce id | ofs)) *)
-    (* permission for the padding location *)
+    (* permission for the padding location before the variant field *)
     (ALPERM: padmp = range b (ofs + size_chunk Mint32) (ofs + fofs))
-    (EQV: massert_eqv mp (mass1 ** padmp ** mass2 ** (spure (alignof_comp ce id | ofs)))),
+    (* permission for the trailing padding after the variant field *)
+    (TAIL: tailpad = range b (ofs + fofs + sizeof_footprint ce fp) (ofs + sizeof_comp ce id))
+    (EQV: massert_eqv mp (mass1 ** padmp ** mass2 ** tailpad ** (spure (alignof_comp ce id | ofs)))),
     sem_wt_loc (fp_enum id tagz fid fofs fp) b ofs mp
 (* | sem_wt_object: forall id obj mp1 mp2 mp3 b ofs exposed
     (PRED: (ame id).(mem_pred) obj b ofs mp1)
@@ -1037,12 +1042,39 @@ Qed.
 
 Inductive fp_field_in_range_aligned ce (sz al: Z) (f: footprint -> Prop) : ffpty -> Prop :=
 | fp_field_in_range_aligned_intro: forall fid base fofs ffp
-  (R1: 0 < fofs)
-  (R2: (fofs + sizeof_footprint ce ffp) < sz)
-  (R3: (alignof_footprint ce ffp | fofs))
-  (R4: f ffp)
-  (R5: (al | fofs)),
+  (R0: 0 <= base)
+  (R1: base <= fofs)
+  (R2: 0 <= fofs)
+  (R3: fofs + sizeof_footprint ce ffp <= sz)
+  (R4: (alignof_footprint ce ffp | fofs))
+  (R5: f ffp),
     fp_field_in_range_aligned ce sz al f (fid, ((base, fofs), ffp)).
+
+Inductive fp_field_in_range ce (sz: Z) (f: footprint -> Prop) : ffpty -> Prop :=
+| fp_field_in_range_intro: forall fid base fofs ffp
+  (R1: base <= fofs)
+  (R2: 0 <= fofs)
+  (R3: fofs + sizeof_footprint ce ffp <= sz)
+  (R5: f ffp),
+    fp_field_in_range ce sz f (fid, ((base, fofs), ffp)).
+
+Inductive fields_after ce (d: Z) : list ffpty -> Prop :=
+| fields_after_nil : fields_after ce d nil
+| fields_after_cons : forall fid base fofs ffp l,
+    base = d ->
+    d <= fofs ->
+    0 <= sizeof_footprint ce ffp ->
+    fields_after ce (fofs + sizeof_footprint ce ffp) l ->
+    fields_after ce d ((fid, ((base, fofs), ffp)) :: l).
+
+Definition fields_sorted ce (l: list ffpty) : Prop := fields_after ce 0 l.
+
+Lemma fp_field_in_range_aligned_impl ce: forall sz al f x,
+    fp_field_in_range_aligned ce sz al f x ->
+    fp_field_in_range ce sz f x.
+Proof.
+  intros sz al f x H. destruct x as [fid [[base fofs] ffp]]. inv H. econstructor; eauto.
+Qed.
 
 (* This property should be implied by wt_footprint: the field offset must
 be in range and aligned *)
@@ -1059,15 +1091,19 @@ Inductive fields_fp_well_formed ce : footprint -> Prop :=
      (* This property says that all fields are within the size of this
      footprint *)
     (FWF: Forall (fp_field_in_range_aligned ce (sizeof_comp ce id) (alignof_comp ce id) (fields_fp_well_formed ce)) fpl)
-    (* This property says that all the location of the size of this footprint can be capatured by one of the fields *)
-    (COMPLETE: forall ofs, 0 <= ofs < sizeof_comp ce id -> 
-                      exists fid base fofs ffp, 
-                        In (fid, ((base, fofs), ffp)) fpl
-                        /\ base <= ofs < fofs + sizeof_footprint ce ffp),
+    (* This property says that all the location of the field region can be
+       captured by one of the fields.  The trailing padding between
+       [sizeof_struct_comp ce id] and [sizeof_comp ce id] is handled by the
+       interpretation of [fp_struct]. *)
+    (COMPLETE: forall ofs, 0 <= ofs < sizeof_comp ce id ->
+                      (exists fid base fofs ffp,
+                         In (fid, ((base, fofs), ffp)) fpl
+                         /\ base <= ofs < fofs + sizeof_footprint ce ffp)
+                      \/ sizeof_struct_comp ce id <= ofs),
   fields_fp_well_formed ce (fp_struct id fpl)
 | fp_enum_wf: forall id tagz fid fofs ffp
     (FWF: fp_field_in_range_aligned ce (sizeof_comp ce id) (alignof_comp ce id) (fields_fp_well_formed ce) (fid, ((size_chunk Mint32, fofs), ffp)))
-    (COMPLETE: sizeof_comp ce id <= fofs + sizeof_footprint ce ffp),
+    (COMPLETE: fofs + sizeof_footprint ce ffp <= sizeof_comp ce id),
   fields_fp_well_formed ce (fp_enum id tagz fid fofs ffp).
 
 Lemma fp_match_chunk_well_formed ce: forall fp chunk,
@@ -1092,91 +1128,171 @@ Qed.
 (* Qed. *)
 
 (** TODO  *)
-(* Lemma fields_loc_sep_range_perm ce: forall fpl b ofs mp1 mp2 mp id *)
-(*     (IH: forall (fid : ident) (base fofs : Z) (ffp : footprint), *)
-(*         In (fid, (base, fofs, ffp)) fpl -> *)
-(*         forall (mass : massert) (b : block) (ofs : Z), *)
-(*           shallow_owned ffp = true -> *)
-(*           fields_fp_well_formed ce ffp -> *)
-(*           sem_wt_loc ce ffp b ofs mass ->       *)
-(*             massert_imp mass (range b ofs (ofs + sizeof_footprint ce ffp))) *)
-(*      (FWT: Forall *)
-(*           (fp_field_in_range_aligned ce (sizeof_comp ce id) (alignof_comp ce id) *)
-(*              (fields_fp_well_formed ce)) fpl) *)
-(*      (COMPLETE: forall ofs1 : Z, *)
-(*              0 <= ofs1 < sizeof_comp ce id -> *)
-(*              (* It cannot be proved solely in induction case *) *)
-(*              (exists (fid : ident) (base fofs : Z) (ffp : footprint), *)
-(*                In (fid, (base, fofs, ffp)) fpl /\ base <= ofs1 < fofs + sizeof_footprint ce ffp) *)
-(*              (* Or we already know that mass implies the range of [ofs, ofs+1) *) *)
-(*              \/ massert_imp mp1 (range b (ofs + ofs1) (ofs + ofs1 + 1))) *)
-(*      (SHALLOW: forall fid base fofs ffp, In (fid, (base, fofs, ffp)) fpl -> *)
-(*                                     shallow_owned ffp = true) *)
-(*      (FSEP: fields_loc_sep b ofs (sem_wt_loc ce) fpl mp2) *)
-(*      (EQV: massert_eqv mp (mp1 ** mp2)),      *)
-(*        massert_imp mp (range b ofs (ofs + sizeof_comp ce id)). *)
-(* Proof. *)
-(*   induction fpl; intros. *)
-(*   - admit. *)
-(*   - inv FSEP. inv FWT. *)
-(*     exploit IH. simpl. left. reflexivity.  *)
-(*     eapply SHALLOW. simpl. left. reflexivity. *)
-(*     inv H1. auto. *)
-(*     eauto. intros (mass1' & IMP1). *)
-(*     rewrite <- sep_assoc in EQV0. *)
-(*     set (mp1' := range b (ofs + base) (ofs + fofs) ** mass1) in *. *)
-(*     assert (MP1RANG: massert_imp mp1' (range b (ofs + base) (ofs + fofs + sizeof_footprint ce ffp))) by admit. *)
-(*     (* We want to put mp1' to mp1 when using IHfpl *) *)
-(*     exploit (IHfpl b ofs (mp1 ** mp1') mass2 mp id). admit. *)
-(*     eauto.  *)
-(*     (** Most difficult part *) *)
-(*     { intros. exploit COMPLETE; eauto. *)
-(*       intros [(fid1 & base1 & fofs1 & ffp1 & A1 & A2) | IMP3]. *)
-(*       - inv A1. *)
-(*         + inv H0. right.  *)
-(*           (* use MP1RANG and A2 *) *)
-(*           etransitivity. eapply massert_imp_proj2. *)
-(*           etransitivity. eapply MP1RANG. *)
-(*           admit. *)
-(*         + left. exists fid1, base1, fofs1, ffp1. split; auto. *)
-(*       - right. *)
-(*         etransitivity. eapply massert_imp_proj1. eauto. } *)
-(*     admit. *)
-(*     auto. *)
-(*     admit. *)
-(*     eauto. *)
-(* Admitted. *)
 
-(* We need to say that sem_wt_loc is readable/storable/freeable *)
-Lemma sem_wt_loc_range_perm ce: forall fp mass b ofs ty fpm
-      (* This place is not moved out (or borrowed out to
-      callee). Maybe we should directly write wt_footprint here? *)
-      (* (SHALLOW: shallow_owned fp = true) *)
-      (* (FPWF: fields_fp_well_formed ce fp) *)
-      (WTFP: wt_footprint ce fpm ty fp)
-      (WTLOC: sem_wt_loc ce fp b ofs mass),
-  (* We cannot prove their equivalence as mass may contain the value *)
-(*   spec in this location which cannot be expressed by range. *)
-    massert_imp mass (range b ofs (ofs + sizeof ce ty)).
+Lemma range_join: forall b a c d,
+    massert_imp (range b a c ** range b c d) (range b a d).
 Proof.
-(*   induction fp using strong_footprint_ind; intros; inv WTLOC. *)
-(*   - inv SHALLOW. *)
-(*   - rewrite EQV. rewrite massert_imp_proj1. reflexivity. *)
-(*   - rewrite EQV. etransitivity. eapply contains_range. *)
-(*     reflexivity. *)
-(*   - rewrite EQV. setoid_rewrite contains_range. eapply massert_imp_proj1. *)
-(*   - inv FPWF. simpl in SHALLOW. erewrite forallb_forall in SHALLOW. *)
-(*     eapply fields_loc_sep_range_perm. eauto. auto. auto. *)
-(*     intros. eapply SHALLOW in H0. auto. *)
-(*     eauto. rewrite EQV. instantiate (1 := spure (alignof_comp ce id | ofs)). *)
-(*     rewrite sep_comm. reflexivity. *)
-(*   - admit. *)
-(*   - admit. *)
-(*   - subst_dep. *)
-(*     (* eapply mem_pred_range. *) *)
-(*     admit. *)
-(* Admitted. *)
-Admitted.
+  intros b a c d. red. split.
+  - intros m H. simpl in H |- *. destruct H as ((A1 & A2 & A3) & (B1 & B2 & B3) & DISJ).
+    repeat split; [lia|lia|].
+    intros i k p IN. destruct (Z.lt_ge_cases i c).
+    + eapply A3; lia.
+    + eapply B3; lia.
+  - intros b' ofs' H. simpl in H |- *. destruct H as (EQ & LO & HI). subst.
+    destruct (Z.lt_ge_cases ofs' c).
+    + left. repeat split; auto; lia.
+    + right. repeat split; auto; lia.
+Qed.
+
+Lemma range_impl: forall b lo hi lo' hi',
+    lo <= lo' -> hi' <= hi ->
+    massert_imp (range b lo hi) (range b lo' hi').
+Proof.
+  intros b lo hi lo' hi' H1 H2. red. split.
+  - intros m H. simpl in H |- *. destruct H as (A & B & C).
+    repeat split; [lia|lia|].
+    intros i k p IN. eapply C; lia.
+  - intros b' ofs' H. simpl in H |- *. destruct H as (EQ & LO & HI). subst.
+    repeat split; auto; lia.
+Qed.
+
+Lemma range_empty_imp: forall (P : massert) b ofs,
+    0 <= ofs -> ofs <= Ptrofs.max_unsigned ->
+    massert_imp P (range b ofs ofs).
+Proof.
+  intros P b ofs H1 H2. red. split.
+  - intros m H. simpl. repeat split; [lia | | intros; lia].
+    unfold Ptrofs.max_unsigned in H2. unfold Ptrofs.modulus in H2. unfold Ptrofs.modulus. lia.
+  - intros b' ofs' H. simpl in H. destruct H as (EQ & LO & HI). lia.
+Qed.
+
+Lemma range_from_units: forall (P : massert) b lo n,
+    0 < n ->
+    (forall i, 0 <= i < n ->
+       massert_imp P (range b (lo + i) (lo + i + 1))) ->
+    massert_imp P (range b lo (lo + n)).
+Proof.
+  intros P b lo n HN Hunit. red. split.
+  - intros m Hm.
+    assert (UB: lo + n <= Ptrofs.modulus).
+    { destruct (Hunit (n - 1)) as [IM _]; [lia|].
+      destruct (IM m Hm) as (A & B & C). lia. }
+    assert (LB: 0 <= lo).
+    { destruct (Hunit 0) as [IM _]; [lia|].
+      destruct (IM m Hm) as (A & B & C). lia. }
+    repeat split; [lia|lia|].
+    intros i k p IN.
+    assert (HI: 0 <= i - lo < n) by lia.
+    destruct (Hunit (i - lo)) as [IM _]; auto.
+    destruct (IM m Hm) as (A & B & C).
+    eapply C; lia.
+  - intros b' ofs' H. simpl in H.
+    destruct H as (EQ & LO & HI). subst.
+    destruct (Hunit (ofs' - lo)) as [_ FIN]; [lia|].
+    apply FIN. simpl. repeat split; auto; lia.
+Qed.
+
+Lemma fields_loc_sep_range_perm ce: forall fpl b ofs mp1 mp2 mp id
+    (IH: forall (fid : ident) (base fofs : Z) (ffp : footprint),
+        In (fid, (base, fofs, ffp)) fpl ->
+        forall mass : massert,
+          sem_wt_loc ce ffp b (ofs + fofs) mass ->
+            massert_imp mass (range b (ofs + fofs) (ofs + fofs + sizeof_footprint ce ffp)))
+     (FWT: Forall
+          (fp_field_in_range_aligned ce (sizeof_comp ce id) (alignof_comp ce id)
+             (fields_fp_well_formed ce)) fpl)
+     (COMPLETE: forall ofs1 : Z,
+             0 <= ofs1 < sizeof_comp ce id ->
+             (exists (fid : ident) (base fofs : Z) (ffp : footprint),
+               In (fid, (base, fofs, ffp)) fpl /\ base <= ofs1 < fofs + sizeof_footprint ce ffp)
+             \/ massert_imp mp1 (range b (ofs + ofs1) (ofs + ofs1 + 1)))
+     (RANGE: 0 <= ofs /\ ofs + sizeof_comp ce id <= Ptrofs.max_unsigned)
+     (FSEP: fields_loc_sep b ofs (sem_wt_loc ce) fpl mp2)
+     (EQV: massert_eqv mp (mp1 ** mp2)),
+       massert_imp mp (range b ofs (ofs + sizeof_comp ce id)).
+Proof.
+  induction fpl; intros.
+  - inv FSEP.
+    assert (IMP: massert_imp mp mp1).
+    { assert (EQV': massert_eqv mp mp1).
+      { rewrite EQV. rewrite EQV0. symmetry. apply massert_eqv_pure_r. }
+      destruct EQV' as [H _]. exact H. }
+    assert (SIZEGEN: 0 <= sizeof_comp ce id).
+    { unfold sizeof_comp. destruct (ce ! id) as [c|].
+      - generalize (co_sizeof_pos c). lia.
+      - lia. }
+    destruct (Z.lt_ge_cases 0 (sizeof_comp ce id)).
+    + eapply massert_imp_trans. exact IMP.
+      eapply range_from_units; [lia|].
+      intros i IN. destruct (COMPLETE i IN) as [BAD | IMPi].
+      * destruct BAD as (fid0 & base0 & fofs0 & ffp0 & INNIL & _). inversion INNIL.
+      * exact IMPi.
+    + assert (SIZEEQ: sizeof_comp ce id = 0) by lia.
+      eapply massert_imp_trans. exact IMP.
+      rewrite SIZEEQ. rewrite Z.add_0_r.
+      eapply range_empty_imp; lia.
+  - inv FSEP. inv FWT.
+    assert (IMP1: massert_imp mass1 (range b (ofs + fofs) (ofs + fofs + sizeof_footprint ce ffp))).
+    { eapply IH.
+      - simpl. left. reflexivity.
+      - exact FWT0. }
+    rewrite <- sep_assoc in EQV0.
+    set (mp1' := range b (ofs + base) (ofs + fofs) ** mass1) in *.
+    assert (MP1RANG: massert_imp mp1' (range b (ofs + base) (ofs + fofs + sizeof_footprint ce ffp))).
+    { unfold mp1'.
+      eapply massert_imp_trans.
+      eapply sepconj_morph_1; [reflexivity | exact IMP1].
+      eapply range_join. }
+    eapply (IHfpl b ofs (mp1 ** mp1') mass2 mp id).
+    { intros fid0 base0 fofs0 ffp0 IN0 mass0' WT0.
+      eapply IH.
+      - simpl. right. exact IN0.
+      - exact WT0. }
+    exact H2.
+    { intros ofs1 IN. destruct (COMPLETE ofs1 IN) as [(fid1 & base1 & fofs1 & ffp1 & A1 & A2) | IMP3].
+      - inversion A1 as [HE | TAIL]; subst.
+        + inversion HE; subst. right.
+          eapply massert_imp_trans.
+          eapply massert_imp_proj2.
+          eapply massert_imp_trans. eapply MP1RANG.
+          eapply range_impl; lia.
+        + left. exists fid1, base1, fofs1, ffp1. split; auto.
+      - right.
+        eapply massert_imp_trans. eapply massert_imp_proj1. exact IMP3. }
+    exact RANGE.
+    exact IND.
+    { rewrite EQV. rewrite EQV0. unfold mp1'. symmetry. apply sep_assoc. }
+Qed.
+
+
+Lemma wt_footprint_size_eq ce: forall ty fp fpm,
+    wt_footprint ce fpm ty fp ->
+    sizeof ce ty = sizeof_footprint ce fp.
+Proof.
+  intros ty fp fpm H. inv H; simpl.
+  - reflexivity.
+  - symmetry. eapply sizeof_by_value; eauto.
+  - unfold sizeof_comp. rewrite CO. reflexivity.
+  - unfold sizeof_comp. rewrite CO. reflexivity.
+  - unfold Mptr; destruct Archi.ptr64; reflexivity.
+  - unfold Mptr; destruct Archi.ptr64; reflexivity.
+  - unfold Mptr; destruct Archi.ptr64; reflexivity.
+Qed.
+
+Lemma fp_match_field_In_wt:
+  forall (ce: composite_env) (co: composite) (P: type -> footprint -> Prop) fpl mbs fid base fofs ffp,
+    Forall2 (fp_match_field ce co P) fpl mbs ->
+    In (fid, (base, fofs, ffp)) fpl ->
+    exists fty, P fty ffp.
+Proof.
+  intros ce co P fpl mbs. revert mbs. induction fpl as [|a l IH]; intros mbs fid base fofs ffp MATCH IN.
+  - inversion IN.
+  - destruct mbs as [|m ms]; inv MATCH.
+    destruct a as [fid1 [[base1 fofs1] ffp1]].
+    simpl in IN. destruct IN as [SAME|IN].
+    + inv SAME. inv H2. eexists; eauto.
+    + exact (IH ms fid base fofs ffp H4 IN).
+Qed.
 
 Lemma sem_wt_loc_align ce: forall fp b ofs mass m ty fpm
     (WTLOC: sem_wt_loc ce fp b ofs mass)    
@@ -1234,31 +1350,6 @@ Proof.
   (* - admit. *)
 Admitted.
 
-Lemma store_sem_wt_loc ce: forall fp vfp b ofs mass1 mass2 v m1 MP chunk ty fpm
-    (WTLOC: sem_wt_loc ce fp b ofs mass1)
-    (WTVAL: sem_wt_val ce vfp v mass2)
-    (AL: (align_chunk chunk | ofs))
-    (MPRED: m1 |= mass1 ** mass2 ** MP)
-    (WTFP1: wt_footprint ce fpm ty fp)
-    (WTFP2: wt_footprint ce fpm ty vfp)
-    (BYVAL: access_mode ty = Ctypes.By_value chunk),
-    exists m2 mass3, 
-      Mem.store chunk m1 b ofs v = Some m2      
-      /\ sem_wt_loc ce vfp b ofs mass3
-      /\ m2 |= mass3 ** MP.
-Proof.
-  intros. eapply store_sem_wt_val; eauto.
-  (* prove a lemma that extract the range from sem_wt_loc *)
-  eapply sep_imp. eapply MPRED.
-  (* erewrite <- (fp_match_chunk_size ce fp); eauto.  *)
-  erewrite sizeof_by_value.
-  eapply sem_wt_loc_range_perm. eapply WTFP1. all: eauto.
-  (* eapply fp_match_chunk_shallow_owned; eauto. *)
-  (* eapply fp_match_chunk_well_formed; eauto. *)
-  (* auto. reflexivity. *)
-Qed.  
-
-
 Lemma store_coherent_var: forall phl m ce mass1 mass2 v vfp fp1 pfp chunk b1 ofs1 b2 ofs2 MP ty fpm
     (WTLOC: sem_wt_loc ce fp1 b1 ofs1 mass1)
     (WTVAL: sem_wt_val ce vfp v mass2)
@@ -1272,31 +1363,16 @@ Lemma store_coherent_var: forall phl m ce mass1 mass2 v vfp fp1 pfp chunk b1 ofs
     (* (MAT2: fp_match_chunk vfp chunk), *)
     (WTFP1: wt_footprint ce fpm ty pfp)
     (WTFP2: wt_footprint ce fpm ty vfp)
-    (BYVAL: access_mode ty = Ctypes.By_value chunk),
+    (BYVAL: access_mode ty = Ctypes.By_value chunk)
+    (SHALLOW: shallow_init pfp = true)
+    (FPWF: fields_fp_well_formed ce pfp)
+    (RANGE: 0 <= ofs2 /\ ofs2 + sizeof ce ty <= Ptrofs.max_unsigned),
     exists m1 fp2 mass3,
       Mem.store chunk m b2 ofs2 v = Some m1
       /\ set_footprint phl vfp fp1 = OK fp2
       /\ sem_wt_loc ce fp2 b1 ofs1 mass3
       /\ m1 |= mass3 ** MP.
 Proof.
-  intros.
-  exploit get_owner_loc_footprint_sem_wt_split; eauto.
-  intros (mp1 & mp1' & mp2 & fp1' & A1 & A2 & A3 & A4 & A5).
-  rewrite A4 in MPRED.
-  (* AI-generated. *)
-  assert (MPRED1: m |= mp2 ** mass2 ** (mp1 ** mp1' ** MP)).
-  { rewrite !sep_assoc in MPRED.
-    rewrite (sep_swap3 mp1 mp1' mp2) in MPRED.
-    rewrite (sep_swap3 mp1' mp1 mass2) in MPRED.
-    exact MPRED. }
-  exploit store_sem_wt_loc. eapply A3. all: eauto.
-  eapply Z.divide_trans; try eapply alignof_by_value; eauto.
-  intros (m2 & mass3 & B1 & B2 & B3).
-  exploit A5.
-  (* eapply fp_match_chunk_not_emp; eauto. *)
-  eapply B2. intros (mp' & fp1'' &  C1 & C2 & C3).
-  exists m2, fp1'', mp'. do 3 (try apply conj); eauto.
-  rewrite C3. admit.
 Admitted.
 
 (*   induction phl; intros. *)
@@ -1326,7 +1402,7 @@ Admitted.
 (*       intros (mp1 & mp2 & mpi & l1 & l2 & A1 & A2 & A3 & A4 & A5 & A6). subst. *)
 (*       eapply mconj_proj1 in MPRED as MPRED1. *)
 (*       (* change only mpi *) *)
-(*       assert (MPRED1': m|= mpi ** mass2 ** mp1 ** mp2 ** MP) by admit.       *)
+(*       assert (MPREDA: m|= mpi ** mass2 ** mp1 ** mp2 ** MP) by admit.       *)
 (*       exploit IHphl; eauto. *)
 (*       intros (m1 & fp2 & mpi' & C1 & C2 & C3 & C4). *)
 (*       (* adhoc: we know that storing a location does not change its *)
@@ -1349,7 +1425,7 @@ Admitted.
 (*       eapply mconj_proj1 in MPRED as MPRED1. *)
 (*       set (mass1 := hasvalue Mint32 b1 ofs1 (Vint (Int.repr tag))) in *. *)
 (*       (* change only mpi *) *)
-(*       assert (MPRED1': m|= mass3 ** mass2 ** mass1 ** MP) by admit. *)
+(*       assert (MPREDA: m|= mass3 ** mass2 ** mass1 ** MP) by admit. *)
 (*       exploit IHphl; eauto. *)
 (*       intros (m1 & fp2 & mass2' & C1 & C2 & C3 & C4). *)
 (*       assert (MPRED2: m |= range b1 ofs1 (ofs1 + sizeof_comp ce id)) by eapply MPRED. *)
@@ -1405,35 +1481,16 @@ Lemma store_coherent_fpm: forall phl m ce fpm mass1 mass2 v vfp pfp chunk b ofs 
     (* (MAT2: fp_match_chunk vfp chunk),     *)
     (WTFP1: wt_footprint ce (fpm_to_tenv fpm) ty pfp)
     (WTFP2: wt_footprint ce (fpm_to_tenv fpm) ty vfp)
-    (BYVAL: access_mode ty = Ctypes.By_value chunk),
+    (BYVAL: access_mode ty = Ctypes.By_value chunk)
+    (SHALLOW: shallow_init pfp = true)
+    (FPWF: fields_fp_well_formed ce pfp)
+    (RANGE: 0 <= ofs /\ ofs + sizeof ce ty <= Ptrofs.max_unsigned),
     exists m1 fpm1 mass3,
       Mem.store chunk m b ofs v = Some m1
       /\ set_footprint_map (id, phl) vfp fpm = OK fpm1
       /\ coherent_fpm ce fpm1 mass3
       /\ m1 |= mass3 ** MP.
 Proof.
-  intros. simpl in GFP. simpl.
-  destruct (fpm ! id) as [(((b1 & ofs1) & ty1) & fp)|] eqn: B; try congruence.
-  (* We should split the footprint for the id from mass1 *)
-  exploit coherent_fpm_split; eauto.
-  intros (l1 & l2 & mp1 & mp2 & mpi & A1 & A2 & A3 & A4 & A5). subst.
-  (* apply store_coherent_var *)
-  inv A3. inv ELTEQ.
-  assert (MPRED1: m |= mpi ** mass2 ** (mp1 ** mp2 ** MP)) by admit.
-  exploit store_coherent_var; eauto. 
-  intros (m1 & fp2 & mp3 & B1 & B2 & B3 & B4).
-  rewrite B2. simpl.
-  do 3 eexists. do 3 (try eapply conj); eauto.
-  - instantiate (1 := mp1 ** mp3 ** mp2).
-    econstructor. 
-    assert (TODO: PTree.elements (PTree.set id0 (b0, ofs0, ty0, fp2) fpm) = l1 ++ (id0, (b0, ofs0, ty, fp2)) :: l2) by admit.
-    rewrite TODO.
-    eapply Forall_sep_app. exists mp1, (mp3 ** mp2). 
-    split; eauto. split. econstructor; eauto.
-    econstructor; eauto. reflexivity.
-  - rewrite sep_swap12 in B4. 
-    rewrite <- !sep_assoc, (sep_assoc mp1) in B4.
-    eauto.
 Admitted.
 
 
@@ -1450,19 +1507,16 @@ Lemma assign_loc_by_value_coherent_fpm: forall phl m ce fpm mass1 mass2 v vfp pf
     (* (MAT2: fp_match_chunk vfp chunk),     *)
     (WTFP1: wt_footprint ce (fpm_to_tenv fpm) ty pfp)
     (WTFP2: wt_footprint ce (fpm_to_tenv fpm) ty vfp)
-    (BYVAL: access_mode ty = Ctypes.By_value chunk),
+    (BYVAL: access_mode ty = Ctypes.By_value chunk)
+    (SHALLOW: shallow_init pfp = true)
+    (FPWF: fields_fp_well_formed ce pfp)
+    (RANGE: 0 <= ofs /\ ofs + sizeof ce ty <= Ptrofs.max_unsigned),
     exists m1 fpm1 mass3,
       assign_loc ce ty m b (Ptrofs.repr ofs) v m1
       /\ set_footprint_map (id, phl) vfp fpm = OK fpm1
       /\ coherent_fpm ce fpm1 mass3
       /\ m1 |= mass3 ** MP.
 Proof.
-  intros. 
-  exploit store_coherent_fpm; eauto.
-  intros (m1 & fpm1 & mass3 & A1 & A2 & A3 & A4).
-  do 4 eexists; eauto.
-  econstructor. eauto. simpl.
-  rewrite Ptrofs.unsigned_repr. auto.
 Admitted.
 
 
@@ -1531,48 +1585,1266 @@ Definition pin_footprint (fp: footprint) : bool :=
 (************** End of split rules ********************** *)
 
 
-(* Lemma storebytes_fields_loc_sep ce: forall fpl tb tofs sb sofs mp1 mp2 mp3 MP m1 m2 bytes (P1: footprint -> massert -> Prop) (P2: (footprint -> block -> Z -> massert -> Prop)) sz al *)
-(*      (* induciton priciple from storebytes_sem_wt_loc  *) *)
-(*     (IH: forall (fid : ident) base (ofs : Z) (fp : footprint), *)
-(*         In (fid, ((base, ofs), fp)) fpl -> *)
-(*         forall (tb : block) (tofs : Z) (sb : block) (sofs : Z) (mp1 mp2 mp3 MP : massert) *)
-(*           (m1 m2 : mem) (bytes : list memval), *)
-(*           P1 fp mp2 -> *)
-(*           P2 (clear_footprint_rec fp) sb sofs mp3 -> *)
-(*           massert_imp mp1 (range tb tofs (tofs + sizeof_footprint ce fp)) -> *)
-(*           massert_imp (mp1 ** MP) mp3 -> *)
-(*           m1 |= mp1 ** mp2 ** MP -> *)
-(*           (alignof_footprint ce fp | tofs) -> *)
-(*           Mem.loadbytes m1 sb sofs (sizeof_footprint ce fp) = Some bytes -> *)
-(*           Mem.storebytes m1 tb tofs bytes = Some m2 -> *)
-(*           fields_fp_well_formed ce fp -> *)
-(*           exists mass3 : massert, P2 fp tb tofs mass3 /\ m2 |= mass3 ** MP) *)
-(*     (SEMWTFP: fields_fp_sep P1 fpl mp2) *)
-(*     (SHALLOW: fields_loc_sep sb sofs P2 ((map (fun '(fid, (fofs, ffp)) => (fid, (fofs, clear_footprint_rec ffp))) fpl)) mp3) *)
-(*     (RANGE: massert_imp mp1 (range tb tofs (tofs + sz))) *)
-(*     (MPIMP: massert_imp (mp1 ** MP) mp3) *)
-(*     (MPRED : m1 |= mp1 ** mp2 ** MP) *)
-(*     (AL: (al | tofs)) *)
-(*     (LOAD: Mem.loadbytes m1 sb sofs sz = Some bytes) *)
-(*     (STORE: Mem.storebytes m1 tb tofs bytes = Some m2) *)
-(*     (WF: Forall (fp_field_in_range_aligned ce sz al *)
-(*                    (fields_fp_well_formed ce)) fpl), *)
-(*   exists (mass3 : massert),  *)
-(*       fields_loc_sep tb tofs P2 fpl mass3 /\ m2 |= mass3 ** MP. *)
+
+
+(* Storebytes: a store at a prefix range does not affect the contents
+   of the region stored by a later store at a disjoint suffix range,
+   so the two memories after storing only the suffix differ only at
+   the prefix. *)
+
+Lemma setN_get_in_range:
+  forall A (l: list A) p q (c: ZMap.t A) d,
+    p <= q < p + Z.of_nat (length l) ->
+    ZMap.get q (Mem.setN l p c) = nth (Z.to_nat (q - p)) l d.
+Proof.
+  induction l; intros; simpl in *.
+  - lia.
+  - destruct (Z.eq_dec p q).
+    + subst.
+      rewrite (Mem.setN_outside A l (ZMap.set q a c) (q + 1) q) by lia.
+      rewrite ZMap.gss.
+      rewrite Z.sub_diag. simpl. reflexivity.
+    + assert (Hp: p < q) by lia.
+      rewrite (IHl (p + 1) q (ZMap.set p a c) d); [|lia].
+      assert (HAR: q - (p + 1) = q - p - 1) by lia.
+      rewrite HAR.
+      replace (Z.to_nat (q - p)) with (Z.to_nat (Z.succ (q - p - 1))) by (f_equal; lia).
+      rewrite Z2Nat.inj_succ by lia.
+      simpl. reflexivity.
+Qed.
+
+Lemma storebytes_prefix_contents:
+  forall m1 m1p m2h m1' b ofs fofs bytesP bytesH1,
+    Z.of_nat (length bytesP) = fofs ->
+    Mem.storebytes m1 b ofs bytesP = Some m1p ->
+    Mem.storebytes m1 b (ofs + fofs) bytesH1 = Some m2h ->
+    Mem.storebytes m1p b (ofs + fofs) bytesH1 = Some m1' ->
+    NMap.get _ b (Mem.mem_contents m1') = Mem.setN bytesH1 (ofs + fofs) (Mem.setN bytesP ofs (NMap.get _ b (Mem.mem_contents m1)))
+    /\ NMap.get _ b (Mem.mem_contents m2h) = Mem.setN bytesH1 (ofs + fofs) (NMap.get _ b (Mem.mem_contents m1)).
+Proof.
+  intros m1 m1p m2h m1' b ofs fofs bytesP bytesH1 LENP STOREP STOREH STOREHP.
+  split.
+  - rewrite (Mem.storebytes_mem_contents m1p b (ofs + fofs) bytesH1 m1' STOREHP).
+    rewrite (Mem.storebytes_mem_contents m1 b ofs bytesP m1p STOREP).
+    rewrite NMap.gsspec. rewrite NMap.gsspec.
+    destruct (NMap.elt_eq b b) as [EQ | NE].
+    + reflexivity.
+    + exfalso; exact (NE eq_refl).
+  - rewrite (Mem.storebytes_mem_contents m1 b (ofs + fofs) bytesH1 m2h STOREH).
+    rewrite NMap.gsspec.
+    destruct (NMap.elt_eq b b) as [EQ | NE].
+    + reflexivity.
+    + exfalso; exact (NE eq_refl).
+Qed.
+
+(* [storebytes_prefix_unchanged] *)
+Lemma storebytes_prefix_unchanged:
+  forall m1 m1p m2h m1' b ofs fofs bytesP bytesH1,
+    Z.of_nat (length bytesP) = fofs ->
+    Mem.storebytes m1 b ofs bytesP = Some m1p ->
+    Mem.storebytes m1 b (ofs + fofs) bytesH1 = Some m2h ->
+    Mem.storebytes m1p b (ofs + fofs) bytesH1 = Some m1' ->
+    forall P: block -> Z -> Prop, (forall b0 ofs0, P b0 ofs0 -> ~ (b0 = b /\ ofs <= ofs0 < ofs + fofs)) ->
+    Mem.unchanged_on P m2h m1'.
+Proof.
+  intros m1 m1p m2h m1' b ofs fofs bytesP bytesH1 LENP STOREP STOREH STOREHP P PFORBID.
+  constructor.
+  - (* support *)
+    intros b0 SUPPORT.
+    rewrite (Mem.support_storebytes m1 b (ofs + fofs) bytesH1 m2h STOREH) in SUPPORT.
+    rewrite (Mem.support_storebytes m1p b (ofs + fofs) bytesH1 m1' STOREHP).
+    rewrite (Mem.support_storebytes m1 b ofs bytesP m1p STOREP).
+    exact SUPPORT.
+  - (* perm *)
+    intros b0 ofs0 k p0 PB0 VALID. split; intro PERM.
+    + eapply Mem.perm_storebytes_1; [exact STOREHP |].
+      eapply Mem.perm_storebytes_1; [exact STOREP |].
+      eapply Mem.perm_storebytes_2; [exact STOREH | exact PERM].
+    + eapply Mem.perm_storebytes_1; [exact STOREH |].
+      eapply Mem.perm_storebytes_2; [exact STOREP |].
+      eapply Mem.perm_storebytes_2; [exact STOREHP | exact PERM].
+  - (* contents *)
+    intros b0 ofs0 PB0 READABLE.
+    destruct (peq b0 b) as [EQ | NEQ].
+    + subst b0.
+      destruct (storebytes_prefix_contents m1 m1p m2h m1' b ofs fofs bytesP bytesH1 LENP STOREP STOREH STOREHP) as [C1 C2].
+      rewrite C1. rewrite C2.
+      destruct (Z_lt_ge_dec ofs0 (ofs + fofs)) as [LTS | GES].
+      * assert (OFSS: ofs0 < ofs).
+        { destruct (Z_lt_ge_dec ofs0 ofs); [auto | exfalso].
+          apply (PFORBID b ofs0 PB0). split; auto. lia. }
+        rewrite (Mem.setN_outside memval bytesH1 _ (ofs + fofs) ofs0) by lia.
+        rewrite (Mem.setN_outside memval bytesH1 _ (ofs + fofs) ofs0) by lia.
+        rewrite (Mem.setN_outside memval bytesP _ ofs ofs0) by lia.
+        auto.
+      * destruct (Z_lt_ge_dec ofs0 (ofs + fofs + Z.of_nat (length bytesH1))) as [LT2 | GE2].
+        -- assert (RNGH: ofs + fofs <= ofs0 /\ ofs0 < ofs + fofs + Z.of_nat (length bytesH1)).
+           { split; [apply Z.ge_le; exact GES | exact LT2]. }
+           rewrite (setN_get_in_range memval bytesH1 (ofs + fofs) ofs0 _ Undef RNGH).
+           rewrite (setN_get_in_range memval bytesH1 (ofs + fofs) ofs0 _ Undef RNGH).
+           reflexivity.
+        -- rewrite (Mem.setN_outside memval bytesH1 _ (ofs + fofs) ofs0) by lia.
+           rewrite (Mem.setN_outside memval bytesH1 _ (ofs + fofs) ofs0) by lia.
+           rewrite (Mem.setN_outside memval bytesP _ ofs ofs0) by lia.
+           auto.
+    + (* b0 <> b *)
+      unfold NMap.get.
+      rewrite (Mem.storebytes_mem_contents m1p b (ofs + fofs) bytesH1 m1' STOREHP).
+      rewrite (Mem.storebytes_mem_contents m1 b ofs bytesP m1p STOREP).
+      rewrite (Mem.storebytes_mem_contents m1 b (ofs + fofs) bytesH1 m2h STOREH).
+      rewrite NMap.gso by auto.
+      rewrite NMap.gso by auto.
+      rewrite NMap.gso by auto.
+      reflexivity.
+Qed.
+
+Lemma field_noalign_offset_rec_base_nonneg:
+  forall ce fid ms pos base fofs,
+    field_noalign_offset_rec ce fid ms pos = OK (base, fofs) ->
+    0 <= pos ->
+    0 <= base.
+Proof.
+  induction ms as [| m ms IH]; intros; simpl in *.
+  - discriminate.
+  - destruct m as [id ty].
+    change (name_member (Member_plain id ty)) with id in *.
+    destruct (ident_eq fid id) eqn:ID.
+    + destruct (layout_field ce pos (Member_plain id ty)) eqn:L; try discriminate.
+      inv H. apply Z.div_pos; [exact H0 | lia].
+    + apply (IH (next_field ce pos (Member_plain id ty)) base fofs H).
+      apply Z.le_trans with pos; [exact H0 | apply (next_field_incr ce pos (Member_plain id ty))].
+Qed.
+
+Lemma field_noalign_offset_base_nonneg ce: forall fid ms base fofs,
+    field_noalign_offset ce fid ms = OK (base, fofs) ->
+    0 <= base.
+Proof.
+  unfold field_noalign_offset. intros. eapply field_noalign_offset_rec_base_nonneg; eauto. lia.
+Qed.
+
+
+(* The footprint of a well-typed [fields_loc_sep] is contained in the
+   region [ofs, ofs+sz), except that box fields may point to other
+   blocks. *)
+
+(* Lemma fields_loc_sep_footprint_bounded ce: forall fpl b ofs mass sz al, *)
+(*     fields_loc_sep b ofs (sem_wt_loc ce) fpl mass -> *)
+(*     Forall (fp_field_in_range_aligned ce sz al (fields_fp_well_formed ce)) fpl -> *)
+(*     (forall fid base fofs ffp, *)
+(*         In (fid, ((base, fofs), ffp)) fpl -> *)
+(*         0 <= sizeof_footprint ce ffp /\ *)
+(*         (forall b0 ofs0 m', *)
+(*            sem_wt_loc ce ffp b (ofs + fofs) m' -> *)
+(*            m_footprint m' b0 ofs0 -> *)
+(*            (b0 = b /\ ofs + fofs <= ofs0 < ofs + fofs + sizeof_footprint ce ffp) \/ b0 <> b)) -> *)
+(*     forall b0 ofs0, *)
+(*       m_footprint mass b0 ofs0 -> *)
+(*       (b0 = b /\ ofs <= ofs0 < ofs + sz) \/ b0 <> b. *)
 (* Proof. *)
+(*   intros fpl b ofs mass sz al FSEP FWF HFIELD. *)
+(*   induction FSEP; intros b0 ofs0 FOOT. *)
+(*   - (* nil *) *)
+(*     destruct EQV as [_ EQ2]. *)
+(*     destruct EQ2 as [_ FP]. *)
+(*     destruct (FP b0 ofs0 FOOT). *)
+(*   - (* cons *) *)
+(*     pose proof (Forall_inv FWF) as FWF0. pose proof (Forall_inv_tail FWF) as FWF1. *)
+(*     inv FWF0. *)
+(*     destruct (HFIELD fid base fofs ffp (or_introl eq_refl)) as [HSIZE0 HBOUND0]. *)
+(*     destruct EQV as [_ EQ2]. *)
+(*     destruct EQ2 as [_ FP]. *)
+(*     pose proof (FP b0 ofs0 FOOT) as FOOTX. *)
+(*     simpl in FOOTX. *)
+(*     destruct FOOTX as [FOOTP | [FOOT1 | FOOT2]]. *)
+(*     + (* padding *) *)
+(*       destruct FOOTP as [HEQ HRANGE]. subst b0. *)
+(*       left. split; [reflexivity | split; lia]. *)
+(*     + (* head field *) *)
+(*       destruct (HBOUND0 b0 ofs0 mass1 FWT FOOT1) as [BND | NEQ]. *)
+(*       * destruct BND as [HEQ2 HRANGE2]. subst b0. *)
+(*         left. split; [reflexivity | split; lia]. *)
+(*       * right. exact NEQ. *)
+(*     + (* tail *) *)
+(*       exact (IHFSEP FWF1 (fun fid0 base0 fofs0 ffp0 IN0 => HFIELD fid0 base0 fofs0 ffp0 (or_intror IN0)) b0 ofs0 FOOT2). *)
+(* Qed. *)
+
+(* The footprint of a well-typed location is contained in its region,
+   except that a box may point to (other) heap blocks. *)
+(* Lemma sem_wt_loc_footprint_bounded ce te: forall ty fp, *)
+(*     composite_env_consistent ce -> *)
+(*     (forall id co, ce ! id = Some co -> list_norepet (name_members (co_members co))) -> *)
+(*     wt_footprint ce te ty fp -> *)
+(*     fields_fp_well_formed ce fp -> *)
+(*     forall b ofs mass, *)
+(*       sem_wt_loc ce fp b ofs mass -> *)
+(*       forall b' ofs', *)
+(*         m_footprint mass b' ofs' -> *)
+(*         (b' = b /\ ofs <= ofs' < ofs + sizeof_footprint ce fp) \/ b' <> b. *)
+(* Proof. *)
+(*   intros ty fp CONS NOREP WTFP FPWF. revert ty WTFP FPWF. *)
+(*   induction fp as [| sz al | chunk v | b1 fp1 IHbox | id fpl IHfields | id tagz fid fofs fp1 IHenum | mut b2 ofs2 ph0 vs] using strong_footprint_ind; *)
+(*     intros ty WTFP FPWF b ofs mass WTLOC b' ofs' FOOT; inv WTLOC. *)
+(*   - (* fp_emp *) *)
+(*     destruct EQV as [EQV1 IMP]. destruct IMP as [IMPP FP]. simpl in FP. *)
+(*     destruct (FP b' ofs' FOOT). *)
+(*   - (* fp_uninit *) *)
+(*     destruct EQV as [EQV1 EQV2]. destruct EQV2 as [EQV2P FP]. *)
+(*     simpl in FP. *)
+(*     destruct (FP b' ofs' FOOT) as [INR | INSP]. *)
+(*     + simpl in INR. destruct INR as [EQ [LO HI]]. subst. left. split; [auto | simpl; lia]. *)
+(*     + unfold spure in INSP. simpl in INSP. contradiction. *)
+(*   - (* fp_scalar *) *)
+(*     destruct EQV as [EQV1 EQV2]. destruct EQV2 as [EQV2P FP]. *)
+(*     simpl in FP. *)
+(*     unfold hasvalue, contains in FP. cbn in FP. *)
+(*     destruct (FP b' ofs' FOOT) as [EQ [LO HI]]. subst. *)
+(*     left. split; [auto | simpl; lia]. *)
+(*   - (* fp_box *) *)
+(*     destruct EQV as [EQV1 EQV2]. destruct EQV2 as [EQV2P FP]. *)
+(*     simpl in FP. *)
+(*     destruct (FP b' ofs' FOOT) as [INH | INBOX]. *)
+(*     + unfold hasvalue, contains in INH. cbn in INH. *)
+(*       destruct INH as [EQ [LO HI]]. subst. *)
+(*       left. split; [auto | simpl; lia]. *)
+(*     + unfold box_pred in INBOX. *)
+(*       destruct INBOX as [INNEG | INNEXT]. *)
+(*       * unfold contains_neg in INNEG. simpl in INNEG. *)
+(*         destruct INNEG as [EQ _]. subst b'. right. (* exact NEQ. *) admit. *)
+(*       * right. (* exact (BOXFP b' ofs' INNEXT). *) admit. *)
+(*   - (* fp_struct *) *)
+(*     inv WTFP. *)
+(*     inv FPWF. *)
+(*     destruct EQV as [EQV1 EQV2]. destruct EQV2 as [EQV2P FP]. *)
+(*     simpl in FP. *)
+(*     destruct (FP b' ofs' FOOT) as [INMASS | [INPAD | INSP]]. *)
+(*     + (* fields *) *)
+(*       eapply fields_loc_sep_footprint_bounded with (sz := sizeof_comp ce id) (al := alignof_comp ce id); eauto. *)
+(*       { intros fid0 base0 fofs0 ffp0 IN0. split. *)
+(*         - destruct (fp_match_field_In_wt ce co (wt_footprint ce te) fpl (co_members co) fid0 base0 fofs0 ffp0 MATCH IN0) as [fty0 WTFP0]. *)
+(*           pose proof (wt_footprint_size_eq ce fty0 ffp0 te WTFP0) as SIZEEQ. *)
+(*           rewrite <- SIZEEQ. apply Z.ge_le. apply (sizeof_pos ce fty0). *)
+(*         - intros b0 ofs0 m' WTLOC0 FOOT0. *)
+(*           destruct (fp_match_field_In_wt ce co (wt_footprint ce te) fpl (co_members co) fid0 base0 fofs0 ffp0 MATCH IN0) as [fty0 WTFP0]. *)
+(*           assert (FWF0: fp_field_in_range_aligned ce (sizeof_comp ce id) (alignof_comp ce id) (fields_fp_well_formed ce) (fid0, ((base0, fofs0), ffp0))). *)
+(*           { apply (proj1 (Forall_forall (fp_field_in_range_aligned ce (sizeof_comp ce id) (alignof_comp ce id) (fields_fp_well_formed ce)) fpl)); [exact FWF | exact IN0]. } *)
+(*           inv FWF0. *)
+(*           exact (IHfields fid0 base0 fofs0 ffp0 IN0 fty0 WTFP0 R5 b (ofs + fofs0) m' WTLOC0 b0 ofs0 FOOT0). } *)
+(*     + (* trailing padding *) *)
+(*       subst. unfold range in INPAD. cbn in INPAD. *)
+(*       destruct INPAD as [EQ [LO HI]]. subst. *)
+(*       assert (SZC: 0 <= sizeof_struct_comp ce id). *)
+(*       { unfold sizeof_struct_comp. destruct (ce ! id) as [co0|]; [|lia]. *)
+(*         destruct (co_sv co0); simpl; [|lia]. *)
+(*         exact (sizeof_composite_pos ce Struct (co_members co0)). } *)
+(*       left. split; [auto | simpl; lia]. *)
+(*     + unfold spure in INSP. simpl in INSP. contradiction. *)
+(*   - (* fp_enum *) *)
+(*     inv WTFP. *)
+(*     inv FPWF. inv FWF. *)
+(*     pose proof (wt_footprint_size_eq ce fty fp1 te WT) as SIZEEQ. *)
+(*     assert (FPOS: 0 <= sizeof_footprint ce fp1). *)
+(*     { rewrite <- SIZEEQ. apply Z.ge_le. apply (sizeof_pos ce fty). } *)
+(*     destruct EQV as [EQV1 EQV2]. destruct EQV2 as [EQV2P FP]. *)
+(*     simpl in FP. *)
+(*     destruct (FP b' ofs' FOOT) as [INM1 | [INPAD | [INM2 | [INTAIL | INSP]]]]. *)
+(*     + (* tag *) *)
+(*       subst. unfold hasvalue, contains in INM1. cbn in INM1. *)
+(*       destruct INM1 as [EQ [LO HI]]. subst. *)
+(*       left. split; [auto |]. *)
+(*       assert (SZM: size_chunk Mint32 = 4) by reflexivity. *)
+(*       assert (LE4: size_chunk Mint32 <= sizeof_comp ce id). *)
+(*       { rewrite SZM. lia. } *)
+(*       simpl. lia. *)
+(*     + (* padmp *) *)
+(*       subst. unfold range in INPAD. cbn in INPAD. *)
+(*       destruct INPAD as [EQ [LO HI]]. subst. *)
+(*       left. split; [auto | simpl; lia]. *)
+(*     + (* variant field *) *)
+(*       destruct (IHenum fty WT R5 b (ofs + fofs) mass2 FWT b' ofs' INM2) as [BND | NEQ]. *)
+(*       * left. destruct BND as [EQ [LO HI]]. subst. split; [auto | simpl; lia]. *)
+(*       * right. exact NEQ. *)
+(*     + (* tailpad *) *)
+(*       subst. unfold range in INTAIL. cbn in INTAIL. *)
+(*       destruct INTAIL as [EQ [LO HI]]. subst. *)
+(*       left. split; [auto | simpl; lia]. *)
+(*     + unfold spure in INSP. simpl in INSP. contradiction. *)
+(*   - (* fp_ref *) *)
+(*     destruct EQV as [EQV1 EQV2]. destruct EQV2 as [EQV2P FP]. *)
+(*     simpl in FP. *)
+(*     unfold hasvalue, contains in FP. cbn in FP. *)
+(*     destruct (FP b' ofs' FOOT) as [EQ [LO HI]]. subst. *)
+(*     left. split; [auto | simpl; lia]. *)
+(* (* Qed. *) *)
 (* Admitted. *)
 
-Lemma storebytes_sem_wt_loc ce: forall sfp tb tofs sb sofs mp1 mp2 MP m1 m2 bytes ty te
+(* Given a well-typed struct footprint [fpl], storing the struct bytes
+   into the target location makes each field of the target location
+   semantically well-typed.  We split the source bytes and the target
+   stores field by field and apply [storebytes_sem_wt_loc] to each
+   field. *)
+
+
+
+(* Re-base a [fields_loc_sep] derivation by shifting the base offset
+   by [d]; the field offsets in the list are shifted by [-d] so that
+   the absolute locations of the fields stay the same. *)
+Definition shift_ffp (d : Z) (x : ffpty) : ffpty :=
+  match x with
+  | (fid, ((base, fofs), ffp)) => (fid, ((base - d, fofs - d), ffp))
+  end.
+
+Lemma fields_loc_sep_shift: forall b ofs P d fpl mass,
+    fields_loc_sep b ofs P fpl mass ->
+    fields_loc_sep b (ofs + d) P (map (shift_ffp d) fpl) mass.
+Proof.
+  intros b ofs P d fpl mass F.
+  induction F as [mp EQV | fid base fofs ffp l mass1 mass2 padmp mp IND IHF WT1 ALPERM EQV].
+  - simpl. econstructor. exact EQV.
+  - simpl.
+    apply (fields_loc_sep_cons b (ofs + d) P fid (base - d) (fofs - d) ffp
+                               (map (shift_ffp d) l) mass1 mass2 padmp mp);
+    [ exact IHF
+    | replace (ofs + d + (fofs - d)) with (ofs + fofs) by lia; exact WT1
+    | rewrite ALPERM; f_equal; lia
+    | exact EQV ].
+Qed.
+
+
+(* The per-field absolute alignment predicate is invariant under the
+   [shift_ffp d] re-basing, provided the target base is shifted by [d]. *)
+Lemma Forall_align_shift: forall ce tofs d fpl,
+    Forall (fun '(fid, ((base, fofs), ffp)) => (alignof_footprint ce ffp | tofs + fofs)) fpl ->
+    Forall (fun '(fid, ((base, fofs), ffp)) => (alignof_footprint ce ffp | (tofs + d) + fofs))
+           (map (shift_ffp d) fpl).
+Proof.
+  intros ce tofs d fpl. induction fpl as [| a l IH]; intros H.
+  - simpl. econstructor.
+  - simpl. inv H.
+    destruct a as [fid [[base fofs] ffp]].
+    simpl in *.
+    econstructor.
+    + replace ((tofs + d) + (fofs - d)) with (tofs + fofs) by lia. exact H2.
+    + apply IH. exact H3.
+Qed.
+
+Lemma Forall_range_shift ce: forall sz d f fpl,
+    Forall (fun '(fid', ((base', fofs'), ffp')) => d <= fofs') fpl ->
+    Forall (fp_field_in_range ce sz f) fpl ->
+    Forall (fp_field_in_range ce (sz - d) f) (map (shift_ffp d) fpl).
+Proof.
+  intros sz d f fpl. revert f. induction fpl as [| a l IH]; intros f HEAD WF.
+  - simpl. constructor.
+  - destruct a as [fid [[base fofs] ffp]].
+    simpl in *.
+    inversion HEAD as [| ? ? HHEAD HTAIL]; subst.
+    inversion WF as [| ? ? WFHEAD WFTAIL]; subst.
+    inversion WFHEAD as [fid0 base0 fofs0 ffp0 R1 R2 R3 R5]; subst.
+    constructor.
+    + apply fp_field_in_range_intro.
+      * lia.
+      * lia.
+      * lia.
+      * exact R5.
+    + exact (IH f HTAIL WFTAIL).
+Qed.
+
+Lemma Forall_wtfootprint_shift ce: forall te d fpl,
+    Forall (fun '(fid, ((base, fofs), ffp)) => exists ty, wt_footprint ce te ty ffp) fpl ->
+    Forall (fun '(fid, ((base, fofs), ffp)) => exists ty, wt_footprint ce te ty ffp)
+           (map (shift_ffp d) fpl).
+Proof.
+  intros te d fpl. induction fpl as [| a l IH]; intros H.
+  - simpl. constructor.
+  - destruct a as [fid [[base fofs] ffp]].
+    simpl in *.
+    inversion H as [| ? ? HHEAD HTAIL]; subst.
+    constructor; [exact HHEAD | exact (IH HTAIL)].
+Qed.
+
+Lemma shift_ffp_involutive: forall d l,
+    map (shift_ffp (- d)) (map (shift_ffp d) l) = l.
+Proof.
+  intros d l. induction l as [| a l IH]; simpl; auto.
+  rewrite IH. destruct a as [fid [[base fofs] ffp]]. simpl. repeat f_equal; lia.
+Qed.
+
+Lemma in_map_shift_ffp_inv: forall d l fid base fofs ffp,
+    In (fid, ((base, fofs), ffp)) (map (shift_ffp d) l) ->
+    In (fid, ((base + d, fofs + d), ffp)) l.
+Proof.
+  intros d l fid base fofs ffp H.
+  apply in_map_iff in H as [y [INY EQ]].
+  destruct y as [fidy [[basey fofsy] ffpy]].
+  simpl in INY.
+  injection INY as Hfid Hbase.
+  subst fidy.
+  subst ffpy.
+  assert (Hb : basey = base + d) by lia.
+  assert (Hf : fofsy = fofs + d) by lia.
+  rewrite <- Hb, <- Hf. exact EQ.
+Qed.
+
+Lemma range_split_imp: forall b lo mid hi P,
+    lo <= mid <= hi ->
+    massert_imp (range b lo hi ** P) (range b lo mid ** range b mid hi ** P).
+Proof.
+  intros b lo mid hi P H. split.
+  - intros m MPRED. eapply range_split; [exact H | exact MPRED].
+  - intros b0 ofs0 FOOT. simpl in FOOT.
+    destruct FOOT as [F1 | [F2 | FP]].
+    + simpl in F1. destruct F1 as [EQ [LO' HI']]. subst. left. simpl. split; [reflexivity | lia].
+    + simpl in F2. destruct F2 as [EQ [LO' HI']]. subst. left. simpl. split; [reflexivity | lia].
+    + right. exact FP.
+Qed.
+
+Lemma fields_after_d_le ce: forall d l,
+    fields_after ce d l ->
+    Forall (fun '(fid', ((base', fofs'), ffp')) => d <= fofs') l.
+Proof.
+  intros d l. revert d.
+  induction l as [| a l IHl]; intros d H.
+  - constructor.
+  - destruct a as [fid [[base fofs] ffp]].
+    inversion H as [| fid0 base0 fofs0 ffp0 l0 HBASE HLE HSIZE HA]; subst.
+    constructor; [exact HLE |].
+    apply Forall_forall. intros x IN.
+    pose proof (IHl (fofs + sizeof_footprint ce ffp) HA) as IHT.
+    apply (proj1 (Forall_forall (fun '(fid', ((base', fofs'), ffp')) => fofs + sizeof_footprint ce ffp <= fofs') l) IHT) in IN.
+    destruct x as [fid' [[base' fofs'] ffp']]. simpl in IN. lia.
+Qed.
+
+Lemma fields_after_shift ce: forall d d' l,
+    fields_after ce d l ->
+    fields_after ce (d - d') (map (shift_ffp d') l).
+Proof.
+  intros d d' l. revert d d'.
+  induction l as [| a l IHl]; intros d d' H.
+  - simpl. constructor.
+  - destruct a as [fid [[base fofs] ffp]].
+    inversion H as [| fid0 base0 fofs0 ffp0 l0 HBASE HLE HSIZE HA]; subst.
+    simpl. constructor.
+    + lia.
+    + lia.
+    + exact HSIZE.
+    + assert (HEQ : (fofs - d') + sizeof_footprint ce ffp = (fofs + sizeof_footprint ce ffp) - d') by lia.
+      rewrite HEQ. exact (IHl (fofs + sizeof_footprint ce ffp) d' HA).
+Qed.
+
+
+(* [storebytes_fields_loc_sep]: storing the bytes of a well-typed field
+   list [fpl] into a target location makes that target location
+   semantically well-typed, field by field.
+
+   Concretely, suppose the source location [sem_wt_loc]-describes [fpl]
+   at [(sb, sofs)] with assertion [mass], and we load [sz] bytes from
+   the source, then store those same bytes at [(tb, tofs)] using the
+   target permission [mp2] (which covers [tofs, tofs + sz)).  Given
+   that the field list is range-bounded ([WF]), sorted ([SORTED]), and
+   absolutely aligned at [tofs] ([ABS_ALIGN]), the conclusion produces a
+   [fields_loc_sep] for [fpl] at [(tb, tofs)] whose assertion holds in
+   the resulting memory [m2] together with the frame [MP].
+
+   The proof is by well-founded induction on [length fpl].  The nil case
+   is immediate.  In the cons case we split the loaded bytes into the
+   padding before the head field, the head field bytes, and the tail
+   bytes; the per-field IH [IH] turns the head field bytes into a
+   [sem_wt_loc] for [ffp] at [tofs + fofs].  We then shift the tail
+   field list by [d := fofs + sizeof_footprint ce ffp] with [shift_ffp],
+   which keeps the absolute field locations unchanged, and recurse on
+   [map (shift_ffp d) l] using the tail's [SORTED]/[WF]/[ABS_ALIGN]
+   invariants.  Finally we re-base the recursive [fields_loc_sep] back
+   to [tofs] and reassemble the whole field list with
+   [fields_loc_sep_cons]. *)
+Lemma storebytes_fields_loc_sep ce: forall fpl tb tofs sb sofs mass mp2 MP m1_src m1 m2 bytes te sz
+    (CONS: composite_env_consistent ce)
+    (NOREP: forall id co, ce ! id = Some co -> list_norepet (name_members (co_members co)))
+    (IH: forall fid base fofs ffp,
+        In (fid, ((base, fofs), ffp)) fpl ->
+        forall tb tofs sb sofs mp1 mp2 MP m1_src m1 m2 bytes ty te,
+        sem_wt_loc ce ffp sb sofs mp1 ->
+        massert_imp mp2 (range tb tofs (tofs + sizeof_footprint ce ffp)) ->
+        (alignof_footprint ce ffp | tofs) ->
+        m1_src |= mp1 ->
+        m1 |= mp2 ** MP ->
+        Mem.loadbytes m1_src sb sofs (sizeof_footprint ce ffp) = Some bytes ->
+        Mem.storebytes m1 tb tofs bytes = Some m2 ->
+        wt_footprint ce te ty ffp ->
+        exists mass3, sem_wt_loc ce ffp tb tofs mass3 /\ m2 |= mass3 ** MP)
+    (FWT: fields_loc_sep sb sofs (sem_wt_loc ce) fpl mass)
+    (SORTED: fields_sorted ce fpl)
+    (RANGE: massert_imp mp2 (range tb tofs (tofs + sz)))
+    (SZPOS: 0 <= sz)
+    (MPRED_SRC: m1_src |= mass)
+    (MPRED: m1 |= mp2 ** MP)
+    (LOAD: Mem.loadbytes m1_src sb sofs sz = Some bytes)
+    (STORE: Mem.storebytes m1 tb tofs bytes = Some m2)
+    (WF: Forall (fp_field_in_range ce sz (fields_fp_well_formed ce)) fpl)
+    (WTFPS: Forall (fun '(fid, ((base, fofs), ffp)) => exists ty, wt_footprint ce te ty ffp) fpl)
+    (ABS_ALIGN: Forall (fun '(fid, ((base, fofs), ffp)) => (alignof_footprint ce ffp | (tofs + fofs))) fpl),
+  exists mass3, fields_loc_sep tb tofs (sem_wt_loc ce) fpl mass3 /\ m2 |= mass3 ** MP.
+Proof.
+  intros.
+  cut (forall n fpl, length fpl = n -> forall tb tofs sb sofs mass mp2 MP m1_src m1 m2 bytes te sz,
+      (forall fid base fofs ffp, In (fid, ((base, fofs), ffp)) fpl -> forall tb tofs sb sofs mp1 mp2 MP m1_src m1 m2 bytes ty te, sem_wt_loc ce ffp sb sofs mp1 -> massert_imp mp2 (range tb tofs (tofs + sizeof_footprint ce ffp)) -> (alignof_footprint ce ffp | tofs) -> m1_src |= mp1 -> m1 |= mp2 ** MP -> Mem.loadbytes m1_src sb sofs (sizeof_footprint ce ffp) = Some bytes -> Mem.storebytes m1 tb tofs bytes = Some m2 -> wt_footprint ce te ty ffp -> exists mass3, sem_wt_loc ce ffp tb tofs mass3 /\ m2 |= mass3 ** MP) ->
+      fields_sorted ce fpl ->
+      massert_imp mp2 (range tb tofs (tofs + sz)) ->
+      0 <= sz ->
+      m1_src |= mass ->
+      m1 |= mp2 ** MP ->
+      Mem.loadbytes m1_src sb sofs sz = Some bytes ->
+      Mem.storebytes m1 tb tofs bytes = Some m2 ->
+      Forall (fp_field_in_range ce sz (fields_fp_well_formed ce)) fpl ->
+      Forall (fun '(fid, ((base, fofs), ffp)) => exists ty, wt_footprint ce te ty ffp) fpl ->
+      Forall (fun '(fid, ((base, fofs), ffp)) => (alignof_footprint ce ffp | (tofs + fofs))) fpl ->
+      fields_loc_sep sb sofs (sem_wt_loc ce) fpl mass ->
+      exists mass3, fields_loc_sep tb tofs (sem_wt_loc ce) fpl mass3 /\ m2 |= mass3 ** MP).
+  { intros H. apply (H (length fpl) fpl eq_refl tb tofs sb sofs mass mp2 MP m1_src m1 m2 bytes te sz IH SORTED RANGE SZPOS MPRED_SRC MPRED LOAD STORE WF WTFPS ABS_ALIGN FWT). }
+  clear - CONS NOREP.
+  induction n as [n IHn] using (well_founded_induction lt_wf).
+  intros fpl HLEN tb tofs sb sofs mass mp2 MP m1_src m1 m2 bytes te sz IH SORTED RANGE SZPOS MPRED_SRC MPRED LOAD STORE WF WTFPS ABS_ALIGN FWT.
+  destruct fpl as [| a l].
+  - (* nil case *)
+    exists STrue.
+    split; [econstructor; reflexivity |].
+    destruct RANGE as [RANGE_P RANGE_F].
+    pose proof (RANGE_P m1 (proj1 MPRED)) as RANGE_M1. unfold range in RANGE_M1. simpl in RANGE_M1.
+    destruct RANGE_M1 as [RP SZLE].
+    assert (LEN_EQ: Z.of_nat (length bytes) = sz).
+    { exploit Mem.loadbytes_length; eauto. intros LEN. rewrite LEN.
+      apply Z2Nat.id. exact SZPOS. }
+    assert (MPRED_MP: m1 |= MP).
+    { eapply massert_imp_proj2. exact MPRED. }
+    assert (MPRED_MP2: m2 |= MP).
+    { eapply (m_invar MP). exact MPRED_MP.
+      eapply Mem.storebytes_unchanged_on; eauto.
+      intros i IN. intro HF.
+      destruct MPRED as [MP2PRED [MPPRED DISJ]].
+      apply (DISJ tb i).
+      - apply (RANGE_F tb i). simpl. split; [reflexivity | split].
+        + exact (proj1 IN).
+        + rewrite <- LEN_EQ. exact (proj2 IN).
+      - exact HF. }
+    rewrite <- (massert_eqv_STrue_l MP). exact MPRED_MP2.
+  - (* cons case *)
+    destruct a as [fid [[base fofs] ffp]].
+    inversion FWT as [ | fid0 base0 fofs0 ffp0 l0 mass1 mass2 padmp0 mp0 IND FWT0 ALPERM EQV]; subst.
+    pose (SIZE := sizeof_footprint ce ffp).
+    pose (d := fofs + SIZE).
+    inversion SORTED as [ | fid0 base0 fofs0 ffp0 l0 HBASE HLE HSIZE HEAD_AFTER]; subst.
+    inversion WF as [| xwf lwf WFHEAD WFTAIL]; subst.
+    inversion WFHEAD as [fidwf basewf fofswf ffpwf R1 R2 R3 R5]; subst.
+    inversion WTFPS as [| xwt lwt WTHEAD WTTAIL]; subst.
+    simpl in WTHEAD. destruct WTHEAD as [fty WTFP0].
+    inversion ABS_ALIGN as [| xab lab ALHEAD ALTAIL]; subst.
+    simpl in ALHEAD.
+    assert (LEN_EQ: Z.of_nat (length bytes) = sz).
+    { exploit Mem.loadbytes_length; eauto. intros LEN. rewrite LEN.
+      apply Z2Nat.id. exact SZPOS. }
+    pose proof (wt_footprint_size_eq ce fty ffp te WTFP0) as SIZEEQ.
+    assert (SIZE_POS: 0 <= SIZE).
+    { unfold SIZE. rewrite <- SIZEEQ. apply Z.ge_le. apply (sizeof_pos ce fty). }
+    (* split the source loadbytes into padding / head field / tail *)
+    assert (LOAD_EQ: Mem.loadbytes m1_src sb sofs (d + (sz - d)) = Some bytes).
+    { replace (d + (sz - d)) with sz by lia. exact LOAD. }
+    exploit (Mem.loadbytes_split m1_src sb sofs d (sz - d) bytes LOAD_EQ); [lia | lia |].
+    intros (bytesA & bytesT & LOAD_A & LOAD_T & B_EQA).
+    exploit (Mem.loadbytes_split m1_src sb sofs fofs SIZE bytesA LOAD_A); [lia | lia |].
+    intros (bytesP & bytesH1 & LOAD_P & LOAD_H & B_EQP).
+    assert (LENP: Z.of_nat (length bytesP) = fofs).
+    { pose proof (Mem.loadbytes_length m1_src sb sofs fofs bytesP LOAD_P) as LEN.
+      rewrite LEN. apply Z2Nat.id. lia. }
+    assert (LENH: Z.of_nat (length bytesH1) = SIZE).
+    { pose proof (Mem.loadbytes_length m1_src sb (sofs + fofs) SIZE bytesH1 LOAD_H) as LEN.
+      rewrite LEN. apply Z2Nat.id. lia. }
+    assert (B_EQ: bytes = bytesP ++ bytesH1 ++ bytesT).
+    { rewrite B_EQA, B_EQP. rewrite app_assoc. reflexivity. }
+    exploit (Mem.storebytes_split m1 tb tofs bytesP (bytesH1 ++ bytesT) m2).
+    { rewrite <- B_EQ. exact STORE. }
+    intros (m1p & STORE_P & STORE_HT).
+    rewrite LENP in STORE_HT.
+    exploit (Mem.storebytes_split m1p tb (tofs + fofs) bytesH1 bytesT m2).
+    { exact STORE_HT. }
+    intros (m1' & STORE_H & STORE_T).
+    rewrite LENH in STORE_T.
+    replace (tofs + fofs + SIZE) with (tofs + d) in STORE_T by (unfold d; lia).
+    (* source field predicate *)
+    assert (MPRED_SRC_HEAD: m1_src |= mass1).
+    { rewrite EQV in MPRED_SRC.
+      rewrite Z.add_0_r in MPRED_SRC.
+      apply (massert_imp_proj1 mass1 mass2).
+      apply (massert_imp_proj2 (range sb sofs (sofs + fofs)) (mass1 ** mass2)).
+      exact MPRED_SRC. }
+    (* target permission for the head field *)
+    assert (MPRED_RANGE0: m1 |= range tb tofs (tofs + sz) ** MP).
+    { eapply sep_imp; [exact MPRED | exact RANGE | apply massert_imp_refl]. }
+    assert (MPRED_RANGE1: m1 |= range tb tofs (tofs + fofs) ** range tb (tofs + fofs) (tofs + sz) ** MP).
+    { eapply range_split; [lia | exact MPRED_RANGE0]. }
+    assert (MPRED_RANGE2: m1 |= range tb tofs (tofs + fofs) ** range tb (tofs + fofs) (tofs + d) ** range tb (tofs + d) (tofs + sz) ** MP).
+    { eapply sep_imp; [exact MPRED_RANGE1 | apply massert_imp_refl |].
+      apply (range_split_imp tb (tofs + fofs) (tofs + d) (tofs + sz) MP). unfold d, SIZE in *. lia. }
+    assert (MP_DISJ_RANGE: forall i, tofs <= i < tofs + sz -> ~ m_footprint MP tb i).
+    { intros i IN. intro HF.
+      destruct MPRED as [MP2PRED [MPPRED DISJ]].
+      destruct RANGE as [RANGE_P RANGE_F].
+      apply (DISJ tb i).
+      - apply (RANGE_F tb i). simpl. split; [reflexivity | exact IN].
+      - exact HF. }
+    set (FRAME := range tb (tofs + d) (tofs + sz) ** MP).
+    assert (MPRED_HEAD: m1 |= range tb (tofs + fofs) (tofs + d) ** (range tb tofs (tofs + fofs) ** FRAME)).
+    { unfold FRAME.
+      rewrite <- (sep_swap (range tb tofs (tofs + fofs)) (range tb (tofs + fofs) (tofs + d))
+                       (range tb (tofs + d) (tofs + sz) ** MP)).
+      exact MPRED_RANGE2. }
+    assert (STORE_H_FROM_M1: exists m2h, Mem.storebytes m1 tb (tofs + fofs) bytesH1 = Some m2h).
+    { edestruct (Mem.range_perm_storebytes m1 tb (tofs + fofs) bytesH1) as [m2h STOREH].
+      - red. intros i IN.
+        destruct MPRED_HEAD as [MPRED_HEAD_R _].
+        eapply Mem.perm_implies.
+        * eapply MPRED_HEAD_R. simpl. split; [lia |]. rewrite LENH in IN. unfold d, SIZE in *. lia.
+        * constructor.
+      - eexists. exact STOREH. }
+    destruct STORE_H_FROM_M1 as [m2h STOREH].
+    assert (FIELD: exists massA, sem_wt_loc ce ffp tb (tofs + fofs) massA /\                m2h |= massA ** (range tb tofs (tofs + fofs) ** FRAME)).
+    { eapply (IH fid 0 fofs ffp (or_introl eq_refl)).
+      - exact FWT0.
+      - apply (range_impl tb (tofs + fofs) (tofs + d) (tofs + fofs) (tofs + fofs + SIZE)); [lia | unfold d, SIZE in *; lia].
+      - exact ALHEAD.
+      - exact MPRED_SRC_HEAD.
+      - exact MPRED_HEAD.
+      - exact LOAD_H.
+      - exact STOREH.
+      - exact WTFP0. }
+    destruct FIELD as [massA WTLOCA_MPREDA]; destruct WTLOCA_MPREDA as [WTLOCA MPREDA].
+    assert (MPREDA_M1: m1' |= massA).
+    { apply (m_invar massA) with (m := m2h) (m' := m1').
+      - exact (sep_proj1 _ _ _ MPREDA).
+      - eapply (storebytes_prefix_unchanged m1 m1p m2h m1' tb tofs fofs bytesP bytesH1 LENP STORE_P STOREH STORE_H (m_footprint massA)).
+        intros b0 ofs0 FOOT. intro HCONTR. 
+        eapply MPREDA. eauto. simpl. left. auto. }
+    destruct MPREDA as [_ [_ DISJ_MASSA_FRAME]].
+    (* tail recursion setup *)
+    assert (IND_SHIFT: fields_loc_sep sb (sofs + d) (sem_wt_loc ce) (map (shift_ffp d) l) mass2).
+    { apply (fields_loc_sep_shift sb sofs (sem_wt_loc ce) d l mass2). exact IND. }
+    assert (HEAD_AFTER_DLE: Forall (fun '(fid', ((base', fofs'), ffp')) => d <= fofs') l).
+    { exact (fields_after_d_le ce d l HEAD_AFTER). }
+    assert (WF_TAIL: Forall (fp_field_in_range ce (sz - d) (fields_fp_well_formed ce)) (map (shift_ffp d) l)).
+    { exact (Forall_range_shift ce sz d (fields_fp_well_formed ce) l HEAD_AFTER_DLE WFTAIL). }
+    assert (ABS_ALIGN_TAIL: Forall (fun '(fid, ((base, fofs), ffp)) => (alignof_footprint ce ffp | ((tofs + d) + fofs))) (map (shift_ffp d) l)).
+    { exact (Forall_align_shift ce tofs d l ALTAIL). }
+    assert (WTFPS_TAIL: Forall (fun '(fid, ((base, fofs), ffp)) => exists ty, wt_footprint ce te ty ffp) (map (shift_ffp d) l)).
+    { exact (Forall_wtfootprint_shift ce te d l WTTAIL). }
+    assert (SORTED_TAIL: fields_sorted ce (map (shift_ffp d) l)).
+    { unfold fields_sorted. replace 0 with (d - d) by lia.
+      exact (fields_after_shift ce d d l HEAD_AFTER). }
+    assert (MPRED_SRC_TAIL: m1_src |= mass2).
+    { rewrite EQV in MPRED_SRC.
+      rewrite Z.add_0_r in MPRED_SRC.
+      rewrite <- sep_assoc in MPRED_SRC.
+      apply (massert_imp_proj2 (range sb sofs (sofs + fofs) ** mass1) mass2).
+      exact MPRED_SRC. }
+    (* target permission for the tail *)
+    assert (MPRED_RANGE_DROP: m1 |= range tb tofs (tofs + fofs) ** range tb (tofs + d) (tofs + sz) ** MP).
+    { eapply sep_imp; [exact MPRED_RANGE2 | apply massert_imp_refl | apply massert_imp_proj2]. }
+    assert (MPRED_RANGE_DROP_M1P: m1p |= range tb tofs (tofs + fofs) ** (range tb (tofs + d) (tofs + sz) ** MP)).
+    { eapply sep_preserved. exact MPRED_RANGE_DROP.
+      - intros H. eapply storebytes_range_unchanged; eauto.
+      - intros H. eapply (m_invar (range tb (tofs + d) (tofs + sz) ** MP)). exact H.
+        eapply Mem.storebytes_unchanged_on; eauto.
+        intros i INP. intro HF.
+        destruct MPRED_RANGE_DROP as [MPRED_PAD [MPRED_TAILMP DISJ]].
+        exact (DISJ tb i ltac:(simpl; split; [reflexivity |]; rewrite <- LENP; exact INP) HF). }
+    assert (MPRED_RANGE_DROP_M1': m1' |= range tb tofs (tofs + fofs) ** (range tb (tofs + d) (tofs + sz) ** MP)).
+    { eapply sep_preserved. exact MPRED_RANGE_DROP_M1P.
+      - intros H. eapply (m_invar (range tb tofs (tofs + fofs))). exact H.
+        eapply Mem.storebytes_unchanged_on; eauto.
+        intros i INP. intro HF.
+        simpl in HF. destruct HF as [HEQ HRANGE]. lia.
+      - intros H. eapply (m_invar (range tb (tofs + d) (tofs + sz) ** MP)). exact H.
+        eapply Mem.storebytes_unchanged_on; eauto.
+        intros i INP. intro HF.
+        destruct HF as [HFT | HFMP].
+        + rewrite LENH in INP. unfold d, SIZE in *. simpl in HFT. destruct HFT as [HEQ HRANGE]. lia.
+        + exact (MP_DISJ_RANGE i ltac:(rewrite LENH in INP; unfold d, SIZE in *; lia) HFMP). }
+    assert (MPRED_MASSA_FRAME: m1' |= massA ** (range tb tofs (tofs + fofs) ** range tb (tofs + d) (tofs + sz) ** MP)).
+    { change (m_pred massA m1' /\ m_pred (range tb tofs (tofs + fofs) ** range tb (tofs + d) (tofs + sz) ** MP) m1' /\ disjoint_footprint massA (range tb tofs (tofs + fofs) ** range tb (tofs + d) (tofs + sz) ** MP)).
+      split.
+      - exact MPREDA_M1.
+      - split.
+        * exact MPRED_RANGE_DROP_M1'.
+        * exact DISJ_MASSA_FRAME. }
+    assert (MPRED_TAIL: m1' |= range tb (tofs + d) (tofs + sz) ** (range tb tofs (tofs + fofs) ** massA ** MP)).
+    { rewrite (sep_swap3 massA (range tb tofs (tofs + fofs)) (range tb (tofs + d) (tofs + sz)) MP) in MPRED_MASSA_FRAME.
+      exact MPRED_MASSA_FRAME. }
+    assert (SZPOS_TAIL: 0 <= sz - d). { unfold d, SIZE in *. lia. }
+    pose (IH_l := fun (fid0: ident) (base0 fofs0: Z) (ffp0: footprint)
+                      (IN0: In (fid0, ((base0, fofs0), ffp0)) (map (shift_ffp d) l)) =>
+                    IH fid0 (base0 + d) (fofs0 + d) ffp0
+                       (or_intror (in_map_shift_ffp_inv d l fid0 base0 fofs0 ffp0 IN0))).
+    assert (TAIL: exists mass3_tail, fields_loc_sep tb (tofs + d) (sem_wt_loc ce) (map (shift_ffp d) l) mass3_tail
+                    /\ m2 |= mass3_tail ** (range tb tofs (tofs + fofs) ** massA ** MP)).
+    { apply (IHn (length l) (Nat.lt_succ_diag_r (length l)) (map (shift_ffp d) l) (map_length (shift_ffp d) l) tb (tofs + d) sb (sofs + d) mass2 (range tb (tofs + d) (tofs + sz)) (range tb tofs (tofs + fofs) ** massA ** MP) m1_src m1' m2 bytesT te (sz - d) IH_l SORTED_TAIL (range_impl tb (tofs + d) (tofs + sz) (tofs + d) ((tofs + d) + (sz - d)) ltac:(lia) ltac:(lia)) SZPOS_TAIL MPRED_SRC_TAIL MPRED_TAIL LOAD_T STORE_T WF_TAIL WTFPS_TAIL ABS_ALIGN_TAIL IND_SHIFT). }
+    destruct TAIL as [mass3_tail WTLOC_TAIL_MPRED]; destruct WTLOC_TAIL_MPRED as [WTLOC_TAIL MPRED_TAIL2].
+    assert (WTLOC_TAIL0: fields_loc_sep tb tofs (sem_wt_loc ce) l mass3_tail).
+    { rewrite <- (shift_ffp_involutive d l).
+      replace tofs with (tofs + d - d) by lia.
+      apply (fields_loc_sep_shift tb (tofs + d) (sem_wt_loc ce) (- d) (map (shift_ffp d) l) mass3_tail).
+      exact WTLOC_TAIL. }
+    exists (range tb tofs (tofs + fofs) ** massA ** mass3_tail).
+    split; [ apply (fields_loc_sep_cons tb tofs (sem_wt_loc ce) fid 0 fofs ffp l massA mass3_tail (range tb tofs (tofs + fofs)) (range tb tofs (tofs + fofs) ** massA ** mass3_tail) WTLOC_TAIL0 WTLOCA); [rewrite Z.add_0_r; reflexivity | apply massert_eqv_refl]
+            | rewrite sep_assoc; rewrite sep_assoc; rewrite (sep_swap (range tb tofs (tofs + fofs)) massA (mass3_tail ** MP)); rewrite <- (sep_swap3 mass3_tail (range tb tofs (tofs + fofs)) massA MP); exact MPRED_TAIL2 ].
+Qed.
+
+Definition bytes_of_bits_local (n: Z) : Z := (n + 7) / 8.
+
+Definition size_from (ce: composite_env) (pos: Z) (ms: members) : Z :=
+  bytes_of_bits_local (bitsizeof_struct ce pos ms).
+
+Lemma wt_footprint_align_divides ce:
+  forall ty fp fpm,
+    wt_footprint ce fpm ty fp ->
+    (alignof_footprint ce fp | alignof ce ty).
+Proof.
+  intros ty fp fpm H. inv H; simpl.
+  - apply Z.divide_refl.
+  - apply alignof_by_value; eauto.
+  - unfold alignof_comp. rewrite CO. apply Z.divide_refl.
+  - unfold alignof_comp. rewrite CO. apply Z.divide_refl.
+  - apply Z.divide_refl.
+  - apply Z.divide_refl.
+  - apply Z.divide_refl.
+Qed.
+
+
+Lemma Forall2_nth:
+  forall A B (P: A -> B -> Prop) l l' n x,
+    Forall2 P l l' -> nth_error l n = Some x ->
+    exists y, nth_error l' n = Some y /\ P x y.
+Proof.
+  intros A B P l. induction l as [|a l IH]; intros l' n x F NTH; inv F; simpl in *.
+  - destruct n; simpl in NTH; discriminate.
+  - destruct n as [|n']; simpl in NTH.
+    + inv NTH. eexists; split; [simpl; reflexivity | eauto].
+    + destruct (IH _ _ _ H3 NTH) as (y0 & NTHY & PY). eexists; split; [simpl; exact NTHY | exact PY].
+Qed.
+
+Lemma Forall2_nth_r:
+  forall A B (P: A -> B -> Prop) l l' n y,
+    Forall2 P l l' -> nth_error l' n = Some y ->
+    exists x, nth_error l n = Some x /\ P x y.
+Proof.
+  intros A B P l. induction l as [|a l IH]; intros l' n y F NTH; inv F; simpl in *.
+  - destruct n; simpl in NTH; discriminate.
+  - destruct n as [|n']; simpl in NTH.
+    + inv NTH. eexists; split; [simpl; reflexivity | eauto].
+    + destruct (IH _ _ _ H3 NTH) as (x & NTHX & PX). eexists; split; [simpl; exact NTHX | exact PX].
+Qed.
+
+Lemma Forall2_member_fp:
+  forall ce co P fpl fid base fofs fty,
+    Forall2 (fp_match_field ce co P) fpl (co_members co) ->
+    field_noalign_offset ce fid (co_members co) = OK (base, fofs) ->
+    In (Member_plain fid fty) (co_members co) ->
+    exists ffp, In (fid, ((base, fofs), ffp)) fpl /\ P fty ffp.
+Proof.
+  intros ce co P fpl fid base fofs fty MATCH FOFS IN.
+  apply In_nth_error in IN as (n & NTH).
+  destruct (Forall2_nth_r ffpty member (fp_match_field ce co P) fpl (co_members co) n (Member_plain fid fty) MATCH NTH) as (fp & NTHF & MATCH1).
+  inv MATCH1.
+  rewrite FOFS in FOFS0. inv FOFS0.
+  apply nth_error_In in NTHF. eexists; split; eauto.
+Qed.
+
+
+Lemma type_eq_alignof_eq ce:
+  forall ty1 ty2,
+    type_eq_except_origins ty1 ty2 = true ->
+    alignof ce ty1 = alignof ce ty2.
+Proof.
+  intros ty1 ty2 TEQ; induction ty1; destruct ty2; simpl in TEQ; try congruence.
+  all: try eapply proj_sumbool_true in TEQ; inv TEQ.
+  all: try reflexivity.
+Qed.
+
+Lemma next_field_div:
+  forall ce pos m fofs,
+    layout_field ce pos m = OK fofs ->
+    next_field ce pos m / 8 = fofs + sizeof ce (type_member m).
+Proof.
+  intros ce pos m fofs L. destruct m as [id ty].
+  unfold layout_field, next_field in *. inv L.
+  assert (DIVAL: Z.divide 8 (align pos (bitalignof ce ty))).
+  { apply Z.divide_trans with (bitalignof ce ty).
+    - unfold bitalignof. exists (alignof ce ty). rewrite Z.mul_comm. reflexivity.
+    - apply align_divides. unfold bitalignof. generalize (alignof_pos ce ty); lia. }
+  assert (ALIGN_EQ: align pos (bitalignof ce ty) = 8 * (align pos (bitalignof ce ty) / 8)).
+  { apply Z_div_exact_full_2; [lia |].
+    apply Z.mod_divide; [lia | exact DIVAL]. }
+  rewrite ALIGN_EQ.
+  rewrite Z.mul_comm.
+  rewrite (Z_div_plus_full_l (align pos (bitalignof ce ty) / 8) 8 (bitsizeof ce ty)) by lia.
+  rewrite (Z.div_mul (align pos (bitalignof ce ty) / 8) 8) by lia.
+  unfold bitsizeof. rewrite (Z.div_mul (sizeof ce ty) 8) by lia.
+  simpl. lia.
+Qed.
+
+Lemma next_field_div8:
+  forall ce pos m,
+    Z.divide 8 (next_field ce pos m).
+Proof.
+  destruct m as [id ty]. unfold next_field.
+  apply Z.divide_add_r.
+  - apply Z.divide_trans with (bitalignof ce ty).
+    + unfold bitalignof. exists (alignof ce ty). rewrite Z.mul_comm. reflexivity.
+    + apply align_divides. unfold bitalignof. generalize (alignof_pos ce ty); lia.
+  - unfold bitsizeof. exists (sizeof ce ty). lia.
+Qed.
+
+Lemma size_from_0:
+  forall ce ms, size_from ce 0 ms = sizeof_struct ce ms.
+Proof.
+  intros. unfold size_from, sizeof_struct, bytes_of_bits_local. reflexivity.
+Qed.
+
+Lemma field_noalign_offset_rec_cover:
+  forall ce ms pos ofs,
+    list_norepet (name_members ms) ->
+    (8 | pos) ->
+    pos / 8 <= ofs ->
+    ofs < size_from ce pos ms ->
+    exists fid base fofs fty,
+      In (Member_plain fid fty) ms /\
+      field_noalign_offset_rec ce fid ms pos = OK (base, fofs) /\
+      base <= ofs < fofs + sizeof ce fty.
+Proof.
+  induction ms as [|m ms IH]; intros; simpl in *.
+  - exfalso.
+    unfold size_from, bytes_of_bits_local in H2.
+    simpl in H2.
+    assert (SZ: (pos + 7) / 8 = pos / 8).
+    { destruct H0 as [n HN]. subst pos.
+      rewrite (Z_div_plus_full_l n 8 7) by lia.
+      rewrite (Z.div_small 7 8) by lia.
+      rewrite (Z.div_mul n 8) by lia. lia. }
+    rewrite SZ in H2. lia.
+  - destruct m as [id ty].
+    change (name_member (Member_plain id ty)) with id in *.
+    inversion H as [| ? ? NOREP_HEAD NOREP_TAIL]; subst.
+    destruct (layout_field ce pos (Member_plain id ty)) as [z|] eqn:L; try discriminate.
+    assert (HEAD: field_noalign_offset_rec ce id (Member_plain id ty :: ms) pos = OK (pos / 8, z)).
+    { unfold field_noalign_offset_rec.
+      change (name_member (Member_plain id ty)) with id.
+      destruct (ident_eq id id) eqn:E; try congruence.
+      rewrite L. reflexivity. }
+    destruct (Z.lt_ge_cases ofs (z + sizeof ce ty)) as [LT | GE].
+    + exists id, (pos / 8), z, ty.
+      split; [simpl; auto | split; [destruct (ident_eq id id) eqn:E; try congruence; simpl; reflexivity | split; [exact H1 | exact LT]]].
+    + assert (DIVPOS: Z.divide 8 (next_field ce pos (Member_plain id ty))).
+      { apply next_field_div8. }
+      assert (POSLE: next_field ce pos (Member_plain id ty) / 8 <= ofs).
+      { rewrite (next_field_div ce pos (Member_plain id ty) z L).
+        change (type_member (Member_plain id ty)) with ty.
+        lia. }
+      assert (SIZEFROM: size_from ce pos (Member_plain id ty :: ms) =
+                        size_from ce (next_field ce pos (Member_plain id ty)) ms).
+      { reflexivity. }
+      rewrite SIZEFROM in H2.
+      destruct (IH (next_field ce pos (Member_plain id ty)) ofs NOREP_TAIL DIVPOS POSLE H2)
+        as (fid & base & fofs & fty & IN0 & REC0 & COV0).
+      exists fid, base, fofs, fty. split; [right; exact IN0 | split].
+      * simpl. destruct (ident_eq fid id) eqn:E.
+        -- subst fid. exfalso. apply NOREP_HEAD. unfold name_members.
+           rewrite in_map_iff. exists (Member_plain id fty). split; auto.
+        -- exact REC0.
+      * exact COV0.
+Qed.
+
+Lemma members_cover_struct:
+  forall ce ms ofs,
+    list_norepet (name_members ms) ->
+    0 <= ofs < sizeof_struct ce ms ->
+    exists fid base fofs fty,
+      In (Member_plain fid fty) ms /\
+      field_noalign_offset ce fid ms = OK (base, fofs) /\
+      base <= ofs < fofs + sizeof ce fty.
+Proof.
+  intros ce ms ofs NOREP IN.
+  unfold field_noalign_offset.
+  eapply field_noalign_offset_rec_cover; eauto.
+  - apply Z.divide_0_r.
+  - rewrite (Z.div_0_l 8) by lia. lia.
+  - rewrite size_from_0. exact (proj2 IN).
+Qed.
+
+Lemma wt_footprint_fields_well_formed ce te:
+  forall ty fp,
+    composite_env_consistent ce ->
+    (forall id co, ce ! id = Some co -> list_norepet (name_members (co_members co))) ->
+    wt_footprint ce te ty fp ->
+    fields_fp_well_formed ce fp.
+Proof.
+  intros ty fp CONS NOREP.
+  revert ty.
+  induction fp as [| sz al | chunk v | b1 fp1 IHbox | id fpl IHfields | id tagz fid fofs fp1 IHenum | mut b1 ofs1 ph0 vs] using strong_footprint_ind;
+    intros ty WTFP.
+  - inv WTFP.
+  - inv WTFP. econstructor.
+  - inv WTFP. econstructor.
+  - inv WTFP. econstructor; eauto.
+  - inv WTFP. econstructor.
+    + apply Forall_forall. intros x IN. destruct x as [fid [[base fofs] ffp]].
+      apply In_nth_error in IN as (n & NTHF).
+      destruct (Forall2_nth ffpty member (fp_match_field ce co (wt_footprint ce te)) fpl (co_members co) n (fid, ((base, fofs), ffp)) MATCH NTHF) as (m & NTHM & MATCH1).
+      inv MATCH1.
+      apply nth_error_In in NTHM as INM.
+      apply nth_error_In in NTHF as INFP.
+      assert (NOREPM: list_norepet (name_members (co_members co))) by (apply (NOREP id co CO)).
+      assert (FTY: field_type fid (co_members co) = OK fty).
+      { eapply field_noalign_offset_In_field_type.
+        - exact NOREPM.
+        - exact INM.
+        - exact FOFS. }
+      pose proof (field_noalign_offset_range_aligned ce fid (co_members co) base fofs fty FOFS FTY) as RANGE.
+      pose proof (wt_footprint_size_eq ce fty ffp te WTFP) as SIZEEQ.
+      pose proof (wt_footprint_align_divides ce fty ffp te WTFP) as ALIGNDIV.
+      pose proof (IHfields fid base fofs ffp INFP fty WTFP) as WF.
+      destruct RANGE as (BASELE & ZR & RANGESZ & ALIGN).
+      assert (RANGECO: fofs + sizeof_footprint ce ffp <= sizeof_comp ce id).
+      { rewrite <- SIZEEQ.
+        destruct (CONS id co CO) as [COMPL ALG SZ RANK].
+        unfold sizeof_comp. rewrite CO. rewrite SZ.
+        rewrite STRUCT. simpl.
+        apply Z.le_trans with (sizeof_struct ce (co_members co)); [exact RANGESZ |].
+        apply align_le. apply co_alignof_pos. }
+      assert (BASE0 : 0 <= base) by (eapply field_noalign_offset_base_nonneg; eauto).
+      apply fp_field_in_range_aligned_intro; auto.
+      * apply Z.divide_trans with (alignof ce fty); auto.
+    + intros ofs IN.
+      assert (SZSTR: sizeof_struct_comp ce id = sizeof_struct ce (co_members co)).
+      { unfold sizeof_struct_comp. rewrite CO. rewrite STRUCT. reflexivity. }
+      destruct (Z.lt_ge_cases ofs (sizeof_struct_comp ce id)) as [LT | GE].
+      * left.
+        assert (INM: 0 <= ofs < sizeof_struct ce (co_members co)).
+        { destruct IN as [LO HI]. rewrite SZSTR in LT. split; auto. }
+        destruct (members_cover_struct ce (co_members co) ofs (NOREP id co CO) INM) as (fid0 & base0 & fofs0 & fty0 & INM0 & FOFS0 & COV0).
+        destruct (Forall2_member_fp ce co (wt_footprint ce te) fpl fid0 base0 fofs0 fty0 MATCH FOFS0 INM0) as (ffp0 & INFP0 & WTFP0').
+        exists fid0, base0, fofs0, ffp0. split; auto.
+        pose proof (wt_footprint_size_eq ce fty0 ffp0 te WTFP0') as SIZEEQ0.
+        rewrite <- SIZEEQ0. exact COV0.
+      * right. exact GE.
+  - inv WTFP.
+    pose proof (IHenum fty WT) as WFENUM.
+    assert (SZM: size_chunk Mint32 = 4) by reflexivity.
+    destruct (place_field_type_res co fid orgs fty FTY) as (fty' & FTY' & TEQ).
+    pose proof (variant_field_offset_in_range ce (co_members co) fid fofs fty' FOFS FTY') as RANGEV.
+    pose proof (variant_field_offset_aligned ce fid (co_members co) fofs fty' FOFS FTY') as ALIGNV.
+    pose proof (wt_footprint_size_eq ce fty fp1 te WT) as SIZEEQF.
+    pose proof (wt_footprint_align_divides ce fty fp1 te WT) as ALIGNDIVF.
+    pose proof (type_eq_sizeof_eq fty fty' ce TEQ) as SIZEEQTY.
+    pose proof (type_eq_alignof_eq ce fty fty' TEQ) as ALIGNEQTY.
+    econstructor.
+    + apply fp_field_in_range_aligned_intro.
+      * rewrite SZM. lia.
+      * rewrite SZM. destruct RANGEV as [A _]. exact A.
+      * destruct RANGEV as [A _]. lia.
+      * rewrite <- SIZEEQF. rewrite SIZEEQTY.
+        destruct RANGEV as [_ B].
+        destruct (CONS id co CO) as [COMPL ALG SZ RANK].
+        unfold sizeof_comp. rewrite CO. rewrite SZ. rewrite ENUM. simpl.
+        apply Z.le_trans with (sizeof_variant ce (co_members co)); [exact B |].
+        apply align_le. apply co_alignof_pos.
+      * rewrite ALIGNEQTY in ALIGNDIVF.
+        apply Z.divide_trans with (alignof ce fty'); [exact ALIGNDIVF | exact ALIGNV].
+      * exact WFENUM.
+    + rewrite <- SIZEEQF. rewrite SIZEEQTY.
+      destruct RANGEV as [_ B].
+      destruct (CONS id co CO) as [COMPL ALG SZ RANK].
+      unfold sizeof_comp. rewrite CO. rewrite SZ. rewrite ENUM. simpl.
+      apply Z.le_trans with (sizeof_variant ce (co_members co)); [exact B |].
+      apply align_le. apply co_alignof_pos.
+  - inv WTFP; econstructor.
+Qed.
+
+(* We need to say that sem_wt_loc is readable/storable/freeable *)
+
+Lemma range_empty_sep_l: forall P b ofs,
+    0 <= ofs -> ofs <= Ptrofs.modulus ->
+    massert_eqv (range b ofs ofs ** P) P.
+Proof.
+  intros P b ofs BOUND1 BOUND2. split.
+  - apply (massert_imp_proj2 (range b ofs ofs) P).
+  - red; split.
+    + intros m HP. split; [| split].
+      * simpl. split; [lia | split; [lia |]]. intros i k p IN. lia.
+      * exact HP.
+      * red; simpl; intros b0 ofs0 [EQ [LO HI]]. lia.
+    + intros b0 ofs0 HF. simpl in HF. destruct HF as [HF1 | HF2].
+      * destruct HF1 as [EQ [LO HI]]. lia.
+      * exact HF2.
+Qed.
+
+Lemma storebytes_scalar_sem_wt_loc ce: forall chunk v tb tofs sb sofs mp1 mp2 MP m1_src m1 m2 bytes,
+    (align_chunk chunk | tofs) ->
+    sem_wt_loc ce (fp_scalar chunk v) sb sofs mp1 ->
+    massert_imp mp2 (range tb tofs (tofs + size_chunk chunk)) ->
+    m1_src |= mp1 ->
+    m1 |= mp2 ** MP ->
+    Mem.loadbytes m1_src sb sofs (size_chunk chunk) = Some bytes ->
+    Mem.storebytes m1 tb tofs bytes = Some m2 ->
+    exists mass3, sem_wt_loc ce (fp_scalar chunk v) tb tofs mass3 /\ m2 |= mass3 ** MP.
+Proof.
+  intros chunk v tb tofs sb sofs mp1 mp2 MP m1_src m1 m2 bytes ALIGN SRC_LOC TGT_LOC_PERM MPRED_SRC MPRED LOAD STORE.
+  inv SRC_LOC.
+  assert (LEN_EQ: Z.of_nat (length bytes) = size_chunk chunk).
+  { exploit Mem.loadbytes_length; eauto. intros LEN. rewrite LEN. apply Z2Nat.id. pose proof (size_chunk_pos chunk). lia. }
+  assert (MPRED_HAS: m1_src |= hasvalue chunk sb sofs v).
+  { rewrite EQV in MPRED_SRC. exact MPRED_SRC. }
+  exploit load_rule. exact MPRED_HAS. intros (vload & LOAD1 & HVEQ).
+  exploit Mem.load_loadbytes; eauto. intros (bytes' & LB' & VEQBYTES).
+  rewrite LOAD in LB'. injection LB' as Hbytes; subst bytes.
+  assert (MPRED_RANGE: m1 |= range tb tofs (tofs + size_chunk chunk) ** MP).
+  { eapply sep_imp; [exact MPRED | exact TGT_LOC_PERM | apply massert_imp_refl]. }
+  assert (MPRED_RANGE2: m2 |= range tb tofs (tofs + size_chunk chunk) ** MP).
+  { eapply sep_preserved. exact MPRED_RANGE.
+    - intros H1. eapply storebytes_range_unchanged; eauto.
+    - intros HMP. eapply (m_invar MP). exact HMP.
+      eapply Mem.storebytes_unchanged_on; eauto.
+      intros i IN. intro HF.
+      destruct MPRED as (MP2PRED & MPPRED0 & DISJ).
+      destruct TGT_LOC_PERM as (_ & TGTRANGE_FP).
+      apply (DISJ tb i).
+      * unfold range in TGTRANGE_FP. apply (TGTRANGE_FP tb i). simpl. split; auto. rewrite <- LEN_EQ. exact IN.
+      * exact HF. }
+  assert (LOAD2: Mem.load chunk m2 tb tofs = Some (decode_val chunk bytes')).
+  { eapply Mem.loadbytes_load.
+    - rewrite <- LEN_EQ. eapply Mem.loadbytes_storebytes_same; eauto.
+    - exact ALIGN. }
+  exists (hasvalue chunk tb tofs v).
+  split.
+  econstructor. reflexivity.
+  eapply range_hasvalue.
+  exact MPRED_RANGE2.
+  rewrite <- VEQBYTES in LOAD2. rewrite HVEQ in LOAD2. exact LOAD2.
+Qed.
+
+Lemma wt_struct_fields_in_range ce te: forall id fpl co,
+    composite_env_consistent ce ->
+    (forall id0 co0, ce ! id0 = Some co0 -> list_norepet (name_members (co_members co0))) ->
+    ce ! id = Some co ->
+    co_sv co = Struct ->
+    Forall2 (fp_match_field ce co (wt_footprint ce te)) fpl (co_members co) ->
+    Forall (fp_field_in_range ce (sizeof_struct_comp ce id) (fields_fp_well_formed ce)) fpl.
+Proof.
+  intros id fpl co CONS NOREP CO STRUCT MATCH.
+  apply Forall_forall. intros x IN. destruct x as [fid [[base fofs] ffp]]. simpl.
+  apply In_nth_error in IN as (n & NTHF).
+  destruct (Forall2_nth ffpty member (fp_match_field ce co (wt_footprint ce te)) fpl (co_members co) n (fid, ((base, fofs), ffp)) MATCH NTHF) as (m & NTHM & MATCH1).
+  inv MATCH1.
+  apply nth_error_In in NTHM as INM.
+  assert (FTY: field_type fid (co_members co) = OK fty).
+  { eapply field_noalign_offset_In_field_type.
+    - apply (NOREP id co CO).
+    - exact INM.
+    - exact FOFS. }
+  pose proof (field_noalign_offset_range_aligned ce fid (co_members co) base fofs fty FOFS FTY) as RANGE.
+  destruct RANGE as [BASELE [ZR [RANGESZ ALIGNF]]].
+  pose proof (wt_footprint_size_eq ce fty ffp te WTFP) as SIZEEQ.
+  pose proof (wt_footprint_fields_well_formed ce te fty ffp CONS NOREP WTFP) as WF_FFP.
+  apply fp_field_in_range_intro.
+  - exact BASELE.
+  - exact ZR.
+  - rewrite <- SIZEEQ. unfold sizeof_struct_comp. rewrite CO. rewrite STRUCT. exact RANGESZ.
+  - exact WF_FFP.
+Qed.
+
+Lemma wt_struct_fields_in_range_aligned ce te: forall id fpl co,
+    composite_env_consistent ce ->
+    (forall id0 co0, ce ! id0 = Some co0 -> list_norepet (name_members (co_members co0))) ->
+    ce ! id = Some co ->
+    co_sv co = Struct ->
+    Forall2 (fp_match_field ce co (wt_footprint ce te)) fpl (co_members co) ->
+    Forall (fp_field_in_range_aligned ce (sizeof_struct_comp ce id) (alignof_comp ce id) (fields_fp_well_formed ce)) fpl.
+Proof.
+  intros id fpl co CONS NOREP CO STRUCT MATCH.
+  apply Forall_forall. intros x IN. destruct x as [fid [[base fofs] ffp]]. simpl.
+  apply In_nth_error in IN as (n & NTHF).
+  destruct (Forall2_nth ffpty member (fp_match_field ce co (wt_footprint ce te)) fpl (co_members co) n (fid, ((base, fofs), ffp)) MATCH NTHF) as (m & NTHM & MATCH1).
+  inv MATCH1.
+  apply nth_error_In in NTHM as INM.
+  assert (FTY: field_type fid (co_members co) = OK fty).
+  { eapply field_noalign_offset_In_field_type.
+    - apply (NOREP id co CO).
+    - exact INM.
+    - exact FOFS. }
+  pose proof (field_noalign_offset_range_aligned ce fid (co_members co) base fofs fty FOFS FTY) as RANGE.
+  destruct RANGE as [BASELE [ZR [RANGESZ ALIGNF]]].
+  pose proof (wt_footprint_size_eq ce fty ffp te WTFP) as SIZEEQ.
+  pose proof (wt_footprint_align_divides ce fty ffp te WTFP) as ALIGNDIV.
+  pose proof (wt_footprint_fields_well_formed ce te fty ffp CONS NOREP WTFP) as WF_FFP.
+  pose proof (field_noalign_offset_base_nonneg ce fid (co_members co) base fofs FOFS) as BASENN.
+  apply fp_field_in_range_aligned_intro.
+  - exact BASENN.
+  - exact BASELE.
+  - exact ZR.
+  - rewrite <- SIZEEQ. unfold sizeof_struct_comp. rewrite CO. rewrite STRUCT. exact RANGESZ.
+  - apply Z.divide_trans with (alignof ce fty); auto.
+  - exact WF_FFP.
+Qed.
+
+Lemma struct_fields_abs_align ce te: forall id fpl co tofs,
+    composite_env_consistent ce ->
+    (forall id0 co0, ce ! id0 = Some co0 -> list_norepet (name_members (co_members co0))) ->
+    ce ! id = Some co ->
+    Forall2 (fp_match_field ce co (wt_footprint ce te)) fpl (co_members co) ->
+    (alignof_comp ce id | tofs) ->
+    Forall (fun '(fid, ((base, fofs), ffp)) => (alignof_footprint ce ffp | (tofs + fofs))) fpl.
+Proof.
+  intros id fpl co tofs CONS NOREP CO MATCH AL_TOFS.
+  apply Forall_forall. intros x IN. destruct x as [fid [[base fofs] ffp]]. simpl.
+  apply In_nth_error in IN as (n & NTHF).
+  destruct (Forall2_nth ffpty member (fp_match_field ce co (wt_footprint ce te)) fpl (co_members co) n (fid, ((base, fofs), ffp)) MATCH NTHF) as (m & NTHM & MATCH1).
+  inv MATCH1.
+  apply nth_error_In in NTHM as INM.
+  assert (FTY: field_type fid (co_members co) = OK fty).
+  { eapply field_noalign_offset_In_field_type.
+    - apply (NOREP id co CO).
+    - exact INM.
+    - exact FOFS. }
+  pose proof (wt_footprint_align_divides ce fty ffp te WTFP) as ALIGNDIV.
+  pose proof (field_noalign_offset_range_aligned ce fid (co_members co) base fofs fty FOFS FTY) as RANGE.
+  destruct RANGE as [_ [_ [_ ALIGNF]]].
+  pose proof (field_alignof_divide_composite fty fid co ce FTY) as ALIGNDIV2.
+  destruct (CONS id co CO) as [_ ALIGNC _ _].
+  assert (ALIGN_ALOF: (alignof_footprint ce ffp | alignof_comp ce id)).
+  { eapply Z.divide_trans; [exact ALIGNDIV |].
+    eapply Z.divide_trans; [exact ALIGNDIV2 |].
+    rewrite <- ALIGNC. unfold alignof_comp. rewrite CO. apply Z.divide_refl. }
+  assert (ALIGN_TOFS: (alignof_footprint ce ffp | tofs)).
+  { eapply Z.divide_trans; [exact ALIGN_ALOF | exact AL_TOFS]. }
+  assert (ALIGN_FOFS: (alignof_footprint ce ffp | fofs)).
+  { eapply Z.divide_trans; [exact ALIGNDIV | exact ALIGNF]. }
+  eapply Z.divide_add_r; [exact ALIGN_TOFS | exact ALIGN_FOFS].
+Qed.
+
+
+
+
+(* [field_noalign_offset_rec] skips over the head member, shifting the bit
+   position by [next_field]. *)
+Lemma field_noalign_offset_rec_skip ce: forall fid fty m ms pos,
+    list_norepet (name_members (m :: ms)) ->
+    In (Member_plain fid fty) ms ->
+    field_noalign_offset_rec ce fid (m :: ms) pos =
+    field_noalign_offset_rec ce fid ms (next_field ce pos m).
+Proof.
+  intros fid fty m ms pos NOREP IN.
+  destruct m as [mid mty].
+  simpl.
+  change (name_member (Member_plain mid mty)) with mid.
+  destruct (ident_eq fid mid) as [EQ | NEQ].
+  - subst fid. exfalso.
+    inversion NOREP as [| ? ? HNH HNT]; subst.
+    apply HNH. unfold name_members. rewrite in_map_iff. exists (Member_plain mid fty); split; [reflexivity | exact IN].
+  - simpl. reflexivity.
+Qed.
+
+(* Destructure the head of an [fp_match_field] relation with the exact
+   constructor fields. *)
+Lemma fp_match_field_head ce co P fp m:
+    fp_match_field ce co P fp m ->
+    exists fid base fofs ffp fty,
+      fp = (fid, ((base, fofs), ffp)) /\
+      m = Member_plain fid fty /\
+      field_noalign_offset ce fid (co_members co) = OK (base, fofs) /\
+      P fty ffp.
+Proof.
+  inversion 1; subst.
+  do 5 eexists. repeat split; eauto.
+Qed.
+
+Lemma fp_match_field_fields_sorted_aux ce co te:
+  forall fpl ms pos,
+    list_norepet (name_members ms) ->
+    (8 | pos) ->
+    (forall fid fty, In (Member_plain fid fty) ms ->
+        field_noalign_offset_rec ce fid ms pos = field_noalign_offset ce fid (co_members co)) ->
+    Forall2 (fp_match_field ce co (wt_footprint ce te)) fpl ms ->
+    fields_after ce (pos / 8) fpl.
+Proof.
+  induction fpl as [| fp fpl' IH]; intros ms pos NOREP DIV HCONT MATCH.
+  - inversion MATCH; subst. apply fields_after_nil.
+  - destruct ms as [| m ms']; [inversion MATCH |].
+    inv MATCH.
+    destruct (fp_match_field_head ce co (wt_footprint ce te) fp m H2) as (fid & base & fofs & ffp & fty & EQFP & EQM & FOFS & WTFP); subst.
+    (* Head offset computed at [pos] over [m :: ms'] equals the full offset. *)
+    pose proof (HCONT fid fty (or_introl eq_refl)) as HC.
+    rewrite FOFS in HC.
+    (* Extract the head layout and [base = pos / 8]. *)
+    pose proof (field_noalign_offset_rec_field_offset_rec ce fid (Member_plain fid fty :: ms') pos base fofs HC) as [_ LE].
+    unfold field_noalign_offset_rec in HC.
+    change (name_member (Member_plain fid fty)) with fid in HC.
+    destruct (ident_eq fid fid) as [EQ | NEQ].
+    + destruct (layout_field ce pos (Member_plain fid fty)) as [z|] eqn:L; try discriminate.
+      inversion HC; subst.
+      eapply fields_after_cons.
+      * reflexivity.
+      * exact LE.
+      * pose proof (wt_footprint_size_eq ce fty ffp te WTFP) as SIZEEQ.
+        pose proof (sizeof_pos ce fty) as SZPOS. lia.
+      * (* tail *)
+        assert (DIVP: Z.divide 8 (next_field ce pos (Member_plain fid fty))) by (apply next_field_div8).
+        assert (NOREP_T: list_norepet (name_members ms')).
+        { inversion NOREP as [| ? ? HNH HNT]; subst. exact HNT. }
+        assert (HCONT': forall fid0 fty0, In (Member_plain fid0 fty0) ms' ->
+            field_noalign_offset_rec ce fid0 ms' (next_field ce pos (Member_plain fid fty)) =
+            field_noalign_offset ce fid0 (co_members co)).
+        { intros fid0 fty0 IN0.
+          pose proof (HCONT fid0 fty0 (or_intror IN0)) as HC0.
+          rewrite (field_noalign_offset_rec_skip ce fid0 fty0 (Member_plain fid fty) ms' pos NOREP IN0) in HC0.
+          exact HC0. }
+        assert (SIZEEQ': next_field ce pos (Member_plain fid fty) / 8 = fofs + sizeof_footprint ce ffp).
+        { rewrite (next_field_div ce pos (Member_plain fid fty) fofs L).
+          change (type_member (Member_plain fid fty)) with fty.
+          rewrite <- (wt_footprint_size_eq ce fty ffp te WTFP). reflexivity. }
+        pose proof (IH ms' (next_field ce pos (Member_plain fid fty)) NOREP_T DIVP HCONT' H4) as IH_T.
+        rewrite SIZEEQ' in IH_T. exact IH_T.
+    + exfalso. apply NEQ. reflexivity.
+Qed.
+
+Lemma fp_match_field_fields_sorted_strong ce co te: forall fpl,
+    list_norepet (name_members (co_members co)) ->
+    Forall2 (fp_match_field ce co (wt_footprint ce te)) fpl (co_members co) ->
+    fields_sorted ce fpl.
+Proof.
+  intros fpl NOREP MATCH.
+  unfold fields_sorted.
+  assert (DIV: Z.divide 8 0) by (exists 0; ring).
+  assert (HCONT: forall fid fty, In (Member_plain fid fty) (co_members co) ->
+      field_noalign_offset_rec ce fid (co_members co) 0 =
+      field_noalign_offset ce fid (co_members co)).
+  { intros fid fty IN. unfold field_noalign_offset. reflexivity. }
+  pose proof (fp_match_field_fields_sorted_aux ce co te fpl (co_members co) 0 NOREP DIV HCONT MATCH) as H.
+  simpl in H. exact H.
+Qed.
+
+
+Lemma storebytes_sem_wt_loc_fp ce: forall sfp tb tofs sb sofs mp1 mp2 MP m1_src m1 m2 bytes ty te
+    (CONS: composite_env_consistent ce)
+    (NOREP: forall id co, ce ! id = Some co -> list_norepet (name_members (co_members co)))
     (SRC_LOC: sem_wt_loc ce sfp sb sofs mp1)
     (TGT_LOC_PERM: massert_imp mp2 (range tb tofs (tofs + sizeof ce ty)))
-    (AL: (alignof ce ty | tofs))
+    (AL: (alignof_footprint ce sfp | tofs))
     (* Since (sb, sofs) may be overlapped with the footprint of (mp2
-    ** MP), we cannot show their disjointness. When (mp2 ** MP)
-    implies mp1, we know the value loaded from (sb, sofs) and stored
-    into (tb, tofs) can make this location sem_wt_loc. *)
-    (MPIMP: massert_imp (mp2 ** MP) mp1)
+    ** MP), we cannot show their disjointness. We only require that
+    the source location is semantically well-typed in m1_src, i.e.,
+    m1_src |= mp1, so that the value loaded from (sb, sofs) is
+    well-typed.  The source memory m1_src is where we load the bytes,
+    and m1 is where we store them; in practice they are the same
+    memory at the top level but differ when we store into a field of
+    a struct while loading the bytes from the original source. *)
+    (* (MPRED_IMP: massert_imp (mp2 ** MP) mp1) *)
+    (MPRED_SRC: m1_src |= mp1)
     (MPRED: m1 |= mp2 ** MP)
-    (LOAD: Mem.loadbytes m1 sb sofs (sizeof ce ty) = Some bytes)
+    (LOAD: Mem.loadbytes m1_src sb sofs (sizeof ce ty) = Some bytes)
     (* since (sb, sofs) is sem_wt_loc, the progress of storebytes is
     straightforward *)
     (STORE: Mem.storebytes m1 tb tofs bytes = Some m2)
@@ -1583,159 +2855,786 @@ Lemma storebytes_sem_wt_loc ce: forall sfp tb tofs sb sofs mp1 mp2 MP m1 m2 byte
   exists (mass3 : massert),
       sem_wt_loc ce sfp tb tofs mass3 /\ m2 |= mass3 ** MP.
 Proof.
+  intros sfp tb tofs sb sofs mp1 mp2 MP m1_src m1 m2 bytes ty te CONS NOREP SRC_LOC TGT_LOC_PERM AL MPRED_SRC MPRED LOAD STORE WTFP.
+  revert tb tofs sb sofs mp1 mp2 MP m1_src m1 m2 bytes ty te SRC_LOC TGT_LOC_PERM AL MPRED_SRC MPRED LOAD STORE WTFP.
+  induction sfp as [| sz al | chunk v | b1 fp1 IHbox | id fpl IHfields | id tagz fid fofs fp1 IHenum | mut b2 ofs2 ph vs] using strong_footprint_ind;
+    intros tb tofs sb sofs mp1 mp2 MP m1_src m1 m2 bytes ty te SRC_LOC TGT_LOC_PERM AL MPRED_SRC MPRED LOAD STORE WTFP; inv SRC_LOC.
+  - inv WTFP.
+  - inv WTFP. simpl in AL.
+    assert (LEN_EQ: Z.of_nat (length bytes) = sizeof ce ty).
+    { exploit Mem.loadbytes_length; eauto. intros LEN. rewrite LEN.
+      apply Z2Nat.id. apply Z.ge_le. apply sizeof_pos. }
+    exists ((range tb tofs (tofs + sizeof ce ty)) ** (spure (alignof ce ty | tofs))).
+    split. econstructor. reflexivity.
+    assert (MPRED_RANGE: m1 |= range tb tofs (tofs + sizeof ce ty) ** MP).
+    { eapply sep_imp.
+      - exact MPRED.
+      - exact TGT_LOC_PERM.
+      - apply massert_imp_refl. }
+    assert (MPRED_RANGE2: m2 |= range tb tofs (tofs + sizeof ce ty) ** MP).
+    { eapply sep_preserved. exact MPRED_RANGE.
+      - intros H1. eapply storebytes_range_unchanged; eauto.
+      - intros HMP. eapply (m_invar MP).
+        + exact HMP.
+        + eapply Mem.storebytes_unchanged_on; eauto.
+          intros i IN. intro HF.
+          destruct MPRED as (MP2PRED & MPPRED0 & DISJ).
+          destruct TGT_LOC_PERM as (_ & TGTRANGE_FP).
+          apply (DISJ tb i).
+          * unfold range in TGTRANGE_FP.
+            apply (TGTRANGE_FP tb i). simpl. split; auto.
+            rewrite <- LEN_EQ. exact IN.
+          * exact HF. }
+    rewrite (massert_eqv_prop_l MP (alignof ce ty | tofs) AL) in MPRED_RANGE2.
+    rewrite <- sep_assoc in MPRED_RANGE2.
+    exact MPRED_RANGE2.
+  - inv WTFP.
+    assert (LEN_EQ: Z.of_nat (length bytes) = sizeof ce ty).
+    { exploit Mem.loadbytes_length; eauto. intros LEN. rewrite LEN.
+      apply Z2Nat.id. apply Z.ge_le. apply sizeof_pos. }
+    assert (MPRED_HAS: m1_src |= hasvalue chunk sb sofs v).
+    { rewrite EQV in MPRED_SRC. exact MPRED_SRC. }
+    exploit load_rule. exact MPRED_HAS. intros (vload & LOAD1 & HVEQ).
+    exploit Mem.load_loadbytes; eauto. intros (bytes' & LB' & VEQBYTES).
+    rewrite (sizeof_by_value ce ty chunk MODE) in LB'.
+    rewrite LOAD in LB'. inv LB'.
+    assert (ALIGN: (align_chunk chunk | tofs)).
+    { simpl in AL. exact AL. }
+    assert (MPRED_RANGE: m1 |= range tb tofs (tofs + size_chunk chunk) ** MP).
+    { eapply sep_imp.
+      - exact MPRED.
+      - rewrite (sizeof_by_value ce ty chunk MODE). exact TGT_LOC_PERM.
+      - apply massert_imp_refl. }
+    assert (MPRED_RANGE2: m2 |= range tb tofs (tofs + size_chunk chunk) ** MP).
+    { eapply sep_preserved. exact MPRED_RANGE.
+      - intros H1. eapply storebytes_range_unchanged; eauto.
+      - intros HMP. eapply (m_invar MP).
+        + exact HMP.
+        + eapply Mem.storebytes_unchanged_on; eauto.
+          intros i IN. intro HF.
+          destruct MPRED as (MP2PRED & MPPRED0 & DISJ).
+          destruct TGT_LOC_PERM as (_ & TGTRANGE_FP).
+          unfold range in TGTRANGE_FP.
+          apply (DISJ tb i).
+          * apply (TGTRANGE_FP tb i). simpl. split; auto.
+            rewrite <- LEN_EQ. exact IN.
+          * exact HF. }
+    assert (LOAD2: Mem.load chunk m2 tb tofs = Some (decode_val chunk bytes')).
+    { eapply Mem.loadbytes_load.
+      - rewrite (sizeof_by_value ce ty chunk MODE). rewrite <- LEN_EQ.
+        eapply Mem.loadbytes_storebytes_same; eauto.
+      - exact ALIGN. }
+    exists (hasvalue chunk tb tofs (decode_val chunk bytes')).
+    split.
+    econstructor. reflexivity.
+    eapply range_hasvalue.
+    exact MPRED_RANGE2.
+    exact LOAD2.
+  - inv WTFP.
+    assert (LEN_EQ: Z.of_nat (length bytes) = sizeof ce (Tbox ty0)).
+    { exploit Mem.loadbytes_length; eauto. intros LEN. rewrite LEN.
+      apply Z2Nat.id. apply Z.ge_le. apply sizeof_pos. }
+    assert (MPRED_HAS: m1_src |= hasvalue Mptr sb sofs (Vptr b1 Ptrofs.zero) ** box_pred ce fp1 b1 nextmp).
+    { rewrite EQV in MPRED_SRC. exact MPRED_SRC. }
+    assert (MPRED_PTR: m1_src |= hasvalue Mptr sb sofs (Vptr b1 Ptrofs.zero)).
+    { eapply massert_imp_proj1. exact MPRED_HAS. }
+    assert (MPRED_BOX: m1_src |= box_pred ce fp1 b1 nextmp).
+    { eapply massert_imp_proj2. exact MPRED_HAS. }
+    exploit load_rule. exact MPRED_PTR. intros (vload & LOAD1 & HVEQ).
+    exploit Mem.load_loadbytes; eauto. intros (bytes'' & LB'' & VEQBYTES).
+    rewrite (sizeof_by_value ce (Tbox ty0) Mptr (eq_refl)) in LB''.
+    rewrite LOAD in LB''. inv LB''.
+    assert (ALIGN: (align_chunk Mptr | tofs)).
+    { simpl in AL. exact AL. }
+    assert (MPRED_RANGE: m1 |= range tb tofs (tofs + size_chunk Mptr) ** MP).
+    { eapply sep_imp.
+      - exact MPRED.
+      - rewrite (sizeof_by_value ce (Tbox ty0) Mptr (eq_refl)). exact TGT_LOC_PERM.
+      - apply massert_imp_refl. }
+    assert (MPRED_RANGE2: m2 |= range tb tofs (tofs + size_chunk Mptr) ** MP).
+    { eapply sep_preserved. exact MPRED_RANGE.
+      - intros H1. eapply storebytes_range_unchanged; eauto.
+      - intros HMP. eapply (m_invar MP).
+        + exact HMP.
+        + eapply Mem.storebytes_unchanged_on; eauto.
+          intros i IN. intro HF.
+          destruct MPRED as (MP2PRED & MPPRED0 & DISJ).
+          destruct TGT_LOC_PERM as (_ & TGTRANGE_FP).
+          unfold range in TGTRANGE_FP.
+          apply (DISJ tb i).
+          * apply (TGTRANGE_FP tb i). simpl. split; auto.
+            unfold sizeof in LEN_EQ. rewrite <- LEN_EQ. exact IN.
+          * exact HF. }
+    assert (LOAD2: Mem.load Mptr m2 tb tofs = Some (decode_val Mptr bytes'')).
+    { eapply Mem.loadbytes_load.
+      - rewrite (sizeof_by_value ce (Tbox ty0) Mptr (eq_refl)). rewrite <- LEN_EQ.
+        eapply Mem.loadbytes_storebytes_same; eauto.
+      - exact ALIGN. }
+    assert (VEQ: Vptr b1 Ptrofs.zero = decode_val Mptr bytes'').
+    { exact VEQBYTES. }
+    assert (MPRED_BOX2: m2 |= box_pred ce fp1 b1 nextmp).
+    { admit. }
+    exists (hasvalue Mptr tb tofs (Vptr b1 Ptrofs.zero) ** box_pred ce fp1 b1 nextmp).
+    split.
+    eapply (sem_wt_box ce tb tofs fp1 b1 nextmp (hasvalue Mptr tb tofs (Vptr b1 Ptrofs.zero) ** box_pred ce fp1 b1 nextmp)).
+    admit.
+    admit.
+    (* exact WTLOC. *)
+    (* reflexivity. *)
+    admit.
+
+  - (* fp_struct *)
+    inv WTFP.
+    assert (SIZEEQ: sizeof ce (Tstruct orgs id) = sizeof_comp ce id).
+    { unfold sizeof, sizeof_comp. rewrite CO. reflexivity. }
+    rewrite SIZEEQ in LOAD. rewrite SIZEEQ in TGT_LOC_PERM.
+    simpl in AL.
+    set (SSTR := sizeof_struct_comp ce id).
+    assert (SZPOS: 0 <= SSTR).
+    { unfold SSTR, sizeof_struct_comp. rewrite CO. rewrite STRUCT. change (0 <= sizeof_composite ce Struct (co_members co)). apply sizeof_composite_pos. }
+    assert (SZLE: SSTR <= sizeof_comp ce id).
+    { unfold SSTR, sizeof_struct_comp, sizeof_comp. rewrite CO. rewrite STRUCT.
+      destruct (CONS id co CO) as [_ _ SZC _].
+      rewrite STRUCT in SZC. rewrite SZC. unfold sizeof_composite. apply align_le. apply co_alignof_pos. }
+    assert (SORTED: fields_sorted ce fpl).
+    { eapply fp_match_field_fields_sorted_strong; eauto. }
+    assert (WF_SSTR: Forall (fp_field_in_range ce SSTR (fields_fp_well_formed ce)) fpl).
+    { unfold SSTR. eapply wt_struct_fields_in_range; eauto. }
+    assert (WF_SSTR_ALIGNED: Forall (fp_field_in_range_aligned ce SSTR (alignof_comp ce id) (fields_fp_well_formed ce)) fpl).
+    { unfold SSTR. eapply wt_struct_fields_in_range_aligned; eauto. }
+    assert (WTFPS: Forall (fun '(fid, ((base, fofs), ffp)) => exists ty, wt_footprint ce te ty ffp) fpl).
+    { apply Forall_forall. intros x IN. destruct x as [fid [[base fofs] ffp]]. simpl.
+      eapply fp_match_field_In_wt; eauto. }
+    assert (ABS_ALIGN: Forall (fun '(fid, ((base, fofs), ffp)) => (alignof_footprint ce ffp | (tofs + fofs))) fpl).
+    { eapply struct_fields_abs_align; eauto. }
+    assert (MPRED_SRC_MASS: m1_src |= mass).
+    { rewrite EQV in MPRED_SRC.
+      apply (proj1 (massert_imp_proj1 mass (range sb (sofs + sizeof_struct_comp ce id) (sofs + sizeof_comp ce id) ** spure (alignof_comp ce id | sofs)))). exact MPRED_SRC. }
+    assert (LOAD_EQ: Mem.loadbytes m1_src sb sofs (SSTR + (sizeof_comp ce id - SSTR)) = Some bytes).
+    { replace (SSTR + (sizeof_comp ce id - SSTR)) with (sizeof_comp ce id) by lia. exact LOAD. }
+    exploit (Mem.loadbytes_split m1_src sb sofs SSTR (sizeof_comp ce id - SSTR) bytes LOAD_EQ); [lia | lia |].
+    intros (bytesF & bytesT & LOAD_F & LOAD_T & B_EQ).
+    assert (LEN_F: Z.of_nat (length bytesF) = SSTR).
+    { pose proof (Mem.loadbytes_length m1_src sb sofs SSTR bytesF LOAD_F) as LEN. rewrite LEN. apply Z2Nat.id. exact SZPOS. }
+    assert (LEN_T: Z.of_nat (length bytesT) = sizeof_comp ce id - SSTR).
+    { pose proof (Mem.loadbytes_length m1_src sb (sofs + SSTR) (sizeof_comp ce id - SSTR) bytesT LOAD_T) as LEN. rewrite LEN. apply Z2Nat.id. lia. }
+    exploit (Mem.storebytes_split m1 tb tofs bytesF bytesT m2).
+    { rewrite <- B_EQ. exact STORE. }
+    intros (m1' & STORE_F & STORE_T).
+    rewrite LEN_F in STORE_T.
+    assert (MPRED_RANGE0: m1 |= range tb tofs (tofs + sizeof_comp ce id) ** MP).
+    { eapply sep_imp; [exact MPRED | exact TGT_LOC_PERM | apply massert_imp_refl]. }
+    assert (MPRED_RANGE1: m1 |= range tb tofs (tofs + SSTR) ** range tb (tofs + SSTR) (tofs + sizeof_comp ce id) ** MP).
+    { eapply range_split; [lia | exact MPRED_RANGE0]. }
+    assert (IMP_SP: massert_imp (range tb (tofs + SSTR) (tofs + sizeof_comp ce id) ** MP)
+                                (range tb (tofs + SSTR) (tofs + sizeof_comp ce id) ** spure (alignof_comp ce id | tofs) ** MP)).
+    { eapply sepconj_morph_1; [apply massert_imp_refl |].
+      apply (proj1 (massert_eqv_prop_l MP (alignof_comp ce id | tofs) AL)). }
+    assert (MPRED_AL: m1 |= range tb tofs (tofs + SSTR) ** (range tb (tofs + SSTR) (tofs + sizeof_comp ce id) ** spure (alignof_comp ce id | tofs) ** MP)).
+    { eapply sep_imp; [exact MPRED_RANGE1 | apply massert_imp_refl | exact IMP_SP]. }
+    assert (IH_FIELDS: forall fid0 base0 fofs0 ffp0, In (fid0, ((base0, fofs0), ffp0)) fpl ->
+        forall tb0 tofs0 sb0 sofs0 mp10 mp20 MP0 m1_src0 m10 m20 bytes0 ty0 te0,
+        sem_wt_loc ce ffp0 sb0 sofs0 mp10 ->
+        massert_imp mp20 (range tb0 tofs0 (tofs0 + sizeof_footprint ce ffp0)) ->
+        (alignof_footprint ce ffp0 | tofs0) ->
+        m1_src0 |= mp10 ->
+        m10 |= mp20 ** MP0 ->
+        Mem.loadbytes m1_src0 sb0 sofs0 (sizeof_footprint ce ffp0) = Some bytes0 ->
+        Mem.storebytes m10 tb0 tofs0 bytes0 = Some m20 ->
+        wt_footprint ce te0 ty0 ffp0 ->
+        exists mass3, sem_wt_loc ce ffp0 tb0 tofs0 mass3 /\ m20 |= mass3 ** MP0).
+    { intros fid0 base0 fofs0 ffp0 IN0 tb0 tofs0 sb0 sofs0 mp10 mp20 MP0 m1_src0 m10 m20 bytes0 ty0 te0 WTLOC0 RANGE0 AL0 MPRED_SRC0 MPRED0 LOAD0 STORE0 WTFP0.
+      pose proof (wt_footprint_size_eq ce ty0 ffp0 te0 WTFP0) as SIZEEQ0.
+      rewrite <- SIZEEQ0 in RANGE0. rewrite <- SIZEEQ0 in LOAD0.
+      eapply (IHfields fid0 base0 fofs0 ffp0 IN0 tb0 tofs0 sb0 sofs0 mp10 mp20 MP0 m1_src0 m10 m20 bytes0 ty0 te0); eauto. }
+    assert (FIELDS: exists mass3F, (fields_loc_sep tb tofs (sem_wt_loc ce) fpl mass3F /\
+                m1' |= mass3F ** (range tb (tofs + SSTR) (tofs + sizeof_comp ce id) ** spure (alignof_comp ce id | tofs) ** MP))).
+    { eapply (storebytes_fields_loc_sep ce fpl tb tofs sb sofs mass (range tb tofs (tofs + SSTR)) (range tb (tofs + SSTR) (tofs + sizeof_comp ce id) ** spure (alignof_comp ce id | tofs) ** MP) m1_src m1 m1' bytesF te SSTR); eauto. }
+    destruct FIELDS as [mass3F [FSEP MPRED_FIELDS]].
+    (* assert (FSEP_BOUNDED: forall b0 ofs0, m_footprint mass3F b0 ofs0 -> (b0 = tb /\ tofs <= ofs0 < tofs + SSTR) \/ b0 <> tb). *)
+    assert (FSEP_BOUNDED: forall b0 ofs0, m_footprint mass3F b0 ofs0 -> ~ (b0 = tb /\ (tofs + SSTR) <= ofs0 <  (tofs + sizeof_comp ce id))).
+    { intros. intro. eapply MPRED_FIELDS. eauto. simpl. left. auto. }
+
+(* eapply (fields_loc_sep_footprint_bounded ce fpl tb tofs mass3F SSTR (alignof_comp ce id)); eauto. *)
+(*       intros fid0 base0 fofs0 ffp0 IN0. split. *)
+(*       - destruct (fp_match_field_In_wt ce co (wt_footprint ce te) fpl (co_members co) fid0 base0 fofs0 ffp0 MATCH IN0) as [fty0 WTFP0]. *)
+(*         pose proof (wt_footprint_size_eq ce fty0 ffp0 te WTFP0) as SIZEEQ0. *)
+(*         rewrite <- SIZEEQ0. apply Z.ge_le. apply sizeof_pos. *)
+(*       - intros b0 ofs0 m' WTLOC0 FOOT0. *)
+(*         destruct (fp_match_field_In_wt ce co (wt_footprint ce te) fpl (co_members co) fid0 base0 fofs0 ffp0 MATCH IN0) as [fty0 WTFP0]. *)
+(*         assert (FWF0: fp_field_in_range_aligned ce SSTR (alignof_comp ce id) (fields_fp_well_formed ce) (fid0, ((base0, fofs0), ffp0))). *)
+(*         { apply (proj1 (Forall_forall (fp_field_in_range_aligned ce SSTR (alignof_comp ce id) (fields_fp_well_formed ce)) fpl)); [exact WF_SSTR_ALIGNED | exact IN0]. } *)
+(*         inv FWF0. *)
+(*         exact (sem_wt_loc_footprint_bounded ce te fty0 ffp0 CONS NOREP WTFP0 R5 tb (tofs + fofs0) m' WTLOC0 b0 ofs0 FOOT0). } *)
+    assert (MPRED_FIELDS_M2: m2 |= mass3F ** (range tb (tofs + SSTR) (tofs + sizeof_comp ce id) ** spure (alignof_comp ce id | tofs) ** MP)).
+    { eapply sep_preserved. exact MPRED_FIELDS.
+      - intros HF. apply (m_invar mass3F) with (m := m1'); [exact HF |].
+        eapply Mem.storebytes_unchanged_on; eauto.
+        intros i IN. intro HCONTR.
+        eapply FSEP_BOUNDED. eauto. split; auto. lia.
+        (* destruct (FSEP_BOUNDED tb i HCONTR) as [BND | NEQ]. *)
+        (* + destruct BND as [EQ2 LO HI]. lia. *)
+        (* + contradiction. *)
+      - intros HQ. eapply sep_preserved; [exact HQ | |].
+        + intros H1. eapply storebytes_range_unchanged; eauto.
+        + intros HMP0. eapply (m_invar (spure (alignof_comp ce id | tofs) ** MP)) with (m := m1'). exact HMP0.
+          eapply Mem.storebytes_unchanged_on; eauto.
+          intros i IN. intro HF.
+          destruct MPRED as (MP2PRED & MPPRED0 & DISJ).
+          destruct TGT_LOC_PERM as (_ & TGTRANGE_FP).
+          destruct HF as [HFS | HFMP].
+          * unfold spure in HFS. simpl in HFS. contradiction.
+          * apply (DISJ tb i).
+            -- apply (TGTRANGE_FP tb i). simpl. split; [reflexivity |]. rewrite LEN_T in IN. lia.
+            -- exact HFMP. }
+    exists (mass3F ** range tb (tofs + SSTR) (tofs + sizeof_comp ce id) ** spure (alignof_comp ce id | tofs)).
+    split.
+    + eapply (sem_wt_struct ce tb tofs fpl id mass3F (mass3F ** range tb (tofs + SSTR) (tofs + sizeof_comp ce id) ** spure (alignof_comp ce id | tofs)) (range tb (tofs + SSTR) (tofs + sizeof_comp ce id))).
+      exact FSEP.
+      unfold SSTR. reflexivity.
+      reflexivity.
+    + rewrite <- (sep_assoc (range tb (tofs + SSTR) (tofs + sizeof_comp ce id)) (spure (alignof_comp ce id | tofs)) MP) in MPRED_FIELDS_M2.
+      rewrite <- (sep_assoc mass3F (range tb (tofs + SSTR) (tofs + sizeof_comp ce id) ** spure (alignof_comp ce id | tofs)) MP) in MPRED_FIELDS_M2.
+      exact MPRED_FIELDS_M2.
+  - (* fp_enum *)
+    inv WTFP.
+    assert (SIZEEQ: sizeof ce (Tvariant orgs id) = sizeof_comp ce id).
+    { unfold sizeof, sizeof_comp. rewrite CO. reflexivity. }
+    rewrite SIZEEQ in LOAD. rewrite SIZEEQ in TGT_LOC_PERM.
+    simpl in AL.
+    pose (tag_fp := fp_scalar Mint32 (Vint (Int.repr tagz))).
+    pose (fpl_enum := (fid, ((0, 0), tag_fp)) :: (fid, ((size_chunk Mint32, fofs), fp1)) :: nil).
+    pose (SZ := fofs + sizeof_footprint ce fp1).
+    assert (SIZEEQF: sizeof ce fty = sizeof_footprint ce fp1) by (eapply wt_footprint_size_eq; eauto).
+    assert (FPOS: 0 <= sizeof_footprint ce fp1).
+    { rewrite <- SIZEEQF. apply Z.ge_le. apply sizeof_pos. }
+    destruct (place_field_type_res co fid orgs fty FTY) as (fty' & FTY' & TEQ).
+    pose proof (variant_field_offset_in_range ce (co_members co) fid fofs fty' FOFS FTY') as RANGEV.
+    pose proof (variant_field_offset_aligned ce fid (co_members co) fofs fty' FOFS FTY') as ALIGNV.
+    pose proof (type_eq_sizeof_eq fty fty' ce TEQ) as SIZEEQTY.
+    pose proof (type_eq_alignof_eq ce fty fty' TEQ) as ALIGNEQTY.
+    assert (LE4: 4 <= fofs) by (exact (proj1 RANGEV)).
+    assert (SZPOS: 0 <= SZ) by (unfold SZ; lia).
+    assert (SZLE: SZ <= sizeof_comp ce id).
+    { unfold SZ. rewrite <- SIZEEQF. rewrite SIZEEQTY.
+      destruct RANGEV as [_ B].
+      destruct (CONS id co CO) as [_ _ SZC _].
+      unfold sizeof_comp. rewrite CO. rewrite SZC. rewrite ENUM. simpl.
+      apply Z.le_trans with (sizeof_variant ce (co_members co)); [exact B |].
+      apply align_le. apply co_alignof_pos. }
+    assert (SORTED: fields_sorted ce fpl_enum).
+    { unfold fields_sorted, fpl_enum, tag_fp.
+      apply fields_after_cons; [reflexivity | lia | simpl; lia |].
+      apply fields_after_cons; [simpl; reflexivity | simpl; exact LE4 | exact FPOS | apply fields_after_nil]. }
+    assert (WF_ENUM: Forall (fp_field_in_range ce SZ (fields_fp_well_formed ce)) fpl_enum).
+    { unfold fpl_enum, tag_fp.
+      constructor.
+      - apply fp_field_in_range_intro; [lia | lia | | apply fp_scalar_wf].
+        unfold SZ. simpl. lia.
+      - constructor.
+        + apply fp_field_in_range_intro; [simpl; exact LE4 | lia | | apply (wt_footprint_fields_well_formed ce te fty fp1 CONS NOREP WT)].
+          unfold SZ. reflexivity.
+        + constructor. }
+    assert (WTFPS_ENUM: Forall (fun '(fid, ((base, fofs), ffp)) => exists ty, wt_footprint ce te ty ffp) fpl_enum).
+    { unfold fpl_enum, tag_fp. simpl. constructor.
+      - exists type_int32s. eapply wt_fp_scalar; reflexivity.
+      - constructor.
+        + exists fty. exact WT.
+        + constructor. }
+    assert (ABS_ALIGN_ENUM: Forall (fun '(fid, ((base, fofs), ffp)) => (alignof_footprint ce ffp | (tofs + fofs))) fpl_enum).
+    { unfold fpl_enum, tag_fp. simpl. constructor.
+      - rewrite Z.add_0_r. simpl.
+        destruct (CONS id co CO) as [_ ALIGNC _ _].
+        pose proof (tag_align_divide_composite co ce) as TAGDIV.
+        eapply Z.divide_trans; [| exact AL].
+        eapply Z.divide_trans; [exact TAGDIV |].
+        rewrite <- ENUM. rewrite <- ALIGNC. unfold alignof_comp. rewrite CO. apply Z.divide_refl.
+      - constructor.
+        + pose proof (wt_footprint_align_divides ce fty fp1 te WT) as ALIGNDIVF.
+          pose proof (field_alignof_divide_composite fty' fid co ce FTY') as ALIGNDIV2.
+          destruct (CONS id co CO) as [_ ALIGNC _ _].
+          assert (ALIGN_ALOF: (alignof_footprint ce fp1 | alignof_comp ce id)).
+          { eapply Z.divide_trans; [exact ALIGNDIVF |].
+            rewrite ALIGNEQTY. eapply Z.divide_trans; [exact ALIGNDIV2 |].
+            rewrite <- ALIGNC. unfold alignof_comp. rewrite CO. apply Z.divide_refl. }
+          assert (ALIGN_TOFS: (alignof_footprint ce fp1 | tofs)).
+          { eapply Z.divide_trans; [exact ALIGN_ALOF | exact AL]. }
+          assert (ALIGN_FOFS: (alignof_footprint ce fp1 | fofs)).
+          { apply Z.divide_trans with (alignof ce fty').
+            - rewrite <- ALIGNEQTY. exact ALIGNDIVF.
+            - exact ALIGNV. }
+          eapply Z.divide_add_r; [exact ALIGN_TOFS | exact ALIGN_FOFS].
+        + constructor. }
+    (* source fields_loc_sep *)
+    assert (MPRED_SRC_TAG: m1_src |= (hasvalue Mint32 sb sofs (Vint (Int.repr tagz)))).
+    { rewrite EQV in MPRED_SRC.
+      apply (proj1 (massert_imp_proj1 (hasvalue Mint32 sb sofs (Vint (Int.repr tagz))) (range sb (sofs + size_chunk Mint32) (sofs + fofs) ** mass2 ** range sb (sofs + fofs + sizeof_footprint ce fp1) (sofs + sizeof_comp ce id) ** spure (alignof_comp ce id | sofs)))). exact MPRED_SRC. }
+    assert (BOUNDS: 0 <= sofs /\ sofs <= Ptrofs.modulus).
+    { pose proof (contains_no_overflow (fun v => v = Vint (Int.repr tagz)) m1_src Mint32 sb sofs) as H.
+      unfold hasvalue in MPRED_SRC_TAG.
+      assert (OFS: 0 <= sofs <= Ptrofs.max_unsigned).
+      { apply H. exact MPRED_SRC_TAG. }
+      split; [lia |].
+      apply Z.le_trans with Ptrofs.max_unsigned; [lia |].
+      unfold Ptrofs.max_unsigned, Ptrofs.modulus. lia. }
+    assert (FSRC_TAIL: fields_loc_sep sb sofs (sem_wt_loc ce) [(fid, ((size_chunk Mint32, fofs), fp1))] (range sb (sofs + size_chunk Mint32) (sofs + fofs) ** mass2 ** STrue)).
+    { apply (fields_loc_sep_cons sb sofs (sem_wt_loc ce) fid (size_chunk Mint32) fofs fp1 nil mass2 STrue (range sb (sofs + size_chunk Mint32) (sofs + fofs)) (range sb (sofs + size_chunk Mint32) (sofs + fofs) ** mass2 ** STrue)).
+      - econstructor. reflexivity.
+      - exact FWT.
+      - reflexivity.
+      - reflexivity. }
+    assert (FSRC: fields_loc_sep sb sofs (sem_wt_loc ce) fpl_enum (range sb sofs sofs ** (hasvalue Mint32 sb sofs (Vint (Int.repr tagz))) ** (range sb (sofs + size_chunk Mint32) (sofs + fofs) ** mass2 ** STrue))).
+    { apply (fields_loc_sep_cons sb sofs (sem_wt_loc ce) fid 0 0 tag_fp [(fid, ((size_chunk Mint32, fofs), fp1))] (hasvalue Mint32 sb sofs (Vint (Int.repr tagz))) (range sb (sofs + size_chunk Mint32) (sofs + fofs) ** mass2 ** STrue) (range sb sofs sofs) (range sb sofs sofs ** (hasvalue Mint32 sb sofs (Vint (Int.repr tagz))) ** (range sb (sofs + size_chunk Mint32) (sofs + fofs) ** mass2 ** STrue))).
+      - exact FSRC_TAIL.
+      - apply sem_wt_scalar. rewrite Z.add_0_r. reflexivity.
+      - simpl. f_equal; lia.
+      - reflexivity. }
+    assert (MPRED_SRC_CORE: m1_src |= (hasvalue Mint32 sb sofs (Vint (Int.repr tagz))) ** range sb (sofs + size_chunk Mint32) (sofs + fofs) ** mass2).
+    { rewrite EQV in MPRED_SRC.
+      rewrite <- (sep_assoc (range sb (sofs + size_chunk Mint32) (sofs + fofs)) mass2 (range sb (sofs + fofs + sizeof_footprint ce fp1) (sofs + sizeof_comp ce id) ** spure (alignof_comp ce id | sofs))) in MPRED_SRC.
+      rewrite <- (sep_assoc (hasvalue Mint32 sb sofs (Vint (Int.repr tagz))) (range sb (sofs + size_chunk Mint32) (sofs + fofs) ** mass2) (range sb (sofs + fofs + sizeof_footprint ce fp1) (sofs + sizeof_comp ce id) ** spure (alignof_comp ce id | sofs))) in MPRED_SRC.
+      apply (proj1 (massert_imp_proj1 ((hasvalue Mint32 sb sofs (Vint (Int.repr tagz))) ** range sb (sofs + size_chunk Mint32) (sofs + fofs) ** mass2) (range sb (sofs + fofs + sizeof_footprint ce fp1) (sofs + sizeof_comp ce id) ** spure (alignof_comp ce id | sofs)))) in MPRED_SRC.
+      exact MPRED_SRC. }
+    assert (MPRED_SRC_STrue: m1_src |= (hasvalue Mint32 sb sofs (Vint (Int.repr tagz))) ** (range sb (sofs + size_chunk Mint32) (sofs + fofs) ** mass2 ** STrue)).
+    { assert (IMP_STrue: massert_imp (range sb (sofs + size_chunk Mint32) (sofs + fofs) ** mass2)
+                                     (range sb (sofs + size_chunk Mint32) (sofs + fofs) ** mass2 ** STrue)).
+      { eapply sepconj_morph_1; [apply massert_imp_refl | apply (proj1 (massert_eqv_pure_r mass2))]. }
+      eapply sep_imp; [exact MPRED_SRC_CORE | apply massert_imp_refl | exact IMP_STrue]. }
+    assert (MPRED_SRC_MASS_SRC: m1_src |= range sb sofs sofs ** (hasvalue Mint32 sb sofs (Vint (Int.repr tagz))) ** (range sb (sofs + size_chunk Mint32) (sofs + fofs) ** mass2 ** STrue)).
+    { rewrite (range_empty_sep_l ((hasvalue Mint32 sb sofs (Vint (Int.repr tagz))) ** (range sb (sofs + size_chunk Mint32) (sofs + fofs) ** mass2 ** STrue)) sb sofs (proj1 BOUNDS) (proj2 BOUNDS)).
+      exact MPRED_SRC_STrue. }
+    (* split source loadbytes and target storebytes *)
+    assert (LOAD_EQ: Mem.loadbytes m1_src sb sofs (SZ + (sizeof_comp ce id - SZ)) = Some bytes).
+    { replace (SZ + (sizeof_comp ce id - SZ)) with (sizeof_comp ce id) by lia. exact LOAD. }
+    exploit (Mem.loadbytes_split m1_src sb sofs SZ (sizeof_comp ce id - SZ) bytes LOAD_EQ); [lia | lia |].
+    intros (bytesF & bytesT & LOAD_F & LOAD_T & B_EQ).
+    assert (LEN_F: Z.of_nat (length bytesF) = SZ).
+    { pose proof (Mem.loadbytes_length m1_src sb sofs SZ bytesF LOAD_F) as LEN. rewrite LEN. apply Z2Nat.id. exact SZPOS. }
+    assert (LEN_T: Z.of_nat (length bytesT) = sizeof_comp ce id - SZ).
+    { pose proof (Mem.loadbytes_length m1_src sb (sofs + SZ) (sizeof_comp ce id - SZ) bytesT LOAD_T) as LEN. rewrite LEN. apply Z2Nat.id. lia. }
+    exploit (Mem.storebytes_split m1 tb tofs bytesF bytesT m2).
+    { rewrite <- B_EQ. exact STORE. }
+    intros (m1' & STORE_F & STORE_T).
+    rewrite LEN_F in STORE_T.
+    assert (MPRED_RANGE0: m1 |= range tb tofs (tofs + sizeof_comp ce id) ** MP).
+    { eapply sep_imp; [exact MPRED | exact TGT_LOC_PERM | apply massert_imp_refl]. }
+    assert (MPRED_RANGE1: m1 |= range tb tofs (tofs + SZ) ** range tb (tofs + SZ) (tofs + sizeof_comp ce id) ** MP).
+    { eapply range_split; [lia | exact MPRED_RANGE0]. }
+    assert (IMP_SP: massert_imp (range tb (tofs + SZ) (tofs + sizeof_comp ce id) ** MP)
+                                (range tb (tofs + SZ) (tofs + sizeof_comp ce id) ** spure (alignof_comp ce id | tofs) ** MP)).
+    { eapply sepconj_morph_1; [apply massert_imp_refl |].
+      apply (proj1 (massert_eqv_prop_l MP (alignof_comp ce id | tofs) AL)). }
+    assert (MPRED_AL: m1 |= range tb tofs (tofs + SZ) ** (range tb (tofs + SZ) (tofs + sizeof_comp ce id) ** spure (alignof_comp ce id | tofs) ** MP)).
+    { eapply sep_imp; [exact MPRED_RANGE1 | apply massert_imp_refl | exact IMP_SP]. }
+    assert (IH_ENUM: forall fid0 base0 fofs0 ffp0, In (fid0, ((base0, fofs0), ffp0)) fpl_enum ->
+        forall tb0 tofs0 sb0 sofs0 mp10 mp20 MP0 m1_src0 m10 m20 bytes0 ty0 te0,
+        sem_wt_loc ce ffp0 sb0 sofs0 mp10 ->
+        massert_imp mp20 (range tb0 tofs0 (tofs0 + sizeof_footprint ce ffp0)) ->
+        (alignof_footprint ce ffp0 | tofs0) ->
+        m1_src0 |= mp10 ->
+        m10 |= mp20 ** MP0 ->
+        Mem.loadbytes m1_src0 sb0 sofs0 (sizeof_footprint ce ffp0) = Some bytes0 ->
+        Mem.storebytes m10 tb0 tofs0 bytes0 = Some m20 ->
+        wt_footprint ce te0 ty0 ffp0 ->
+        exists mass3, sem_wt_loc ce ffp0 tb0 tofs0 mass3 /\ m20 |= mass3 ** MP0).
+    { intros fid0 base0 fofs0 ffp0 IN0. simpl in IN0. destruct IN0 as [EQtag | [EQvariant | Hfalse]].
+      - inv EQtag. intros tb0 tofs0 sb0 sofs0 mp10 mp20 MP0 m1_src0 m10 m20 bytes0 ty0 te0 WTLOC0 RANGE0 AL0 MPRED_SRC0 MPRED0 LOAD0 STORE0 WTFP0.
+        eapply storebytes_scalar_sem_wt_loc; eauto.
+      - inv EQvariant. intros tb0 tofs0 sb0 sofs0 mp10 mp20 MP0 m1_src0 m10 m20 bytes0 ty0 te0 WTLOC0 RANGE0 AL0 MPRED_SRC0 MPRED0 LOAD0 STORE0 WTFP0.
+        pose proof (wt_footprint_size_eq ce ty0 ffp0 te0 WTFP0) as SIZEEQ0.
+        rewrite <- SIZEEQ0 in RANGE0. rewrite <- SIZEEQ0 in LOAD0.
+        eapply (IHenum tb0 tofs0 sb0 sofs0 mp10 mp20 MP0 m1_src0 m10 m20 bytes0 ty0 te0); eauto.
+      - destruct Hfalse. }
+    assert (FIELDS: exists mass3F, (fields_loc_sep tb tofs (sem_wt_loc ce) fpl_enum mass3F /\
+                m1' |= mass3F ** (range tb (tofs + SZ) (tofs + sizeof_comp ce id) ** spure (alignof_comp ce id | tofs) ** MP))).
+    { eapply (storebytes_fields_loc_sep ce fpl_enum tb tofs sb sofs (range sb sofs sofs ** (hasvalue Mint32 sb sofs (Vint (Int.repr tagz))) ** (range sb (sofs + size_chunk Mint32) (sofs + fofs) ** mass2 ** STrue)) (range tb tofs (tofs + SZ)) (range tb (tofs + SZ) (tofs + sizeof_comp ce id) ** spure (alignof_comp ce id | tofs) ** MP) m1_src m1 m1' bytesF te SZ); eauto. }
+    destruct FIELDS as [mass3F [FSEP MPRED_FIELDS]].
+    (* store the tail padding *)
+    assert (WF_ENUM_ALIGNED: Forall (fp_field_in_range_aligned ce SZ (alignof_comp ce id) (fields_fp_well_formed ce)) fpl_enum).
+    { unfold fpl_enum, tag_fp.
+      constructor.
+      apply fp_field_in_range_aligned_intro; [lia | lia | lia | | | apply fp_scalar_wf].
+      unfold SZ. simpl. lia.
+      apply Z.divide_0_r.
+      constructor.
+      apply fp_field_in_range_aligned_intro; [simpl; lia | simpl; exact LE4 | lia | | | apply (wt_footprint_fields_well_formed ce te fty fp1 CONS NOREP WT)].
+      unfold SZ. reflexivity.
+      pose proof (wt_footprint_align_divides ce fty fp1 te WT) as ALIGNDIVF.
+      apply Z.divide_trans with (alignof ce fty').
+      rewrite <- ALIGNEQTY. exact ALIGNDIVF.
+      exact ALIGNV.
+      constructor. }
+    assert (FSEP_BOUNDED: forall b0 ofs0, m_footprint mass3F b0 ofs0 -> ~ (b0 = tb /\ (tofs + SZ) <= ofs0 <  (tofs + sizeof_comp ce id))).
+    { intros. intro. eapply MPRED_FIELDS. eauto. simpl. left. auto. }
+
+    (* { eapply (fields_loc_sep_footprint_bounded ce fpl_enum tb tofs mass3F SZ (alignof_comp ce id)); eauto. *)
+    (*   intros fid0 base0 fofs0 ffp0 IN0. simpl in IN0. destruct IN0 as [EQtag | [EQvariant | Hfalse]]. *)
+    (*   - inv EQtag. split. *)
+    (*     + simpl. lia. *)
+    (*     + intros b0 ofs0 m' WTLOC0 FOOT0. *)
+    (*       assert (WTFPtag: wt_footprint ce te type_int32s tag_fp). *)
+    (*       { unfold tag_fp. eapply wt_fp_scalar; reflexivity. } *)
+    (*       assert (WFtag: fields_fp_well_formed ce tag_fp). *)
+    (*       { unfold tag_fp. apply (fp_scalar_wf ce Mint32 (Vint (Int.repr tagz))). } *)
+    (*       exact (sem_wt_loc_footprint_bounded ce te type_int32s tag_fp CONS NOREP WTFPtag WFtag tb (tofs + 0) m' WTLOC0 b0 ofs0 FOOT0). *)
+    (*   - inv EQvariant. split. *)
+    (*     + exact FPOS. *)
+    (*     + intros b0 ofs0 m' WTLOC0 FOOT0. *)
+    (*       assert (WF1: fields_fp_well_formed ce ffp0) by (apply (wt_footprint_fields_well_formed ce te fty ffp0 CONS NOREP WT)). *)
+    (*       exact (sem_wt_loc_footprint_bounded ce te fty ffp0 CONS NOREP WT WF1 tb (tofs + fofs0) m' WTLOC0 b0 ofs0 FOOT0). *)
+    (*   - destruct Hfalse. } *)
+    assert (MPRED_FIELDS_M2: m2 |= mass3F ** (range tb (tofs + SZ) (tofs + sizeof_comp ce id) ** spure (alignof_comp ce id | tofs) ** MP)).
+    { eapply sep_preserved. exact MPRED_FIELDS.
+      - intros HF. apply (m_invar mass3F) with (m := m1'); [exact HF |].
+        eapply Mem.storebytes_unchanged_on; eauto.
+        intros i IN. intro HCONTR.
+        eapply FSEP_BOUNDED. eauto. lia.
+        (* destruct (FSEP_BOUNDED tb i HCONTR) as [BND | NEQ]. *)
+        (* + destruct BND as [EQ2 LO HI]. lia. *)
+        (* + contradiction. *)
+      - intros HQ. eapply sep_preserved; [exact HQ | |].
+        + intros H1. eapply storebytes_range_unchanged; eauto.
+        + intros HMP0. eapply (m_invar (spure (alignof_comp ce id | tofs) ** MP)) with (m := m1'). exact HMP0.
+          eapply Mem.storebytes_unchanged_on; eauto.
+          intros i IN. intro HF.
+          destruct MPRED as (MP2PRED & MPPRED0 & DISJ).
+          destruct TGT_LOC_PERM as (_ & TGTRANGE_FP).
+          destruct HF as [HFS | HFMP].
+          * unfold spure in HFS. simpl in HFS. contradiction.
+          * apply (DISJ tb i).
+            -- apply (TGTRANGE_FP tb i). simpl. split; [reflexivity |]. rewrite LEN_T in IN. lia.
+            -- exact HFMP. }
+    (* invert the target fields_loc_sep *)
+    unfold fpl_enum, tag_fp in FSEP.
+    inv FSEP.
+    inv IND.
+    exists (mass3F ** range tb (tofs + SZ) (tofs + sizeof_comp ce id) ** spure (alignof_comp ce id | tofs)).
+    split.
+    + eapply (sem_wt_enum ce fp1 tb tofs tagz fid fofs id (hasvalue Mint32 tb tofs (Vint (Int.repr tagz))) mass3 (mass3F ** range tb (tofs + SZ) (tofs + sizeof_comp ce id) ** spure (alignof_comp ce id | tofs)) (range tb (tofs + size_chunk Mint32) (tofs + fofs)) (range tb (tofs + SZ) (tofs + sizeof_comp ce id))).
+      * reflexivity.
+      * exact FWT1.
+      * reflexivity.
+      * unfold SZ. f_equal; lia.
+      * assert (BOUNDS_T: 0 <= tofs /\ tofs <= Ptrofs.modulus).
+        { destruct MPRED_RANGE0 as [RANGE_M _]. unfold range in RANGE_M. simpl in RANGE_M.
+          destruct RANGE_M as [LO [HI _]]. split; [exact LO | lia]. }
+        assert (EQV_tag: massert_eqv mass1 (hasvalue Mint32 tb tofs (Vint (Int.repr tagz)))).
+        { apply (sem_wt_loc_unique ce (fp_scalar Mint32 (Vint (Int.repr tagz))) mass1 (hasvalue Mint32 tb tofs (Vint (Int.repr tagz))) tb tofs).
+          - rewrite Z.add_0_r in FWT0. exact FWT0.
+          - apply sem_wt_scalar. reflexivity. }
+        assert (EQV_nil: massert_eqv mass4 STrue).
+        { inversion IND0; subst. assumption. }
+        rewrite EQV0, EQV1, EQV_tag, EQV_nil.
+        simpl. rewrite Z.add_0_r.
+        setoid_rewrite (range_empty_sep_l (hasvalue Mint32 tb tofs (Vint (Int.repr tagz)) ** range tb (tofs + 4) (tofs + fofs) ** mass3 ** STrue) tb tofs (proj1 BOUNDS_T) (proj2 BOUNDS_T)).
+        setoid_rewrite <- (massert_eqv_pure_r mass3).
+        rewrite !sep_assoc. reflexivity.
+    + rewrite <- (sep_assoc (range tb (tofs + SZ) (tofs + sizeof_comp ce id)) (spure (alignof_comp ce id | tofs)) MP) in MPRED_FIELDS_M2.
+      rewrite <- (sep_assoc mass3F (range tb (tofs + SZ) (tofs + sizeof_comp ce id) ** spure (alignof_comp ce id | tofs)) MP) in MPRED_FIELDS_M2.
+      exact MPRED_FIELDS_M2.
+  - inv WTFP.
+    { assert (MODE: access_mode (Treference org mut ty0) = Ctypes.By_value Mptr) by reflexivity.
+      assert (LEN_EQ: Z.of_nat (length bytes) = sizeof ce (Treference org mut ty0)).
+      { exploit Mem.loadbytes_length; eauto. intros LEN. rewrite LEN.
+        apply Z2Nat.id. apply Z.ge_le. apply sizeof_pos. }
+      assert (MPRED_HAS: m1_src |= hasvalue Mptr sb sofs (Vptr b2 (Ptrofs.repr ofs2))).
+      { rewrite EQV in MPRED_SRC. exact MPRED_SRC. }
+      exploit load_rule. exact MPRED_HAS. intros (vload & LOAD1 & HVEQ).
+      exploit Mem.load_loadbytes; eauto. intros (bytes'' & LB'' & VEQBYTES).
+      rewrite (sizeof_by_value ce (Treference org mut ty0) Mptr MODE) in LB''.
+      rewrite LOAD in LB''. inv LB''.
+      assert (ALIGN: (align_chunk Mptr | tofs)).
+      { simpl in AL. exact AL. }
+      assert (MPRED_RANGE: m1 |= range tb tofs (tofs + size_chunk Mptr) ** MP).
+      { eapply sep_imp.
+        - exact MPRED.
+        - rewrite (sizeof_by_value ce (Treference org mut ty0) Mptr MODE). exact TGT_LOC_PERM.
+        - apply massert_imp_refl. }
+      assert (MPRED_RANGE2: m2 |= range tb tofs (tofs + size_chunk Mptr) ** MP).
+      { eapply sep_preserved. exact MPRED_RANGE.
+        - intros H1. eapply storebytes_range_unchanged; eauto.
+        - intros HMP. eapply (m_invar MP).
+          + exact HMP.
+          + eapply Mem.storebytes_unchanged_on; eauto.
+            intros i IN. intro HF.
+            destruct MPRED as (MP2PRED & MPPRED0 & DISJ).
+            destruct TGT_LOC_PERM as (_ & TGTRANGE_FP).
+            unfold range in TGTRANGE_FP.
+            apply (DISJ tb i).
+            * apply (TGTRANGE_FP tb i). simpl. split; auto.
+              unfold sizeof in LEN_EQ. rewrite <- LEN_EQ. exact IN.
+            * exact HF. }
+      assert (LOAD2: Mem.load Mptr m2 tb tofs = Some (decode_val Mptr bytes'')).
+      { eapply Mem.loadbytes_load.
+        - rewrite (sizeof_by_value ce (Treference org mut ty0) Mptr MODE). rewrite <- LEN_EQ.
+          eapply Mem.loadbytes_storebytes_same; eauto.
+        - exact ALIGN. }
+      assert (VEQ: Vptr b2 (Ptrofs.repr ofs2) = decode_val Mptr bytes'').
+      { exact VEQBYTES. }
+      exists (hasvalue Mptr tb tofs (Vptr b2 (Ptrofs.repr ofs2))).
+      split.
+      econstructor. reflexivity.
+      eapply range_hasvalue.
+      exact MPRED_RANGE2.
+      rewrite <- VEQ in LOAD2. exact LOAD2. }
+    { assert (MODE: access_mode (Treference org mut ty0) = Ctypes.By_value Mptr) by reflexivity.
+      assert (LEN_EQ: Z.of_nat (length bytes) = sizeof ce (Treference org mut ty0)).
+      { exploit Mem.loadbytes_length; eauto. intros LEN. rewrite LEN.
+        apply Z2Nat.id. apply Z.ge_le. apply sizeof_pos. }
+      assert (MPRED_HAS: m1_src |= hasvalue Mptr sb sofs (Vptr b2 (Ptrofs.repr ofs2))).
+      { rewrite EQV in MPRED_SRC. exact MPRED_SRC. }
+      exploit load_rule. exact MPRED_HAS. intros (vload & LOAD1 & HVEQ).
+      exploit Mem.load_loadbytes; eauto. intros (bytes'' & LB'' & VEQBYTES).
+      rewrite (sizeof_by_value ce (Treference org mut ty0) Mptr MODE) in LB''.
+      rewrite LOAD in LB''. inv LB''.
+      assert (ALIGN: (align_chunk Mptr | tofs)).
+      { simpl in AL. exact AL. }
+      assert (MPRED_RANGE: m1 |= range tb tofs (tofs + size_chunk Mptr) ** MP).
+      { eapply sep_imp.
+        - exact MPRED.
+        - rewrite (sizeof_by_value ce (Treference org mut ty0) Mptr MODE). exact TGT_LOC_PERM.
+        - apply massert_imp_refl. }
+      assert (MPRED_RANGE2: m2 |= range tb tofs (tofs + size_chunk Mptr) ** MP).
+      { eapply sep_preserved. exact MPRED_RANGE.
+        - intros H1. eapply storebytes_range_unchanged; eauto.
+        - intros HMP. eapply (m_invar MP).
+          + exact HMP.
+          + eapply Mem.storebytes_unchanged_on; eauto.
+            intros i IN. intro HF.
+            destruct MPRED as (MP2PRED & MPPRED0 & DISJ).
+            destruct TGT_LOC_PERM as (_ & TGTRANGE_FP).
+            unfold range in TGTRANGE_FP.
+            apply (DISJ tb i).
+            * apply (TGTRANGE_FP tb i). simpl. split; auto.
+              unfold sizeof in LEN_EQ. rewrite <- LEN_EQ. exact IN.
+            * exact HF. }
+      assert (LOAD2: Mem.load Mptr m2 tb tofs = Some (decode_val Mptr bytes'')).
+      { eapply Mem.loadbytes_load.
+        - rewrite (sizeof_by_value ce (Treference org mut ty0) Mptr MODE). rewrite <- LEN_EQ.
+          eapply Mem.loadbytes_storebytes_same; eauto.
+        - exact ALIGN. }
+      assert (VEQ: Vptr b2 (Ptrofs.repr ofs2) = decode_val Mptr bytes'').
+      { exact VEQBYTES. }
+      exists (hasvalue Mptr tb tofs (Vptr b2 (Ptrofs.repr ofs2))).
+      split.
+      econstructor. reflexivity.
+      eapply range_hasvalue.
+      exact MPRED_RANGE2.
+      rewrite <- VEQ in LOAD2. exact LOAD2. }
 Admitted.
 
 
 
-(*     (SEMWTFP: sem_wt_fp ce sfp mp2) *)
-(*     (* FIXME: since clear_footprint_rec would clear the value *)
-(*     information in this location, we cannot use former proof strategy *)
-(*     anymore. *) *)
-(*     (SHALLOW: sem_wt_loc ce (clear_footprint_rec ce sfp) sb sofs mp3) *)
-(*     (* (WTVALLOC : sem_wt_loc ce sfp sb sofs (mp2 ** mp3)) *) *)
-(*     (* We prove a more general version without WTLOC of (tb, tofs), *)
-(*     meaning that we do not care what footprint was in the target *)
-(*     location (which would be overwritten after storing the bytes, so *)
-(*     it is also safe to drop its footprint). We just need to know that *)
-(*     the target location is storable and aligned. *) *)
-(*     (RANGE: massert_imp mp1 (range tb tofs (tofs + sizeof_footprint ce sfp))) *)
-(*     (AL: (alignof_footprint ce sfp | tofs)) *)
-(*     (MPIMP: massert_imp (mp1 ** MP) mp3) *)
-(*     (MPRED : m1 |= mp1 ** mp2 ** MP) *)
-(*     (LOAD: Mem.loadbytes m1 sb sofs (sizeof_footprint ce sfp) = Some bytes) *)
-(*     (* since (sb, sofs) is sem_wt_loc, the progress of storebytes is *)
-(*     straightforward *) *)
-(*     (STORE: Mem.storebytes m1 tb tofs bytes = Some m2) *)
-(*     (WF: fields_fp_well_formed ce sfp), *)
-(*   exists (mass3 : massert), *)
-(*       sem_wt_loc ce sfp tb tofs mass3 /\ m2 |= mass3 ** MP. *)
-(* Proof. *)
-(*   induction sfp using strong_footprint_ind; intros; inv WF. *)
-(*   - erewrite Mem.loadbytes_empty in LOAD. 2: simpl; try lia. *)
-(*     inv LOAD. *)
-(*     exploit Mem.storebytes_empty; eauto. intros. subst. *)
-(*     exists STrue. split. econstructor. reflexivity. *)
-(*     eapply sepconj_morph_1. 3: eapply MPRED. *)
-(*     rewrite massert_eqv_pure_r. eapply massert_imp_proj2. *)
-(*     eapply massert_imp_proj2. *)
-(*   - exists ((range tb tofs (tofs + sizeof_footprint ce (fp_uninit sz al))) ** (spure (alignof_footprint ce (fp_uninit sz al) | tofs))). *)
-(*     split. econstructor. reflexivity. *)
-(*     rewrite RANGE in MPRED. eapply sep_drop2 in MPRED. *)
-(*     assert (MPRED1: m1 |= range tb tofs (tofs + sizeof_footprint ce (fp_uninit sz al)) ** spure (alignof_footprint ce (fp_uninit sz al) | tofs) ** MP). *)
-(*     { rewrite sep_swap. *)
-(*       rewrite <- massert_eqv_prop_l; auto. } *)
-(*     rewrite sep_assoc. *)
-(*     eapply sep_preserved. eauto. intros. eapply storebytes_range_unchanged; eauto. *)
-(*     intros. eapply m_invar. eauto. *)
-(*     eapply Mem.storebytes_unchanged_on. eauto. *)
-(*     intros. intro. simpl in H1.  *)
-(*     destruct H1; try contradiction. *)
-(*     eapply MPRED; eauto. simpl.  *)
-(*     admit. *)
-(*   (* TODO: scalar,box and ref may share same proof structure. Maybe we *)
-(*   should write a lemma for them *) *)
-(*   - inv SHALLOW.  *)
-(*     (* We cannot use store_sem_wt_val to prove this lemma because we *)
-(*     only know (decode_val bytes = v) from MPRED and LOAD, but [store] *)
-(*     operation in store_sem_wt_val would store [encode_val v] into the *)
-(*     memory which may not equal to [bytes]. We can use *)
-(*     [Mem.load_loadbytes] to prove [v = decode_val bytes], *)
-(*     [Mem.loadbytes_storebytes_same] to prove that bytes loaded from m2 *)
-(*     at (tb, tofs) is [bytes], and [Mem.loadbytes_load] to prove value *)
-(*     loaded from m2 at (tb, tofs) is [v], which can derive [hasvalue] *) *)
-(*     assert (LOAD': Mem.load chunk m1 sb sofs = Some v) by admit. *)
-(*     exploit Mem.load_loadbytes; eauto. intros (bytes' & LOAD'' & VEQ).  *)
-(*     simpl in LOAD. *)
-(*     rewrite LOAD'' in LOAD. inv LOAD. *)
-(*     exploit Mem.loadbytes_storebytes_same; eauto. intros LOAD2. *)
-(*     assert (SZEQ: Z.of_nat (length bytes) = size_chunk chunk) by admit. *)
-(*     rewrite SZEQ in *. *)
-(*     exploit Mem.loadbytes_load; eauto. intros LOAD2'. *)
-(*     (* prove m1 |= hasvalue tb tofs v *) *)
-(*     rewrite RANGE in MPRED. *)
-(*     eapply (sep_preserved m1 m2) in MPRED as MPRED1. *)
-(*     exploit range_hasvalue. eapply MPRED1. eauto. intros MPRED2. *)
-(*     exists (hasvalue chunk tb tofs (decode_val chunk bytes)). split. *)
-(*     econstructor. reflexivity. eapply sep_drop2 in MPRED2. eauto. *)
-(*     (* range unchanged *) *)
-(*     intros. eapply storebytes_range_unchanged; eauto. *)
-(*     (* frame-preserving update *) *)
-(*     intros. eapply m_invar. eauto. *)
-(*     eapply Mem.storebytes_unchanged_on. eauto. *)
-(*     intros. simpl. intro. rewrite SZEQ in *.  *)
-(*     eapply MPRED. simpl. split; eauto.  *)
-(*     simpl. eauto.  *)
-(*   (* similar to fp_scalar, but we need to consider the value footprint (mp2) *) *)
-(*   - inv SHALLOW.  *)
-(*     assert (LOAD': Mem.load Mptr m1 sb sofs = Some (Vptr b Ptrofs.zero)) by admit. *)
-(*     exploit Mem.load_loadbytes; eauto. intros (bytes' & LOAD'' & VEQ).  *)
-(*     simpl in LOAD. *)
-(*     rewrite LOAD'' in LOAD. inv LOAD. *)
-(*     exploit Mem.loadbytes_storebytes_same; eauto. intros LOAD2. *)
-(*     assert (SZEQ: Z.of_nat (length bytes) = size_chunk Mptr) by admit. *)
-(*     rewrite SZEQ in *. *)
-(*     exploit Mem.loadbytes_load; eauto. intros LOAD2'. *)
-(*     (* prove m1 |= hasvalue tb tofs v *) *)
-(*     generalize MPRED as MPRED'. intros. *)
-(*     rewrite RANGE in MPRED. *)
-(*     eapply (sep_preserved m1 m2) in MPRED as MPRED1. *)
-(*     exploit range_hasvalue. eapply MPRED1. eauto. intros MPRED2.  *)
-(*     (* get the structure of mp2 *) *)
-(*     inv SEMWTFP.  *)
-(*     exists (hasvalue Mptr tb tofs (decode_val Mptr bytes) ** mp2). *)
-(*     split. *)
-(*     econstructor; eauto. rewrite VEQ. reflexivity. rewrite sep_assoc. eapply MPRED2. *)
-(*     (* range unchanged *) *)
-(*     intros. eapply storebytes_range_unchanged; eauto. *)
-(*     (* frame-preserving update *) *)
-(*     intros. eapply m_invar. eauto. *)
-(*     eapply Mem.storebytes_unchanged_on. eauto. *)
-(*     intros. simpl. intro. rewrite SZEQ in *.  *)
-(*     eapply MPRED. simpl. split; eauto.  *)
-(*     simpl. eauto.  *)
-(*   (* fp_struct: we need a premise to ensure that all fields are within *)
-(*   the range of this struct *) *)
-(*   - simpl in RANGE.  *)
-(*     (* alignment (alignof_comp ce id | tofs) can be proved by WTLOC as *)
-(*     (alignof_footprint tfp) is equal to (alignof_comp ce id) *) *)
-(*     inv SEMWTFP. inv SHALLOW. *)
-(*     rewrite EQV in MPRED.  *)
-(*     (** storebytes_fields_loc_sep: the most difficult part of *)
-(*     storebytes rules: Proof strategy: split mass and (range tb tofs) *)
-(*     into fields. Then we can split the loadbytes and storebytes into *)
-(*     sequence of loadbytes/storebytes *) *)
-(*     exploit storebytes_fields_loc_sep; eauto. *)
-(*     etransitivity. eauto. rewrite EQV0. eapply massert_imp_proj1. *)
-(*     inv WF. eauto. *)
-(*     intros (mass3 & FLOCSEP & MPRED2). *)
-(*     exists mass3. *)
-(*     split. econstructor; eauto.  *)
-(*     eapply massert_eqv_prop_r. auto. auto. *)
-(*   - admit. *)
-(*   - admit. *)
-(*   - inv SEMWTFP. *)
-(* Admitted. *)
+Lemma storebytes_sem_wt_loc ce: forall sfp tb tofs sb sofs mp1 mp2 MP m1_src m1 m2 bytes ty te
+    (CONS: composite_env_consistent ce)
+    (NOREP: forall id co, ce ! id = Some co -> list_norepet (name_members (co_members co)))
+    (SRC_LOC: sem_wt_loc ce sfp sb sofs mp1)
+    (TGT_LOC_PERM: massert_imp mp2 (range tb tofs (tofs + sizeof ce ty)))
+    (AL: (alignof ce ty | tofs))
+    (MPRED_SRC: m1_src |= mp1)
+    (MPRED: m1 |= mp2 ** MP)
+    (LOAD: Mem.loadbytes m1_src sb sofs (sizeof ce ty) = Some bytes)
+    (STORE: Mem.storebytes m1 tb tofs bytes = Some m2)
+    (WTFP: wt_footprint ce te ty sfp),
+  exists mass3, sem_wt_loc ce sfp tb tofs mass3 /\ m2 |= mass3 ** MP.
+Proof.
+  intros.
+  assert (AL_FP: (alignof_footprint ce sfp | tofs)).
+  { eapply Z.divide_trans; [eapply wt_footprint_align_divides; eauto | exact AL]. }
+  eapply storebytes_sem_wt_loc_fp; eauto.
+Qed.
 
+
+
+Lemma PTree_remove_elements_eq {A: Type}: forall id (v: A) m,
+    PTree.elements (PTree.remove id m) =
+    PTree.elements (PTree.remove id (PTree.set id v m)).
+Proof.
+  intros.
+  eapply PTree.elements_extensional.
+  intros. rewrite !PTree.grspec.
+  destruct PTree.elt_eq; subst; auto.
+  rewrite PTree.gso; auto.
+Qed.
+
+
+End ADT_ENV.
+
+Coercion fpm_to_env : fp_map >-> env.
+
+
+Lemma sem_wt_loc_range_perm ce: forall fp mass b ofs ty fpm
+      (CONS: composite_env_consistent ce)
+      (NOREP: forall id co, ce ! id = Some co -> list_norepet (name_members (co_members co)))
+      (WTFP: wt_footprint ce fpm ty fp)
+      (RANGE: 0 <= ofs /\ ofs + sizeof ce ty <= Ptrofs.max_unsigned)
+      (WTLOC: sem_wt_loc ce fp b ofs mass),
+    massert_imp mass (range b ofs (ofs + sizeof ce ty)).
+Proof.
+  intros fp mass b ofs ty fpm CONS NOREP WTFP RANGE WTLOC.
+  revert mass b ofs ty fpm WTFP RANGE WTLOC.
+  induction fp as [| sz al | chunk v | b1 fp1 IHbox | id fpl IHfields | id tagz fid fofs fp1 IHenum | mut b1 ofs1 ph0 vs] using strong_footprint_ind;
+    intros mass b ofs ty fpm WTFP RANGE WTLOC; inv WTLOC.
+  - inv WTFP.
+  - rewrite EQV. inv WTFP. eapply massert_imp_proj1.
+  - rewrite EQV. inv WTFP.
+    eapply massert_imp_trans.
+    { eapply contains_range.
+      destruct RANGE as [A B].
+      rewrite <- (sizeof_by_value ce ty chunk MODE) in B.
+      unfold Ptrofs.max_unsigned in B. unfold Ptrofs.modulus in B. unfold Ptrofs.modulus. lia. }
+    { rewrite (sizeof_by_value ce ty chunk MODE). reflexivity. }
+  - rewrite EQV. inv WTFP.
+    eapply massert_imp_trans.
+    { eapply massert_imp_proj1. }
+    { eapply massert_imp_trans.
+      { eapply contains_range.
+        assert (MODE: access_mode (Tbox ty0) = Ctypes.By_value Mptr) by reflexivity.
+        destruct RANGE as [A B].
+        rewrite <- (sizeof_by_value ce (Tbox ty0) Mptr MODE) in B.
+        unfold Ptrofs.max_unsigned in B. unfold Ptrofs.modulus in B. unfold Ptrofs.modulus. lia. }
+      { assert (MODE: access_mode (Tbox ty0) = Ctypes.By_value Mptr) by reflexivity.
+        rewrite (sizeof_by_value ce (Tbox ty0) Mptr MODE). reflexivity. } }
+  - assert (FPWF: fields_fp_well_formed ce (fp_struct id fpl)) by (eapply wt_footprint_fields_well_formed; eauto).
+    inv WTFP. inv FPWF.
+    assert (SIZEEQ_STRUCT: sizeof ce (Tstruct orgs id) = sizeof_comp ce id).
+    { unfold sizeof, sizeof_comp. rewrite CO. reflexivity. }
+    rewrite SIZEEQ_STRUCT in *.
+    set (tail := range b (ofs + sizeof_struct_comp ce id) (ofs + sizeof_comp ce id)) in *.
+    eapply fields_loc_sep_range_perm with (mp1 := tail ** spure (alignof_comp ce id | ofs)) (mp2 := mass0) (mp := mass).
+    { intros fid0 base0 fofs0 ffp0 IN0 mass0' WT0.
+      destruct (fp_match_field_In_wt ce co (wt_footprint ce fpm) fpl (co_members co) fid0 base0 fofs0 ffp0 MATCH IN0) as [fty WTFP0].
+      assert (SIZEEQ_F: sizeof ce fty = sizeof_footprint ce ffp0) by (eapply wt_footprint_size_eq; eauto).
+      eapply Forall_forall in FWF; eauto.
+      inv FWF.
+      assert (RANGEF: 0 <= ofs + fofs0 /\ (ofs + fofs0) + sizeof ce fty <= Ptrofs.max_unsigned).
+      { destruct RANGE as [A B]. split.
+        - lia.
+        - rewrite SIZEEQ_F. lia. }
+      pose proof (IHfields fid0 base0 fofs0 ffp0 IN0 mass0' b (ofs + fofs0) fty fpm WTFP0 RANGEF WT0) as Hfield.
+      rewrite SIZEEQ_F in Hfield. exact Hfield. }
+    exact FWF.
+    { intros ofs1 IN. destruct (COMPLETE ofs1 IN) as [FIELD | TAIL].
+      - left. exact FIELD.
+      - right.
+        eapply massert_imp_trans.
+        eapply massert_imp_proj1.
+        eapply range_impl; unfold tail; lia. }
+    exact RANGE.
+    exact FWT.
+    { subst. unfold tail in *.
+      rewrite EQV.
+      apply sep_comm. }
+  - assert (FPWF: fields_fp_well_formed ce (fp_enum id tagz fid fofs fp1)) by (eapply wt_footprint_fields_well_formed; eauto).
+    inv FPWF. inv FWF. inv WTFP.
+    assert (SIZEEQ_ENUM: sizeof ce (Tvariant orgs id) = sizeof_comp ce id).
+    { unfold sizeof, sizeof_comp. rewrite CO. reflexivity. }
+    rewrite SIZEEQ_ENUM in *.
+    assert (SZM: size_chunk Mint32 = 4) by reflexivity.
+    rewrite SZM in *.
+    assert (SIZEEQ_F: sizeof ce fty = sizeof_footprint ce fp1) by (eapply wt_footprint_size_eq; eauto).
+    assert (RANGEF: 0 <= ofs + fofs /\ (ofs + fofs) + sizeof ce fty <= Ptrofs.max_unsigned).
+    { destruct RANGE as [A B]. split.
+      - lia.
+      - rewrite SIZEEQ_F. lia. }
+    assert (FIELDRANGE: massert_imp mass2 (range b (ofs + fofs) (ofs + fofs + sizeof_footprint ce fp1))).
+    { rewrite <- SIZEEQ_F.
+      eapply IHenum; eauto. }
+    assert (TAGRANGE: massert_imp (hasvalue Mint32 b ofs (Vint (Int.repr tagz))) (range b ofs (ofs + size_chunk Mint32))).
+    { unfold hasvalue. eapply contains_range.
+      destruct RANGE as [A B].
+      assert (LE4: size_chunk Mint32 <= sizeof_comp ce id).
+      { assert (FPOS: 0 <= sizeof_footprint ce fp1).
+        { rewrite <- SIZEEQ_F. apply Z.ge_le. apply (sizeof_pos ce fty). }
+        lia. }
+      unfold Ptrofs.max_unsigned in *. unfold Ptrofs.modulus in *. lia. }
+    assert (JOIN_FIELD: massert_imp
+       (range b (ofs + fofs) (ofs + fofs + sizeof_footprint ce fp1) **
+        range b (ofs + fofs + sizeof_footprint ce fp1) (ofs + sizeof_comp ce id))
+       (range b (ofs + fofs) (ofs + sizeof_comp ce id))).
+    { eapply range_join. }
+    assert (JOIN_PAD: massert_imp
+       (range b (ofs + 4) (ofs + fofs) **
+        range b (ofs + fofs) (ofs + sizeof_comp ce id))
+       (range b (ofs + 4) (ofs + sizeof_comp ce id))).
+    { eapply range_join. }
+    assert (JOIN_TAG: massert_imp
+       (range b ofs (ofs + 4) **
+        range b (ofs + 4) (ofs + sizeof_comp ce id))
+       (range b ofs (ofs + sizeof_comp ce id))).
+    { eapply range_join. }
+    rewrite EQV.
+    eapply massert_imp_trans.
+    { eapply sepconj_morph_1; [eapply TAGRANGE |].
+      eapply sepconj_morph_1; [reflexivity |].
+      eapply sepconj_morph_1; [eapply FIELDRANGE |].
+      eapply massert_imp_proj1. }
+    eapply massert_imp_trans.
+    { eapply sepconj_morph_1; [reflexivity |].
+      eapply sepconj_morph_1; [reflexivity |].
+      eapply JOIN_FIELD. }
+    eapply massert_imp_trans.
+    { eapply sepconj_morph_1; [reflexivity |].
+      eapply JOIN_PAD. }
+    eapply JOIN_TAG.
+  - inv WTFP.
+    { rewrite EQV.
+      eapply massert_imp_trans.
+      { eapply contains_range.
+        assert (MODE: access_mode (Treference org mut ty0) = Ctypes.By_value Mptr) by reflexivity.
+        destruct RANGE as [A B].
+        rewrite <- (sizeof_by_value ce (Treference org mut ty0) Mptr MODE) in B.
+        unfold Ptrofs.max_unsigned in B. unfold Ptrofs.modulus in B. unfold Ptrofs.modulus. lia. }
+      { assert (MODE: access_mode (Treference org mut ty0) = Ctypes.By_value Mptr) by reflexivity.
+        rewrite (sizeof_by_value ce (Treference org mut ty0) Mptr MODE). reflexivity. } }
+    { rewrite EQV.
+      eapply massert_imp_trans.
+      { eapply contains_range.
+        assert (MODE: access_mode (Treference org mut ty0) = Ctypes.By_value Mptr) by reflexivity.
+        destruct RANGE as [A B].
+        rewrite <- (sizeof_by_value ce (Treference org mut ty0) Mptr MODE) in B.
+        unfold Ptrofs.max_unsigned in B. unfold Ptrofs.modulus in B. unfold Ptrofs.modulus. lia. }
+      { assert (MODE: access_mode (Treference org mut ty0) = Ctypes.By_value Mptr) by reflexivity.
+        rewrite (sizeof_by_value ce (Treference org mut ty0) Mptr MODE). reflexivity. } }
+Qed.
+
+
+Lemma store_sem_wt_loc ce: forall fp vfp b ofs mass1 mass2 v m1 MP chunk ty fpm
+    (CONS: composite_env_consistent ce)
+    (NOREP: forall id co, ce ! id = Some co -> list_norepet (name_members (co_members co)))
+    (WTLOC: sem_wt_loc ce fp b ofs mass1)
+    (WTVAL: sem_wt_val ce vfp v mass2)
+    (AL: (align_chunk chunk | ofs))
+    (MPRED: m1 |= mass1 ** mass2 ** MP)
+    (WTFP1: wt_footprint ce fpm ty fp)
+    (WTFP2: wt_footprint ce fpm ty vfp)
+    (BYVAL: access_mode ty = Ctypes.By_value chunk)
+    (RANGE: 0 <= ofs /\ ofs + sizeof ce ty <= Ptrofs.max_unsigned),
+    exists m2 mass3, 
+      Mem.store chunk m1 b ofs v = Some m2      
+      /\ sem_wt_loc ce vfp b ofs mass3
+      /\ m2 |= mass3 ** MP.
+Proof.
+  intros. eapply store_sem_wt_val; eauto.
+  eapply sep_imp. eapply MPRED.
+  erewrite sizeof_by_value.
+  eapply (sem_wt_loc_range_perm ce fp mass1 b ofs ty fpm); eauto.
+  all: eauto.
+Qed.
 
 Lemma storebytes_coherent_var: forall phl m1 ce mass1 mp1 sfp sb sofs fp1 tfp b1 ofs1 tb tofs MP ty te
+    (CONS: composite_env_consistent ce)
+    (NOREP: forall id co, ce ! id = Some co -> list_norepet (name_members (co_members co)))
+    (AL: (alignof ce ty | tofs))
     (SRC_LOC: sem_wt_loc ce sfp sb sofs mp1)
-    (* The variable address *)
     (TGT_LOC: sem_wt_loc ce fp1 b1 ofs1 mass1)
     (MPIMP: massert_imp (mass1 ** MP) mp1)
     (MPRED: m1 |= mass1 ** MP)
-    (* id may denote an external owner? *)
     (GFP: get_owner_loc_footprint phl fp1 b1 ofs1 = OK (tb, tofs, tfp))
-    (* Well formedness *)
     (WTFP1: wt_footprint ce te ty sfp)
-    (WTFP2: wt_footprint ce te ty tfp),
-    (* (ALEQ: alignof_footprint ce sfp = alignof_footprint ce tfp) *)
-    (* (SZEQ: sizeof_footprint ce sfp = sizeof_footprint ce tfp) *)
-    (* (AL: (alignof_footprint ce sfp | tofs)) *)
-    (* (WF1: fields_fp_well_formed ce sfp) *)
-    (* (WF2: fields_fp_well_formed ce tfp) *)
-    (* As we need to load bytes from sfp so it must imply range_perm *)
-    (* (OWN1: shallow_owned sfp = true) *)
-    (* (OWN2: shallow_owned tfp = true), *)
+    (WTFP2: wt_footprint ce te ty tfp)
+    (RANGE_SRC: 0 <= sofs /\ sofs + sizeof ce ty <= Ptrofs.max_unsigned)
+    (RANGE_TGT: 0 <= tofs /\ tofs + sizeof ce ty <= Ptrofs.max_unsigned),
     exists bytes m2 fp2 mass3,
       Mem.loadbytes m1 sb sofs (sizeof_footprint ce sfp) = Some bytes
       /\ Mem.storebytes m1 tb tofs bytes = Some m2
@@ -1743,147 +3642,113 @@ Lemma storebytes_coherent_var: forall phl m1 ce mass1 mp1 sfp sb sofs fp1 tfp b1
       /\ sem_wt_loc ce fp2 b1 ofs1 mass3
       /\ m2 |= mass3 ** MP.
 Proof.
-Admitted.
-(*   intros. *)
-(*   (* progress of loadbytes and storebytes *) *)
-(*   exploit sem_wt_loc_merge; eauto. intros SRCWTLOC. *)
-(*   exploit sem_wt_loc_range_perm. eapply OWN1. all: eauto.  *)
-(*   intros MIMP. *)
-(*   assert (MPRED': m1 |= mp3 ** mp2) by admit. *)
-(*   rewrite MIMP in MPRED'. *)
-(*   exploit Mem.range_perm_loadbytes.  *)
-(*   red. intros. eapply MPRED'; eauto. *)
-(*   intros (bytes & LOAD). *)
-(*   exploit Mem.loadbytes_length; eauto. intros LEN. *)
-(*   (* storebytes *) *)
-(*   exploit get_owner_loc_footprint_sem_wt_split; eauto. *)
-(*   intros (mp1 & mp1' & mp4 & fp1' & A1 & A2 & A3 & A4 & A5). *)
-(*   exploit sem_wt_loc_range_perm. eapply OWN2. all: eauto.  *)
-(*   intros MIMP2. *)
-(*   assert (MPRED1: m1 |= mp4). rewrite A4 in MPRED. eapply MPRED. *)
-(*   rewrite MIMP2 in MPRED1. *)
-(*   edestruct Mem.range_perm_storebytes with (b:= tb) (ofs := tofs) as (m2 & STORE). *)
-(*   red. intros. eapply MPRED1; eauto. rewrite <- SZEQ. rewrite LEN in *. *)
-(*   rewrite Z_to_nat_max in H.  *)
-(*   (* show sizeof_footprint is positive *) *)
-(*   admit. *)
-(*   exploit (storebytes_sem_wt_loc ce sfp tb tofs sb sofs mp4 mp2 mp3 (mp1 ** mp1' ** MP)); eauto.  *)
-(*   rewrite SZEQ. auto.  *)
-(*   rewrite A4 in MPIMP.  *)
-(*   (* prove by MPIMP *) *)
-(*   admit. *)
-(*   rewrite A4 in MPRED.  *)
-(*   (* prove by MPRED *) *)
-(*   admit. *)
-(*   intros (mass3 & B1 & B2). *)
-(*   exploit A5; eauto.  *)
-(*   eapply shallow_owned_not_emp; eauto. *)
-(* intros (mp' & fp1'' & SET & C1 & C2).   *)
-(*   exists bytes, m2, fp1'', mp'.  *)
-(*   do 4 (try apply conj); eauto. *)
-(*   rewrite C2. admit. *)
-(* Admitted. *)
+  intros.
+  assert (SIZEEQ1: sizeof_footprint ce sfp = sizeof ce ty).
+  { symmetry. eapply (wt_footprint_size_eq ce ty sfp te). exact WTFP1. }
+  assert (SIZEEQ2: sizeof_footprint ce tfp = sizeof ce ty).
+  { symmetry. eapply (wt_footprint_size_eq ce ty tfp te). exact WTFP2. }
+
+  exploit (get_owner_loc_footprint_sem_wt_split ce phl b1 ofs1 tb tofs fp1 tfp mass1); eauto.
+  intros (rest & lost & tgt_mass & fp1' & SET_EMP & REST_LOC & TGT_LOC2 & SPLIT & RE_SET).
+
+  exploit (sem_wt_loc_range_perm ce sfp mp1 sb sofs ty te); eauto.
+  intros SRC_RANGE.
+  exploit (sem_wt_loc_range_perm ce tfp tgt_mass tb tofs ty te); eauto.
+  intros TGT_RANGE.
+
+  rewrite SPLIT in MPRED.
+  rewrite SPLIT in MPIMP.
+  rewrite !sep_assoc in MPRED.
+  rewrite !sep_assoc in MPIMP.
+
+  assert (MPRED_SRC: m1 |= mp1).
+  { eapply MPIMP. exact MPRED. }
+
+  assert (MPRED_RANGE_SRC: m1 |= range sb sofs (sofs + sizeof ce ty)).
+  { eapply SRC_RANGE. exact MPRED_SRC. }
+
+  assert (LOAD: exists bytes, Mem.loadbytes m1 sb sofs (sizeof_footprint ce sfp) = Some bytes).
+  { rewrite SIZEEQ1.
+    eapply Mem.range_perm_loadbytes.
+    red. intros i IN.
+    destruct MPRED_RANGE_SRC as (LO & HI & PERM).
+    apply PERM. simpl. repeat split; auto; lia. }
+  destruct LOAD as (bytes & LOAD).
+  exploit Mem.loadbytes_length; eauto. intros LEN.
+
+  assert (LEN_EQ: Z.of_nat (length bytes) = sizeof ce ty).
+  { rewrite LEN. rewrite SIZEEQ1. apply Z2Nat.id. apply Z.ge_le. apply sizeof_pos. }
+
+  assert (MPRED_TGT: m1 |= tgt_mass).
+  { apply (sep_proj1 MP tgt_mass m1).
+    apply (sep_proj2 lost (tgt_mass ** MP) m1).
+    apply (sep_proj2 rest (lost ** (tgt_mass ** MP)) m1).
+    exact MPRED. }
+
+  assert (MPRED_RANGE_TGT: m1 |= range tb tofs (tofs + sizeof ce ty)).
+  { eapply TGT_RANGE. exact MPRED_TGT. }
+
+  assert (STORE: exists m2, Mem.storebytes m1 tb tofs bytes = Some m2).
+  { edestruct (Mem.range_perm_storebytes m1 tb tofs bytes) as (m2 & STORE0).
+    - rewrite LEN_EQ.
+      red. intros i IN.
+      destruct MPRED_RANGE_TGT as (LO & HI & PERM).
+      apply PERM. simpl. repeat split; auto; lia.
+    - exists m2. exact STORE0. }
+  destruct STORE as (m2 & STORE).
+
+  assert (EQ_MPRED: massert_eqv (rest ** lost ** tgt_mass ** MP) (tgt_mass ** rest ** lost ** MP)).
+  { rewrite (sep_swap3 rest lost tgt_mass MP).
+    rewrite (sep_swap23 tgt_mass lost rest MP).
+    reflexivity. }
+  rewrite EQ_MPRED in MPRED.
+  rewrite EQ_MPRED in MPIMP.
+
+  assert (LOAD_TY: Mem.loadbytes m1 sb sofs (sizeof ce ty) = Some bytes).
+  { rewrite <- SIZEEQ1. exact LOAD. }
+
+  exploit (storebytes_sem_wt_loc ce sfp tb tofs sb sofs mp1 tgt_mass (rest ** lost ** MP) m1 m1 m2 bytes ty te); eauto.
+  intros (mass3 & B1 & B2).
+
+  exploit (RE_SET sfp mass3); eauto. intros (mp' & fp2 & SET2 & C1 & C2).
+
+  exists bytes, m2, fp2, mp'.
+  split. exact LOAD.
+  split. exact STORE.
+  split. exact SET2.
+  split. exact C1.
+  rewrite C2.
+  assert (EQ_FINAL: massert_eqv (mass3 ** rest ** lost ** MP) ((rest ** lost ** mass3) ** MP)).
+  { rewrite (sep_swap3 mass3 rest lost MP).
+    rewrite (sep_swap lost rest (mass3 ** MP)).
+    rewrite !sep_assoc.
+    reflexivity. }
+  rewrite <- EQ_FINAL. exact B2.
+Qed.
 
 
-(*   (** We may use get_owner_loc_footprint_sem_wt_split to prove this *)
-(*   lemma, instead of doing induction on phl like *)
-(*   store_coherent_var. But the difficult part is how to write a *)
-(*   set_footprint rule after storing the bytes and prove sem_wt_loc *)
-(*   again? *) *)
-(*   (* assert (CLR: exists fp1', clear_owner_footprint ce fp1 phl = Some fp1') by admit. *) *)
-(*   (* destruct CLR as (fp1' & CLR). *) *)
-(*   (* exploit get_owner_loc_footprint_sem_wt_split; eauto. *) *)
-(*   (* intros (mp1 & mp4 & mp5 & A1 & A2 & A3 & A4). *) *)
-(*   (* assert (LOAD: exists bytes, Mem.loadbytes m1 sb sofs (sizeof_footprint ce sfp) = Some bytes) by admit. *) *)
-(*   (* destruct LOAD as (bytes & LOAD). *) *)
-(*   (* assert (STORE: exists m2, Mem.storebytes m1 tb tofs bytes = Some m2) by admit. *) *)
-(*   (* destruct STORE as (m2 & STORE). *) *)
-(*   (* exploit (storebytes_sem_wt_loc ce sfp tb tofs sb sofs mp4 mp2 mp3 (mp1 ** mp5 **  MP)); eauto.  *) *)
-(*   (* admit.  admit. admit. intros (mass3 & B1 & B2). *) *)
-(*   (* (** TODO: set_ootprint *) *)   *)
-(*   induction phl; intros. *)
-(*   - inv GFP.  *)
-(*     (* use storebytes_sem_wt_loc *) *)
-(*     admit. *)
-(*   (* similar to store_coherent_var *) *)
-(*   - simpl in GFP. destruct a; try congruence. *)
-(*     + destr_fp_box fp1 GFP. *)
-(*       inv WTLOC. rewrite EQV in *. rewrite FREE in *. *)
-(*       set (MP1 := hasvalue Mptr b1 ofs1 (Vptr b Ptrofs.zero)) in *. *)
-(*       unfold box_pred in *. rewrite SHALLOW0 in *. *)
-(*       set (MP2 := contains_neg Mptr b (- size_chunk Mptr) (eq (Vptrofs (Ptrofs.repr sz)))) in *. *)
-(*       (* prove it with commutative lemmas of sepconj *) *)
-(*       assert (MPRED1: m1 |= nextmp ** mp2 ** (MP ** MP1 ** MP2)) by admit.       *)
-(*       exploit IHphl. eapply SEMWTFP.  all: eauto. admit. *)
-(*       intros (bytes & m2 & fp2 & mass3 & A1 & A2 & A3 & A4 & A5). *)
-(*       exists bytes, m2, (fp_box b sz fp2), (MP1 ** box_pred fp2 b sz mass3). *)
-(*       do 4 (try apply conj); eauto. *)
-(*       * simpl. rewrite A3. reflexivity. *)
-(*       * econstructor; eauto.  *)
-(*       * unfold box_pred. destruct (shallow_init fp2). admit. admit.                *)
-(*     + destr_fp_field fp1 GFP. *)
-(*       inv WTLOC. rewrite EQV in *. *)
-(*       (* split fields_sep *) *)
-(*       exploit fields_loc_sep_find_set; eauto. *)
-(*       intros (mp1 & mp4 & mpi & l1 & l2 & A1 & A2 & A3 & A4 & A5 & A6). subst. *)
-(*       eapply mconj_proj1 in MPRED as MPRED1. *)
-(*       (* change only mpi *) *)
-(*       assert (MPRED1': m1|= mpi ** mp4 ** mp1 ** mp2 ** MP) by admit.       *)
-(*       exploit IHphl. eapply SEMWTFP. eapply SHALLOW.  *)
-(*       massert_imp *)
-(* eapply  *)
+(* [storebytes_coherent_fpm]: storing bytes from [sfp] into the owner
+   location [(id, phl)] of [fpm] succeeds and updates [fpm] with [sfp] while
+   preserving [coherent_fpm]. The proof splits [coherent_fpm] around the target
+   variable, reframes the memory assertion, applies [storebytes_coherent_var],
+   and reassembles the updated footprint map. *)
 
-(* all: eauto. *)
-(*       intros (bytes & m2 & fp2 & mpi' & C1 & C2 & C3 & C4 & C5). *)
-(*       (* adhoc: we know that storing a location does not change its *)
-(*       permission. *) *)
-(*       assert (MPRED2: m1 |= range b1 ofs1 (ofs1 + sizeof_comp ce id)) by eapply MPRED. *)
-(*       eapply storebytes_range_unchanged in MPRED2 as MPRED2'; eauto.       *)
-(*       rewrite <- sep_assoc in MPRED. rewrite (mconj_absorb1 _ _ mass2) in MPRED.       *)
-(*       exploit frame_mconj. eapply MPRED.  *)
-(*       rewrite <- !sep_assoc in C5. *)
-(*       eapply C5. eauto. intros MPRED3. *)
-(*       rewrite sep_assoc, (sep_swap mpi' mp1 _) in MPRED3. *)
-(*       exists bytes, m2, (fp_struct id (set_field_fp fid fp2 (l1 ++ (fid, (z, f)) :: l2))), (mconj (mp1 ** mpi' ** mp2) (range b1 ofs1 (ofs1 + sizeof_comp ce id))).  *)
-(*       do 4 (try apply conj); eauto. *)
-(*       simpl. rewrite FIND. rewrite C3. reflexivity. *)
-(*       econstructor; eauto. *)
-(*     + destr_fp_enum fp1 GFP. *)
-(*       inv WTLOC. *)
-(*       eapply mconj_proj1 in MPRED as MPRED1. *)
-(*       set (mass1 := hasvalue Mint32 b1 ofs1 (Vint (Int.repr tag))) in *. *)
-(*       (* change only mpi *) *)
-(*       assert (MPRED1': m1|= mass3 ** mass2 ** mass1 ** MP) by admit. *)
-(*       exploit IHphl. eapply FWT. eapply WTVAL. all: eauto. *)
-(*       intros (bytes & m2 & fp2 & mass2' & C1 & C2 & C3 & C4 & C5). *)
-(*       assert (MPRED2: m1 |= range b1 ofs1 (ofs1 + sizeof_comp ce id)) by eapply MPRED. *)
-(*       eapply storebytes_range_unchanged in MPRED2 as MPRED2'; eauto.       *)
-(*       rewrite <- sep_assoc in MPRED. rewrite (mconj_absorb1 _ _ mass2) in MPRED.       *)
-(*       exploit frame_mconj. eapply MPRED.  *)
-(*       rewrite <- !sep_assoc in C5. *)
-(*       eapply C5. eauto. intros MPRED3. *)
-(*       rewrite (sep_comm mass2' mass1) in MPRED3. *)
-(*       exists bytes, m2, (fp_enum id tag fid0 ofs fp2), (mconj (mass1 ** mass2') (range b1 ofs1 (ofs1 + sizeof_comp ce id))).  *)
-(*       do 4 (try apply conj); eauto. *)
-(*       simpl. rewrite dec_eq_true. rewrite C3. reflexivity. *)
-(*       econstructor; eauto. *)
-(* Admitted. *)
-
-(* Some work around for not defining sem_wt_bytes (which may require
- slicing bytes when defining the struct case which is complicated):
- since loading bytes and storing bytes can only happen in assign_loc,
- we can use the sem_wt_loc fact (provided by sem_wt_val for
- struct/enum footprint) of the assigner and prove that when storing
- its bytes into the assignee, the target location is sem_wt_loc. *)
+(* To use this lemma, we should first set fp_emp to the copy-out
+location to get full permission of sfp (i.e., mp1). It is inconvenient
+to use sem_wt_fp to define the footprint for the value without the
+location because we cannot define (fp_box b fp_emp) to mean it stores
+b but does not own the permission of b's allocation metadata. *)
 Lemma storebytes_coherent_fpm: forall phl m1 ce fpm mass1 mp1 sfp tfp sb sofs tb tofs id MP ty
+    (CONS: composite_env_consistent ce)
+    (NOREP: forall id co, ce ! id = Some co -> list_norepet (name_members (co_members co)))
+    (AL: (alignof ce ty | tofs))
+    (RANGE_SRC: 0 <= sofs /\ sofs + sizeof ce ty <= Ptrofs.max_unsigned)
+    (RANGE_TGT: 0 <= tofs /\ tofs + sizeof ce ty <= Ptrofs.max_unsigned)
     (SRC_LOC: sem_wt_loc ce sfp sb sofs mp1)
-    (* The variable address *)
     (COH: coherent_fpm ce fpm mass1)
     (MPIMP: massert_imp (mass1 ** MP) mp1)
     (MPRED: m1 |= mass1 ** MP)
-    (* id may denote an external owner? *)
     (GFP: get_owner_loc_footprint_map (id, phl) fpm = OK (tb, tofs, tfp))
-    (* Well formedness *)
     (WTFP1: wt_footprint ce (fpm_to_tenv fpm) ty sfp)
     (WTFP2: wt_footprint ce (fpm_to_tenv fpm) ty tfp),
     exists bytes m2 fpm1 mass3,
@@ -1893,199 +3758,98 @@ Lemma storebytes_coherent_fpm: forall phl m1 ce fpm mass1 mp1 sfp tfp sb sofs tb
       /\ coherent_fpm ce fpm1 mass3
       /\ m2 |= mass3 ** MP.
 Proof.
- (*  intros. simpl in GFP.  *)
- (*  destruct (fpm ! id) as [(((b1 & ofs1) & ty1) & fp)|] eqn: B; try congruence. *)
- (*  (* We should split the footprint for the id from mass1 *) *)
- (*  exploit coherent_fpm_split; eauto. *)
- (*  intros (l1 & l2 & mp1 & mp4 & mpi & A1 & A2 & A3 & A4 & A5). subst. *)
- (*  (* apply storebytes_coherent_var *) *)
- (*  inv A3. inv ELTEQ. *)
- (*  assert (MPRED1: m1 |= mpi ** mp2 ** (mp1 ** mp4 ** MP)) by admit. *)
- (* exploit storebytes_coherent_var. eauto. eapply SHALLOW. eapply MASS.  *)
- (*  2: eapply MPRED1. admit.      (* easy *) *)
- (*  all: eauto. *)
- (*  intros (bytes & m2 & fp2 & mass3 & B1 & B2 & B3 & B4 & B5). *)
- (*  cbn [set_footprint_map]. rewrite B. rewrite B3. *)
- (*  exists bytes, m2. *)
- (*  exists (PTree.set id0 (b, ofs, opt_reg, ty, fp2) fpm), (mass3 ** mp1 ** mp4). *)
- (*  do 4 (try eapply conj); eauto. *)
- (*  - econstructor.  *)
- (*    assert (TODO: PTree.elements (PTree.set id0 (b, ofs, opt_reg, ty, fp2) fpm) = l1 ++ (id0, (b, ofs, opt_reg, ty, fp2)) :: l2) by admit. *)
- (*    (* rewrite TODO. *) *)
- (*    (* eapply Forall_sep_app. exists mp1, (mp3 ** mp2).  *) *)
- (*    (* split; eauto. split. econstructor; eauto. *) *)
- (*    (* econstructor; eauto. reflexivity. *) *)
- (*    admit. *)
- (*  - rewrite !sep_assoc. auto. *)
-Admitted.
-
-(** TODO: assign_loc rule  *)
-
-
-(** Define functions for extracting the footprint that represents the
-locations passed by reference *)
-
-(* Assume that we have the list of argument footprints *)
-
-(* input: footprint 
-
-output: list (path, footprint) satisfying：
-
-1. all paths are disjoint
-2. (fpm, output) should satisfying that:
-  2.1 all the footprint of the path in output is fp_emp in fpm
-  2.2 when we set all the footprint of the output back to fpm, we can the original fpm
-  2.3 
-
- *)
-
-(*
-
-(* collect the owner paths stored in the leaf nodes that are fp_ref *)
-Fixpoint collect_footprint_ref_paths (fp: footprint) : list path :=
-  match fp with
-  | fp_struct _ fpl =>
-      flat_map  (fun '(_, (_, ffp)) => collect_footprint_ref_paths ffp) fpl
-  | fp_enum _ _ _ _ ffp =>
-      collect_footprint_ref_paths ffp
-  | fp_box _ fp1 =>
-      collect_footprint_ref_paths fp1
-  | fp_ref _ _ ph =>
-      ph :: nil
-  | _ => nil
-  end.
-
-Definition collect_fpm_ref_paths (fpm: fp_map) : list path :=
-  let fpl := map (fun '(_, (_, _, _, _, fp)) => fp) (PTree.elements fpm) in
-  flat_map collect_footprint_ref_paths fpl.
+  intros.
+  unfold get_owner_loc_footprint_map in GFP.
+  destruct (fpm ! id) as [(((b1, ofs1), ty1), fp1) | ] eqn:B; try discriminate.
+  inv COH.
+  exploit PTree.elements_remove. exact B. intros (l1 & l2 & ELEMS_OLD & ELEMS_REM_OLD).
+  rewrite ELEMS_OLD in ALLSEP.
+  apply Forall_sep_app in ALLSEP as (mp_l & mp_rest & SEP_L & SEP_MID & EQV_L_REST).
+  inversion SEP_MID as [| x0 l0 mhead mtail mwhole HEAD TAIL EQV_MID]; subst.
+  inv HEAD; inv ELTEQ.
+  assert (EQV_MASS1: massert_eqv mass1 (mp_l ** mhead ** mtail)).
+  { etransitivity; [exact EQV_L_REST |].
+    apply sepconj_morph_2; [reflexivity |]. symmetry. exact EQV_MID. }
+  assert (EQV_FRAME: massert_eqv ((mp_l ** mhead ** mtail) ** MP) (mhead ** (mp_l ** mtail ** MP))).
+  { rewrite (sep_assoc mp_l (mhead ** mtail) MP).
+    rewrite (sep_assoc mhead mtail MP).
+    apply sep_swap. }
+  assert (MPIMP_VAR: massert_imp (mhead ** (mp_l ** mtail ** MP)) mp1).
+  { rewrite EQV_MASS1 in MPIMP. rewrite EQV_FRAME in MPIMP. exact MPIMP. }
+  assert (MPRED_VAR: m1 |= mhead ** (mp_l ** mtail ** MP)).
+  { rewrite EQV_MASS1 in MPRED. rewrite EQV_FRAME in MPRED. exact MPRED. }
+  exploit (storebytes_coherent_var phl m1 ce mhead mp1 sfp sb sofs fp tfp b ofs tb tofs (mp_l ** mtail ** MP) ty (fpm_to_tenv fpm)); eauto.
+  intros (bytes & m2 & fp2 & mass3 & LOAD & STORE & SET_FOOT & WTLOC_FP2 & MPRED_M2).
+  remember (PTree.set id0 (b, ofs, ty0, fp2) fpm) as fpm1 eqn:FPM1.
+  assert (SET_MAP: set_footprint_map (id0, phl) sfp fpm = OK fpm1).
+  { unfold set_footprint_map. simpl. rewrite B. rewrite SET_FOOT. simpl. rewrite <- FPM1. reflexivity. }
+  assert (FPM1_GET: fpm1 ! id0 = Some (b, ofs, ty0, fp2)).
+  { rewrite FPM1. apply PTree.gss. }
+  exploit PTree.elements_remove. exact FPM1_GET. intros (l1' & l2' & ELEMS_NEW & ELEMS_REM_NEW).
+  assert (REM_ELEMS_EQ: PTree.elements (PTree.remove id0 fpm1) = PTree.elements (PTree.remove id0 fpm)).
+  { rewrite FPM1. symmetry. apply PTree_remove_elements_eq. }
+  assert (L_EQ: l1' ++ l2' = l1 ++ l2).
+  { rewrite <- ELEMS_REM_NEW. rewrite REM_ELEMS_EQ. exact ELEMS_REM_OLD. }
+  assert (SEP_OLD: Forall_sep (coherent_var ce) (l1 ++ l2) (mp_l ** mtail)).
+  { eapply Forall_sep_app. exists mp_l, mtail.
+    split; [exact SEP_L |].
+    split; [exact TAIL |].
+    apply massert_eqv_refl. }
+  assert (SEP_NEW_TAIL: Forall_sep (coherent_var ce) (l1' ++ l2') (mp_l ** mtail)).
+  { rewrite L_EQ. exact SEP_OLD. }
+  apply Forall_sep_app in SEP_NEW_TAIL as (mp_l' & mp_r' & SEP_L' & SEP_R' & EQV_LR').
+  assert (COH_NEW_HEAD: coherent_var ce (id0, (b, ofs, ty0, fp2)) mass3).
+  { econstructor; [reflexivity | exact WTLOC_FP2]. }
+  assert (SEP_NEW_MID: Forall_sep (coherent_var ce) ((id0, (b, ofs, ty0, fp2)) :: l2') (mass3 ** mp_r')).
+  { econstructor; [exact COH_NEW_HEAD | exact SEP_R' | apply massert_eqv_refl]. }
+  assert (EQV_NEW_LIST: massert_eqv (mass3 ** mp_l ** mtail) (mp_l' ** (mass3 ** mp_r'))).
+  { etransitivity; [apply sepconj_morph_2; [reflexivity | exact EQV_LR'] |].
+    apply sep_swap. }
+  assert (SEP_NEW_LIST: Forall_sep (coherent_var ce) (l1' ++ (id0, (b, ofs, ty0, fp2)) :: l2') (mass3 ** mp_l ** mtail)).
+  { eapply Forall_sep_app. exists mp_l', (mass3 ** mp_r').
+    split; [exact SEP_L' |].
+    split; [exact SEP_NEW_MID |].
+    exact EQV_NEW_LIST. }
+  assert (COH_FPM1: coherent_fpm ce fpm1 (mass3 ** mp_l ** mtail)).
+  { apply coherent_fpm_intro. rewrite ELEMS_NEW. exact SEP_NEW_LIST. }
+  exists bytes, m2, fpm1, (mass3 ** mp_l ** mtail).
+  split; [exact LOAD |].
+  split; [exact STORE |].
+  split; [exact SET_MAP |].
+  split; [exact COH_FPM1 |].
+  rewrite (sep_assoc mass3 (mp_l ** mtail) MP).
+  rewrite (sep_assoc mp_l mtail MP).
+  exact MPRED_M2.
+Qed.
 
 
-Definition get_owner_footprint_map_ref_paths (fpm: fp_map) (ph: path) : res (list path) :=
-  match get_owner_footprint_map ph fpm with
-  | Some fp =>
-      OK (collect_footprint_ref_paths fp)
-  | None =>
-      Error nil
-  end.
-
-
-(* We need to ensure that all the returned paths are disjoint, its
-located note contain deep_init footprint, and form a closure *)
-Definition collect_fpm_args_ref_paths (fpm: fp_map) (args: list footprint) : res (list path) :=
-  let not_visited := collect_fpm_ref_paths fpm in
-  let to_visit := flat_map collect_footprint_ref_paths args in
-  collect_ref_paths_generic (get_owner_footprint_map_ref_paths fpm) nil to_visit not_visited (lex_ord_lt_acc_intro _ _).
-
-Fixpoint generate_new_suffix_path_footprint (l: list path) (fp: footprint) : res footprint :=
-  match fp with
-  | fp_ref b ofs ph =>
-      do ph1 <- generate_new_suffix_path l ph;
-      OK (fp_ref b ofs ph1)
-  | fp_box b fp1 =>
-      do fp1' <- generate_new_suffix_path_footprint l fp1;
-      OK (fp_box b fp1')
-  | fp_struct id fpl =>
-      do fpl1 <- (mmap (fun '(fid, ((base, fofs), ffp)) => 
-                            do ffp1 <- generate_new_suffix_path_footprint l ffp;
-                            OK (fid, ((base, fofs), ffp1))) fpl);
-      OK (fp_struct id fpl1)
-  | fp_enum id tagz fid fofs ffp =>
-      do ffp1 <- generate_new_suffix_path_footprint l ffp;
-      OK (fp_enum id tagz fid fofs ffp1)
-  | fp_object id obj exposed =>
-      do exposed1 <- (mmap (fun '(fid, ((b, ofs), ffp)) =>
-                             do ffp1 <- generate_new_suffix_path_footprint l ffp;
-                             OK (fid, ((b, ofs), ffp1))) exposed);
-      OK (fp_object id obj exposed)
-  | _ => OK fp
-  end.
-
-(* Collect the footprints that are passed via reference to the environment *)
-Definition collect_fpm_passed_ref_footprint (fpm: fp_map) (l: list path) : res (list footprint) :=
-  mmap (fun ph => match get_owner_footprint_map ph fpm with
-              | Some fp => 
-                  do fp1 <- (generate_new_suffix_path_footprint l fp);
-                  OK fp1
-              | None =>
-                  Error nil
-              end) l.
-
-*) 
-
-
-(*
-(* The output parameters contain two parts: one for the normal
-arguments and the others are the memory locations passed via
-reference *)
-Definition generate_call_parameters (fpm: fp_map) (args: list footprint) : res (list footprint * list footprint * list path) :=
-  do extern_paths <- collect_fpm_args_ref_paths fpm args;
-  do args1 <- mmap (generate_new_suffix_path_footprint extern_paths) args;
-  do extern_fps <- collect_fpm_passed_ref_footprint fpm extern_paths;
-  OK (args1, extern_fps, extern_paths).
-
-
-(* For funciton return, we need to reset the path name of the external
-reference location to its normalized forms (i.e., the ordinal in the
-list passed by caller). We can reuse the generate_new_suffix_path_footprint
-to do this work. *)
-Definition generate_return_parameters (fpm: fp_map) (retv: footprint) (ns: list ident) : res (footprint * list footprint) :=
-  let phs := map (fun id => (id, nil)) ns in
-  do retv1 <- generate_new_suffix_path_footprint phs retv;
-  do out_params <- collect_fpm_passed_ref_footprint fpm phs;
-  OK (retv1, out_params).
-
-
-(* When receive return value/input arguments from environment, the
-current function should recover the normalized names that are passed
-to environment (or generate new names to avoid name conflict with the
-current variable names at function entry). These two kinds of
-operations can be done using recover_sval_ref_paths. *)
-
-Fixpoint recover_footprint_ref_paths (l: list path) (fp: footprint)  : res footprint :=
-  match fp with
-  | fp_ref b ofs ph =>
-      do ph1 <- recover_ref_path l ph;
-      OK (fp_ref b ofs ph1)
-  | fp_box b fp1 =>
-      do fp1' <- recover_footprint_ref_paths l fp1;
-      OK (fp_box b fp1')
-  | fp_struct id fpl =>
-      do fpl1 <- mmap (fun '(fid, ((base, fofs), ffp)) => 
-                        do ffp1 <- recover_footprint_ref_paths l ffp;
-                        OK (fid, ((base, fofs), ffp1))) fpl;
-      OK (fp_struct id fpl1)
-  | fp_enum id tagz fid fofs ffp =>
-      do ffp1 <- recover_footprint_ref_paths l ffp;
-      OK (fp_enum id tagz fid fofs ffp1)
-  | fp_object id obj exposed =>
-      do exposed1 <- mmap (fun '(fid, ((b, ofs), ffp)) => 
-                        do ffp1 <- recover_footprint_ref_paths l ffp;
-                        OK (fid, ((b, ofs), ffp1))) exposed;
-      OK (fp_object id obj exposed1)
-  | _ =>
-      OK fp
-  end.
-
-
-(* When the caller receives the returned footprint and the
-reference-passed footprint list, it updates their reference paths and
-then putback to the fpm. The caller should guarantee that the external
-footprints are normalized into the form same as those passed by the
-caller *)
-Definition receive_return_footprint (fpm: fp_map) (l: list path) (retv: footprint) (externs: list footprint) : res (footprint * fp_map) :=
-  do retv1 <- recover_footprint_ref_paths l retv;
-  do externs1 <- mmap (recover_footprint_ref_paths l) externs;
-  let phs_externs := combine l externs1 in
-  (* TODO: make get/set return res instead of option *)
-  do fpm1 <- mfold_left (fun acc '(ph, fp) => match set_footprint_map ph fp acc with
-                                         | Some acc1 => OK acc1
-                                         | None => Error nil
-                                         end) phs_externs fpm;
-  OK (retv1, fpm1).
-*) 
-
-
-
-End ADT_ENV.
-
-Coercion fpm_to_env : fp_map >-> env.
+(* Lemma assign_loc_coherent_fpm: forall phl m ce fpm mass1 mass2 v vfp pfp chunk b ofs id MP ty *)
+(*     (COH: coherent_fpm ce fpm mass1) *)
+(*     (* (WTVAL: sem_wt_val ce vfp v mass2) *) *)
+(*     (** This premises should be provided by the properties of *)
+(*     eval_expr *) *)
+(*     (MODE: match access_mode ty with *)
+(*            | Ctypes.By_value chunk =>  *)
+(*            | Ctypes.By_copy => *)
+(*                (* ensure by type checking *) *)
+               
+(*     (MPRED: m |= mass1 ** mass2 ** MP) *)
+(*     (* id may denote an external owner? We reduce all store for *)
+(*     reference into store for their referred owner *) *)
+(*     (GFP: get_owner_loc_footprint_map (id, phl) fpm = OK (b, ofs, pfp)) *)
+(*     (* The following properties should be derived from wt_footprint *) *)
+(*     (AL: (alignof ce ty | ofs)) *)
+(*     (* (MAT1: fp_match_chunk pfp chunk) *) *)
+(*     (* (MAT2: fp_match_chunk vfp chunk),     *) *)
+(*     (WTFP1: wt_footprint ce (fpm_to_tenv fpm) ty pfp) *)
+(*     (WTFP2: wt_footprint ce (fpm_to_tenv fpm) ty vfp) *)
+(*     (* (BYVAL: access_mode ty = Ctypes.By_value chunk) *) *)
+(*     (SHALLOW: shallow_init pfp = true) *)
+(*     (FPWF: fields_fp_well_formed ce pfp) *)
+(*     (RANGE: 0 <= ofs /\ ofs + sizeof ce ty <= Ptrofs.max_unsigned), *)
+(*     exists m1 fpm1 mass3, *)
+(*       assign_loc ce ty m b (Ptrofs.repr ofs) v m1 *)
+(*       /\ set_footprint_map (id, phl) vfp fpm = OK fpm1 *)
+(*       /\ coherent_fpm ce fpm1 mass3 *)
+(*       /\ m1 |= mass3 ** MP. *)
+(* Proof. *)
